@prefix dcterms: <http://purl.org/dc/terms/> .
@prefix meta: <https://w3id.org/biolink/biolinkml/meta/> .
@prefix owl: <http://www.w3.org/2002/07/owl#> .
@prefix rdfs: <http://www.w3.org/2000/01/rdf-schema#> .
@prefix skos: <http://www.w3.org/2004/02/skos/core#> .
@prefix xsd: <http://www.w3.org/2001/XMLSchema#> .

<http://rs.tdwg.org/dwc/terms> a owl:Ontology ;
    rdfs:label "terms" ;
    dcterms:license "https://creativecommons.org/publicdomain/zero/1.0/" ;
    skos:definition "DarwinCore biolinkml rendering" ;
    meta:generation_date "2021-02-04 09:34" ;
    meta:metamodel_version "1.7.0" ;
    meta:source_file "dwc.yaml" ;
    meta:source_file_date "Thu Feb  4 09:34:46 2021" ;
    meta:source_file_size 192315 .

<http://rs.tdwg.org/dwc/terms/Accepted_Scientific_Name> a owl:ObjectProperty,
        meta:SlotDefinition ;
    rdfs:label "Accepted Scientific Name" ;
    rdfs:range <https://w3id.org/biolink/biolinkml/meta/types/String> ;
    skos:definition "The currently valid (zoological) or accepted (botanical) name for the scientificName." .

<http://rs.tdwg.org/dwc/terms/Accepted_Scientific_Name_ID> a owl:ObjectProperty,
        meta:SlotDefinition ;
    rdfs:label "Accepted Scientific Name ID" ;
    rdfs:range <https://w3id.org/biolink/biolinkml/meta/types/String> ;
    skos:definition "A unique identifier for the acceptedScientificName." .

<http://rs.tdwg.org/dwc/terms/Accepted_Taxon> a owl:ObjectProperty,
        meta:SlotDefinition ;
    rdfs:label "Accepted Taxon" ;
    rdfs:range <https://w3id.org/biolink/biolinkml/meta/types/String> ;
    skos:definition "The currently valid (zoological) or accepted (botanical) name for the ScientificName." .

<http://rs.tdwg.org/dwc/terms/Accepted_Taxon_ID> a owl:ObjectProperty,
        meta:SlotDefinition ;
    rdfs:label "Accepted Taxon ID" ;
    rdfs:range <https://w3id.org/biolink/biolinkml/meta/types/String> ;
    skos:definition "An identifier for the name of the currently valid (zoological) or accepted (botanical) taxon. See acceptedTaxon." .

<http://rs.tdwg.org/dwc/terms/Accepted_Taxon_Name> a owl:ObjectProperty,
        meta:SlotDefinition ;
    rdfs:label "Accepted Taxon Name" ;
    rdfs:range <https://w3id.org/biolink/biolinkml/meta/types/String> ;
    skos:definition "The currently valid (zoological) or accepted (botanical) name for the scientificName." .

<http://rs.tdwg.org/dwc/terms/Accepted_Taxon_Name_ID> a owl:ObjectProperty,
        meta:SlotDefinition ;
    rdfs:label "Accepted Taxon Name ID" ;
    rdfs:range <https://w3id.org/biolink/biolinkml/meta/types/String> ;
    skos:definition "A unique identifier for the acceptedTaxonName." .

<http://rs.tdwg.org/dwc/terms/Access_Constraints> a owl:ObjectProperty,
        meta:SlotDefinition ;
    rdfs:label "Access Constraints" ;
    rdfs:range <https://w3id.org/biolink/biolinkml/meta/types/String> ;
    skos:definition "A description of constraints on the use of the data as shared or access to further data that is not shared." .

<http://rs.tdwg.org/dwc/terms/Accuracy> a owl:ObjectProperty,
        meta:SlotDefinition ;
    rdfs:label "Accuracy" ;
    rdfs:range <https://w3id.org/biolink/biolinkml/meta/types/String> ;
    skos:definition "Abstract term to capture error information about a measurement or fact." .

<http://rs.tdwg.org/dwc/terms/AgeClass> a owl:ObjectProperty,
        meta:SlotDefinition ;
    rdfs:label "AgeClass" ;
    rdfs:range <https://w3id.org/biolink/biolinkml/meta/types/String> ;
    skos:definition "The age class, reproductive stage, life stage of the biological individual (e.g., juvenile, adult, eft, nymph, etc.)." .

<http://rs.tdwg.org/dwc/terms/Attributes> a owl:ObjectProperty,
        meta:SlotDefinition ;
    rdfs:label "Attributes" ;
    rdfs:range <https://w3id.org/biolink/biolinkml/meta/types/String> ;
    skos:definition "List of additional measurements or characteristics (concatenated and separated) for which there is no existing semantic element, but which the data provider nevertheless feels the desire to share. Examples: \"Tragus length: 14mm; Weight: 120g\", \"Height: 1-1.5 meters tall; flowers yellow; uncommon\"." .

<http://rs.tdwg.org/dwc/terms/AuthorYearOfScientificName> a owl:ObjectProperty,
        meta:SlotDefinition ;
    rdfs:label "AuthorYearOfScientificName" ;
    rdfs:range <https://w3id.org/biolink/biolinkml/meta/types/String> ;
    skos:definition "The author of the ScientificName and the year of publication, if known. More than one author can be listed in a concatenated string. Should be formatted with parentheses and year according to the conventions of the applicable NomenclaturalCode." .

<http://rs.tdwg.org/dwc/terms/Basionym> a owl:ObjectProperty,
        meta:SlotDefinition ;
    rdfs:label "Basionym" ;
    rdfs:range <https://w3id.org/biolink/biolinkml/meta/types/String> ;
    skos:definition "The basionym (botany) or basonym (bacteriology) of the scientificName." .

<http://rs.tdwg.org/dwc/terms/Basionym_ID> a owl:ObjectProperty,
        meta:SlotDefinition ;
    rdfs:label "Basionym ID" ;
    rdfs:range <https://w3id.org/biolink/biolinkml/meta/types/String> ;
    skos:definition "A unique identifier for the basionym (botany) or basonym (bacteriology) of the scientificName." .

<http://rs.tdwg.org/dwc/terms/BasisOfRecord> a owl:ObjectProperty,
        meta:SlotDefinition ;
    rdfs:label "BasisOfRecord" ;
    rdfs:range <https://w3id.org/biolink/biolinkml/meta/types/String> ;
    skos:definition "A descriptive term indicating whether the record represents an object or observation. Examples: PreservedSpecimen- A physical object representing one or more organisms, part of organism, or artifact of an organism. synonyms: voucher, collection, lot. FossilSpecimen- A physical object representing one or more fossil organisms, part of fossil organism, or artifact of a fossil organism. LivingSpecimen- An organism removed from its natural occurrence and now living in captivity or cultivation. HumanObservation- A report by a known observer that an organism was present at the place and time. MachineObservation- A report by a monitoring device that an organism was present at the place and time. StillImage- An photograph, drawing, painting. MovingImage- A sequence of still images taken at regular intervals and intended to be played back as a moving image; may include sound. SoundRecording- An audio recording. OtherSpecimen- Any type of specimen not covered by any of the categories above." .

<http://rs.tdwg.org/dwc/terms/Basis_of_Record> a owl:ObjectProperty,
        meta:SlotDefinition ;
    rdfs:label "Basis of Record" ;
    rdfs:range <https://w3id.org/biolink/biolinkml/meta/types/String> ;
    skos:definition "The specific nature of the data record." .

<http://rs.tdwg.org/dwc/terms/Binomial> a owl:ObjectProperty,
        meta:SlotDefinition ;
    rdfs:label "Binomial" ;
    rdfs:range <https://w3id.org/biolink/biolinkml/meta/types/String> ;
    skos:definition "The combination of genus and first (species) epithet of the scientificName." .

<http://rs.tdwg.org/dwc/terms/BoundingBox> a owl:ObjectProperty,
        meta:SlotDefinition ;
    rdfs:label "BoundingBox" ;
    rdfs:range <https://w3id.org/biolink/biolinkml/meta/types/String> ;
    skos:definition "This access point provides a mechanism for performing searches using a bounding box. A Bounding Box element is not typically present in the database, but rather is derived from the DecimalLatitude and DecimalLongitude columns by the data provider." .

<http://rs.tdwg.org/dwc/terms/CatalogNumber> a owl:ObjectProperty,
        meta:SlotDefinition ;
    rdfs:label "CatalogNumber" ;
    rdfs:range <https://w3id.org/biolink/biolinkml/meta/types/String> ;
    skos:definition "The alphanumeric value identifying a record within the collection. It is highly recommended that each record be uniquely identified within a collection by this value. It is also recommended that each record be uniquely identified in a global context by the combination of InstitutionCode, CollectionCode and CatalogNumber." .

<http://rs.tdwg.org/dwc/terms/CatalogNumberNumeric> a owl:ObjectProperty,
        meta:SlotDefinition ;
    rdfs:label "CatalogNumberNumeric" ;
    rdfs:range <https://w3id.org/biolink/biolinkml/meta/types/String> ;
    skos:definition "The CatalogNumber as a numeric value, if applicable. Allows searching on numeric ranges of CatalogNumbers." .

<http://rs.tdwg.org/dwc/terms/CatalogNumberText> a owl:ObjectProperty,
        meta:SlotDefinition ;
    rdfs:label "CatalogNumberText" ;
    rdfs:range <https://w3id.org/biolink/biolinkml/meta/types/String> ;
    skos:definition "An alphanumeric value which identifies an individual cataloged item within the collection. It is recommended that this value provides a key by which the individual cataloged item can be identified." .

<http://rs.tdwg.org/dwc/terms/Catalog_Number_Numeric> a owl:ObjectProperty,
        meta:SlotDefinition ;
    rdfs:label "Catalog Number Numeric" ;
    rdfs:range <https://w3id.org/biolink/biolinkml/meta/types/String> ;
    skos:definition "The numeric value of the catalogNumber, used to facilitate numerical sorting and searching by ranges." .

<http://rs.tdwg.org/dwc/terms/CollectingMethod> a owl:ObjectProperty,
        meta:SlotDefinition ;
    rdfs:label "CollectingMethod" ;
    rdfs:range <https://w3id.org/biolink/biolinkml/meta/types/String> ;
    skos:definition "The name of, reference to, or brief description of the method or protocol under which the collecting event occurred. Examples: \"UV light trap\", \"mist net\", \"bottom trawl\"." .

<http://rs.tdwg.org/dwc/terms/CollectionCode> a owl:ObjectProperty,
        meta:SlotDefinition ;
    rdfs:label "CollectionCode" ;
    rdfs:range <https://w3id.org/biolink/biolinkml/meta/types/String> ;
    skos:definition "The code (or acronym) identifying the collection within the institution in which the organism record is cataloged." .

<http://rs.tdwg.org/dwc/terms/Collection_Code> a owl:ObjectProperty,
        meta:SlotDefinition ;
    rdfs:label "Collection Code" ;
    rdfs:range <https://w3id.org/biolink/biolinkml/meta/types/String> ;
    skos:definition "The name, acronym, coden, or initialism identifying the collection or data set from which the record was derived." .

<http://rs.tdwg.org/dwc/terms/Collection_ID> a owl:ObjectProperty,
        meta:SlotDefinition ;
    rdfs:label "Collection ID" ;
    rdfs:range <https://w3id.org/biolink/biolinkml/meta/types/String> ;
    skos:definition "An identifier for the collection or dataset from which the record was derived." .

<http://rs.tdwg.org/dwc/terms/Collector> a owl:ObjectProperty,
        meta:SlotDefinition ;
    rdfs:label "Collector" ;
    rdfs:range <https://w3id.org/biolink/biolinkml/meta/types/String> ;
    skos:definition "The name(s) (concatenated and separated) of collectors or observers. \"LIKE\" or \"contains\" substring query operations are meant to be used with this element to find matching collector names. The primary collector or observer, especially one whose CollectorNumber is also provided, should be listed first. Example: \"Oliver P. Pearson, Anita K. Pearson\" where the value in CollectorNumber \"OPP 7101\" corresponds to the number for the specimen in the field catalog (collector number) of Oliver P. Pearson." .

<http://rs.tdwg.org/dwc/terms/CollectorNumber> a owl:ObjectProperty,
        meta:SlotDefinition ;
    rdfs:label "CollectorNumber" ;
    rdfs:range <https://w3id.org/biolink/biolinkml/meta/types/String> ;
    skos:definition "An identifying string applied to the cataloged item at the time of collection. Serves as a link between field notes and the cataloged items." .

<http://rs.tdwg.org/dwc/terms/Continent> a owl:ObjectProperty,
        meta:SlotDefinition ;
    rdfs:label "Continent" ;
    rdfs:range <https://w3id.org/biolink/biolinkml/meta/types/String> ;
    skos:definition "The full, unabbreviated name of the continent on which the organism was collected or observed." .

<http://rs.tdwg.org/dwc/terms/ContinentOcean> a owl:ObjectProperty,
        meta:SlotDefinition ;
    rdfs:label "ContinentOcean" ;
    rdfs:range <https://w3id.org/biolink/biolinkml/meta/types/String> ;
    skos:definition "The full, unabbreviated name of the continent or ocean from which the cataloged item was collected." .

<http://rs.tdwg.org/dwc/terms/CoordinatePrecision> a owl:ObjectProperty,
        meta:SlotDefinition ;
    rdfs:label "CoordinatePrecision" ;
    rdfs:range <https://w3id.org/biolink/biolinkml/meta/types/String> ;
    skos:definition "An estimate of how tightly the collecting locality was specified; expressed as a distance, in meters, that corresponds to a radius around the latitude-longitude coordinates. Use NULL where precision is unknown, cannot be estimated, or is not applicable." .

<http://rs.tdwg.org/dwc/terms/CoordinateUncertaintyInMeters> a owl:ObjectProperty,
        meta:SlotDefinition ;
    rdfs:label "CoordinateUncertaintyInMeters" ;
    rdfs:range <https://w3id.org/biolink/biolinkml/meta/types/String> ;
    skos:definition "The upper limit of the distance (in meters) from the given DecimalLatitude and DecimalLongitude describing a circle within which the whole of the described locality lies. Leave the value empty if the uncertainty is unknown, cannot be estimated, or is not applicable (because there are no coordinates). Describes the point-radius representation of the location, along with DecimalLatitude, DecimalLongitude, and GeodeticDatum. Zero is not a valid value for this element." .

<http://rs.tdwg.org/dwc/terms/Coordinate_Precision> a owl:ObjectProperty,
        meta:SlotDefinition ;
    rdfs:label "Coordinate Precision" ;
    rdfs:range <https://w3id.org/biolink/biolinkml/meta/types/String> ;
    skos:definition "A decimal representation of the precision of the coordinates given in the decimalLatitude and decimalLongitude." .

<http://rs.tdwg.org/dwc/terms/Coordinate_Uncertainty_In_Meters> a owl:ObjectProperty,
        meta:SlotDefinition ;
    rdfs:label "Coordinate Uncertainty In Meters" ;
    rdfs:range <https://w3id.org/biolink/biolinkml/meta/types/String> ;
    skos:definition "The horizontal distance (in meters) from the given decimalLatitude and decimalLongitude describing the smallest circle containing the whole of the Location. Leave the value empty if the uncertainty is unknown, cannot be estimated, or is not applicable (because there are no coordinates). Zero is not a valid value for this term." .

<http://rs.tdwg.org/dwc/terms/Country> a owl:ObjectProperty,
        meta:SlotDefinition ;
    rdfs:label "Country" ;
    rdfs:range <https://w3id.org/biolink/biolinkml/meta/types/String> ;
    skos:definition "The full, unabbreviated name of the country or major political unit in which the organism was collected or observed." .

<http://rs.tdwg.org/dwc/terms/Country_Code> a owl:ObjectProperty,
        meta:SlotDefinition ;
    rdfs:label "Country Code" ;
    rdfs:range <https://w3id.org/biolink/biolinkml/meta/types/String> ;
    skos:definition "The standard code for the country in which the Location occurs. Recommended best practice is to use ISO 3166-1-alpha-2 country codes." .

<http://rs.tdwg.org/dwc/terms/County> a owl:ObjectProperty,
        meta:SlotDefinition ;
    rdfs:label "County" ;
    rdfs:range <https://w3id.org/biolink/biolinkml/meta/types/String> ;
    skos:definition "The full, unabbreviated name of the county, shire, or municipality (i.e., the next smaller political region than StateProvince) in which the organism was collected or observed." .

<http://rs.tdwg.org/dwc/terms/Data_Generalizations> a owl:ObjectProperty,
        meta:SlotDefinition ;
    rdfs:label "Data Generalizations" ;
    rdfs:range <https://w3id.org/biolink/biolinkml/meta/types/String> ;
    skos:definition "Actions taken to make the shared data less specific or complete than in its original form. Suggests that alternative data of higher quality may be available on request." .

<http://rs.tdwg.org/dwc/terms/Dataset> a owl:Class,
        meta:ClassDefinition ;
    rdfs:label "Dataset" ;
    skos:altLabel "Dataset" ;
    skos:definition "The category of information pertaining to a logical set of records." .

<http://rs.tdwg.org/dwc/terms/Dataset_ID> a owl:ObjectProperty,
        meta:SlotDefinition ;
    rdfs:label "Dataset ID" ;
    rdfs:range <https://w3id.org/biolink/biolinkml/meta/types/String> ;
    skos:definition "An identifier for the set of data. May be a global unique identifier or an identifier specific to a collection or institution." .

<http://rs.tdwg.org/dwc/terms/Dataset_Name> a owl:ObjectProperty,
        meta:SlotDefinition ;
    rdfs:label "Dataset Name" ;
    rdfs:range <https://w3id.org/biolink/biolinkml/meta/types/String> ;
    skos:definition "The name identifying the data set from which the record was derived." .

<http://rs.tdwg.org/dwc/terms/DateIdentified> a owl:ObjectProperty,
        meta:SlotDefinition ;
    rdfs:label "DateIdentified" ;
    rdfs:range <https://w3id.org/biolink/biolinkml/meta/types/String> ;
    skos:definition "The date-time in the Common Era calendar in which the object or observation was identified as being a member of the taxon given in the ScientificName." .

<http://rs.tdwg.org/dwc/terms/DateLastModified> a owl:ObjectProperty,
        meta:SlotDefinition ;
    rdfs:label "DateLastModified" ;
    rdfs:range <https://w3id.org/biolink/biolinkml/meta/types/String> ;
    skos:definition "The last date-time of publication when any of the data for the record were modified from the previous publication of that record. When publishing a record for the first time, use the publication date-time. Returns values as ISO 8601 date and time. (cf. http://www.w3.org/TR/xmlschema-2/#isoformats and http://www.iso.org/iso/en/prods-services/popstds/dateandtime.html Example: November 5, 1994, 8:15:30 am, US Eastern Standard Time\" would be \"1994-11-05T13:15:30Z\"" .

<http://rs.tdwg.org/dwc/terms/DayCollected> a owl:ObjectProperty,
        meta:SlotDefinition ;
    rdfs:label "DayCollected" ;
    rdfs:range <https://w3id.org/biolink/biolinkml/meta/types/String> ;
    skos:definition "The two digit day of the month in the Common Era calendar during which the cataloged item was collected from the field." .

<http://rs.tdwg.org/dwc/terms/DayIdentified> a owl:ObjectProperty,
        meta:SlotDefinition ;
    rdfs:label "DayIdentified" ;
    rdfs:range <https://w3id.org/biolink/biolinkml/meta/types/String> ;
    skos:definition "The two digit day of the month in the Common Era calendar during which the cataloged item was identified." .

<http://rs.tdwg.org/dwc/terms/DayOfYear> a owl:ObjectProperty,
        meta:SlotDefinition ;
    rdfs:label "DayOfYear" ;
    rdfs:range <https://w3id.org/biolink/biolinkml/meta/types/String> ;
    skos:definition "The ordinal day of the year on which the object or observation was collected (1 for January 1, 365 for December 31, except in a leap year, in which case it is 366). If the EarliestDateCollected and LatestDateCollected do not occur on the same day, do not populate DayOfYear." .

<http://rs.tdwg.org/dwc/terms/DecimalLatitude> a owl:ObjectProperty,
        meta:SlotDefinition ;
    rdfs:label "DecimalLatitude" ;
    rdfs:range <https://w3id.org/biolink/biolinkml/meta/types/String> ;
    skos:definition "The latitude of the geographic center of a location where an event occurred (organism collected, observation made), expressed in decimal degrees. Positive values are North of the Equator, negative values are South of the Equator. Describes the point-radius representation of the location, along with DecimalLongitude, GeodeticDatum, and CoordinateUncertaintyInMeters. Example: -41.0983423" .

<http://rs.tdwg.org/dwc/terms/DecimalLongitude> a owl:ObjectProperty,
        meta:SlotDefinition ;
    rdfs:label "DecimalLongitude" ;
    rdfs:range <https://w3id.org/biolink/biolinkml/meta/types/String> ;
    skos:definition "The longitude of the geographic center of a location where an event occurred (organism collected, observation made), expressed in decimal degrees. Positive values are East of the Greenwich Meridian, negative values are West of the Greenwich Meridian. Describes the point-radius representation of the location, along with DecimalLatitude, GeodeticDatum, and CoordinateUncertaintyInMeters. Example: -71.0943235" .

<http://rs.tdwg.org/dwc/terms/Decimal_Latitude> a owl:ObjectProperty,
        meta:SlotDefinition ;
    rdfs:label "Decimal Latitude" ;
    rdfs:range <https://w3id.org/biolink/biolinkml/meta/types/String> ;
    skos:definition "The geographic latitude (in decimal degrees, using the spatial reference system given in geodeticDatum) of the geographic center of a Location. Positive values are north of the Equator, negative values are south of it. Legal values lie between -90 and 90, inclusive." .

<http://rs.tdwg.org/dwc/terms/Decimal_Longitude> a owl:ObjectProperty,
        meta:SlotDefinition ;
    rdfs:label "Decimal Longitude" ;
    rdfs:range <https://w3id.org/biolink/biolinkml/meta/types/String> ;
    skos:definition "The geographic longitude (in decimal degrees, using the spatial reference system given in geodeticDatum) of the geographic center of a Location. Positive values are east of the Greenwich Meridian, negative values are west of it. Legal values lie between -180 and 180, inclusive." .

<http://rs.tdwg.org/dwc/terms/Dynamic_Properties> a owl:ObjectProperty,
        meta:SlotDefinition ;
    rdfs:label "Dynamic Properties" ;
    rdfs:range <https://w3id.org/biolink/biolinkml/meta/types/String> ;
    skos:definition "A list of additional measurements, facts, characteristics, or assertions about the record. Meant to provide a mechanism for structured content." .

<http://rs.tdwg.org/dwc/terms/EarliestAgeOrLowestStage> a owl:ObjectProperty,
        meta:SlotDefinition ;
    rdfs:label "EarliestAgeOrLowestStage" ;
    rdfs:range <https://w3id.org/biolink/biolinkml/meta/types/String> ;
    skos:definition "The full name of the earliest possible geochronologic age or lowest chronostratigraphic stage attributable to the stratigraphic horizon from which the cataloged item was collected." .

<http://rs.tdwg.org/dwc/terms/EarliestDateCollected> a owl:ObjectProperty,
        meta:SlotDefinition ;
    rdfs:label "EarliestDateCollected" ;
    rdfs:range <https://w3id.org/biolink/biolinkml/meta/types/String> ;
    skos:definition "The earliest date-time (Common Era calendar) in a date-time period during which an organism or group of organisms was collected or observed. If the event is recorded as occurring at a single date-time, populate both EarliestDateCollected and LatestDateCollected with the same value." .

<http://rs.tdwg.org/dwc/terms/EarliestEonOrLowestEonothem> a owl:ObjectProperty,
        meta:SlotDefinition ;
    rdfs:label "EarliestEonOrLowestEonothem" ;
    rdfs:range <https://w3id.org/biolink/biolinkml/meta/types/String> ;
    skos:definition "The full name of the earliest possible geochronologic eon or lowest chrono-stratigraphic eonothem or the informal name (\"Precambrian\") attributable to the stratigraphic horizon from which the cataloged item was collected." .

<http://rs.tdwg.org/dwc/terms/EarliestEpochOrLowestSeries> a owl:ObjectProperty,
        meta:SlotDefinition ;
    rdfs:label "EarliestEpochOrLowestSeries" ;
    rdfs:range <https://w3id.org/biolink/biolinkml/meta/types/String> ;
    skos:definition "The full name of the earliest possible geochronologic epoch or lowest chronostratigraphic series attributable to the stratigraphic horizon from which the cataloged item was collected." .

<http://rs.tdwg.org/dwc/terms/EarliestEraOrLowestErathem> a owl:ObjectProperty,
        meta:SlotDefinition ;
    rdfs:label "EarliestEraOrLowestErathem" ;
    rdfs:range <https://w3id.org/biolink/biolinkml/meta/types/String> ;
    skos:definition "The full name of the earliest possible geochronologic era or lowest chronostratigraphic erathem attributable to the stratigraphic horizon from which the cataloged item was collected." .

<http://rs.tdwg.org/dwc/terms/EarliestPeriodOrLowestSystem> a owl:ObjectProperty,
        meta:SlotDefinition ;
    rdfs:label "EarliestPeriodOrLowestSystem" ;
    rdfs:range <https://w3id.org/biolink/biolinkml/meta/types/String> ;
    skos:definition "The full name of the earliest possible geochronologic period or lowest chronostratigraphic system attributable to the stratigraphic horizon from which the cataloged item was collected." .

<http://rs.tdwg.org/dwc/terms/Earliest_Date_Collected> a owl:ObjectProperty,
        meta:SlotDefinition ;
    rdfs:label "Earliest Date Collected" ;
    rdfs:range <https://w3id.org/biolink/biolinkml/meta/types/String> ;
    skos:definition "The earliest date-time in a period during which a event occurred. If the event is recorded as occurring at a single date-time, populate both EarliestDateCollected and LatestDateCollected with the same value. Recommended best practice is to use an encoding scheme, such as ISO 8601:2004(E)." .

<http://rs.tdwg.org/dwc/terms/End_Time_of_Day> a owl:ObjectProperty,
        meta:SlotDefinition ;
    rdfs:label "End Time of Day" ;
    rdfs:range <https://w3id.org/biolink/biolinkml/meta/types/String> ;
    skos:definition "The time of day when the event ended, expressed as decimal hours from midnight, local time." .

<http://rs.tdwg.org/dwc/terms/Event> a owl:Class,
        meta:ClassDefinition ;
    rdfs:label "Event" ;
    rdfs:subClassOf [ a owl:Restriction ;
            owl:maxQualifiedCardinality 1 ;
            owl:onClass <https://w3id.org/biolink/biolinkml/meta/types/String> ;
            owl:onProperty <http://rs.tdwg.org/dwc/terms/Field_Number> ],
        [ a owl:Restriction ;
            owl:maxQualifiedCardinality 1 ;
            owl:onClass <https://w3id.org/biolink/biolinkml/meta/types/String> ;
            owl:onProperty <http://rs.tdwg.org/dwc/terms/day> ],
        [ a owl:Restriction ;
            owl:maxQualifiedCardinality 1 ;
            owl:onClass <https://w3id.org/biolink/biolinkml/meta/types/String> ;
            owl:onProperty <http://rs.tdwg.org/dwc/terms/Event_Time> ],
        [ a owl:Restriction ;
            owl:maxQualifiedCardinality 1 ;
            owl:onClass <https://w3id.org/biolink/biolinkml/meta/types/String> ;
            owl:onProperty <http://rs.tdwg.org/dwc/terms/habitat> ],
        [ a owl:Restriction ;
            owl:maxQualifiedCardinality 1 ;
            owl:onClass <https://w3id.org/biolink/biolinkml/meta/types/String> ;
            owl:onProperty <http://rs.tdwg.org/dwc/terms/Habitat> ],
        [ a owl:Restriction ;
            owl:maxQualifiedCardinality 1 ;
            owl:onClass <https://w3id.org/biolink/biolinkml/meta/types/String> ;
            owl:onProperty <http://rs.tdwg.org/dwc/terms/Event_Date> ],
        [ a owl:Restriction ;
            owl:maxQualifiedCardinality 1 ;
            owl:onClass <https://w3id.org/biolink/biolinkml/meta/types/String> ;
            owl:onProperty <http://rs.tdwg.org/dwc/terms/Sampling_Effort> ],
        [ a owl:Restriction ;
            owl:maxQualifiedCardinality 1 ;
            owl:onClass <https://w3id.org/biolink/biolinkml/meta/types/String> ;
            owl:onProperty <http://rs.tdwg.org/dwc/terms/Month> ],
        [ a owl:Restriction ;
            owl:maxQualifiedCardinality 1 ;
            owl:onClass <https://w3id.org/biolink/biolinkml/meta/types/String> ;
            owl:onProperty <http://rs.tdwg.org/dwc/terms/Field_Notes> ],
        [ a owl:Restriction ;
            owl:maxQualifiedCardinality 1 ;
            owl:onClass <https://w3id.org/biolink/biolinkml/meta/types/String> ;
            owl:onProperty <http://rs.tdwg.org/dwc/terms/fieldNotes> ],
        [ a owl:Restriction ;
            owl:maxQualifiedCardinality 1 ;
            owl:onClass <https://w3id.org/biolink/biolinkml/meta/types/String> ;
            owl:onProperty <http://rs.tdwg.org/dwc/terms/Day> ],
        [ a owl:Restriction ;
            owl:maxQualifiedCardinality 1 ;
            owl:onClass <https://w3id.org/biolink/biolinkml/meta/types/String> ;
            owl:onProperty <http://rs.tdwg.org/dwc/terms/parentEventID> ],
        [ a owl:Restriction ;
            owl:maxQualifiedCardinality 1 ;
            owl:onClass <https://w3id.org/biolink/biolinkml/meta/types/String> ;
            owl:onProperty <http://rs.tdwg.org/dwc/terms/startDayOfYear> ],
        [ a owl:Restriction ;
            owl:maxQualifiedCardinality 1 ;
            owl:onClass <https://w3id.org/biolink/biolinkml/meta/types/String> ;
            owl:onProperty <http://rs.tdwg.org/dwc/terms/Sampling_Protocol> ],
        [ a owl:Restriction ;
            owl:maxQualifiedCardinality 1 ;
            owl:onClass <https://w3id.org/biolink/biolinkml/meta/types/String> ;
            owl:onProperty <http://rs.tdwg.org/dwc/terms/verbatimEventDate> ],
        [ a owl:Restriction ;
            owl:maxQualifiedCardinality 1 ;
            owl:onClass <https://w3id.org/biolink/biolinkml/meta/types/String> ;
            owl:onProperty <http://rs.tdwg.org/dwc/terms/End_Day_Of_Year> ],
        [ a owl:Restriction ;
            owl:maxQualifiedCardinality 1 ;
            owl:onClass <https://w3id.org/biolink/biolinkml/meta/types/String> ;
            owl:onProperty <http://rs.tdwg.org/dwc/terms/Sample_Size_Unit> ],
        [ a owl:Restriction ;
            owl:maxQualifiedCardinality 1 ;
            owl:onClass <https://w3id.org/biolink/biolinkml/meta/types/String> ;
            owl:onProperty <http://rs.tdwg.org/dwc/terms/month> ],
        [ a owl:Restriction ;
            owl:maxQualifiedCardinality 1 ;
            owl:onClass <https://w3id.org/biolink/biolinkml/meta/types/String> ;
            owl:onProperty <http://rs.tdwg.org/dwc/terms/Start_Day_Of_Year> ],
        [ a owl:Restriction ;
            owl:maxQualifiedCardinality 1 ;
            owl:onClass <https://w3id.org/biolink/biolinkml/meta/types/String> ;
            owl:onProperty <http://rs.tdwg.org/dwc/terms/samplingEffort> ],
        [ a owl:Restriction ;
            owl:maxQualifiedCardinality 1 ;
            owl:onClass <https://w3id.org/biolink/biolinkml/meta/types/String> ;
            owl:onProperty <http://rs.tdwg.org/dwc/terms/Verbatim_EventDate> ],
        [ a owl:Restriction ;
            owl:maxQualifiedCardinality 1 ;
            owl:onClass <https://w3id.org/biolink/biolinkml/meta/types/String> ;
            owl:onProperty <http://rs.tdwg.org/dwc/terms/year> ],
        [ a owl:Restriction ;
            owl:maxQualifiedCardinality 1 ;
            owl:onClass <https://w3id.org/biolink/biolinkml/meta/types/String> ;
            owl:onProperty <http://rs.tdwg.org/dwc/terms/eventRemarks> ],
        [ a owl:Restriction ;
            owl:maxQualifiedCardinality 1 ;
            owl:onClass <https://w3id.org/biolink/biolinkml/meta/types/String> ;
            owl:onProperty <http://rs.tdwg.org/dwc/terms/Event_ID> ],
        [ a owl:Restriction ;
            owl:maxQualifiedCardinality 1 ;
            owl:onClass <https://w3id.org/biolink/biolinkml/meta/types/String> ;
            owl:onProperty <http://rs.tdwg.org/dwc/terms/eventTime> ],
        [ a owl:Restriction ;
            owl:maxQualifiedCardinality 1 ;
            owl:onClass <https://w3id.org/biolink/biolinkml/meta/types/String> ;
            owl:onProperty <http://rs.tdwg.org/dwc/terms/samplingProtocol> ],
        [ a owl:Restriction ;
            owl:maxQualifiedCardinality 1 ;
            owl:onClass <https://w3id.org/biolink/biolinkml/meta/types/String> ;
            owl:onProperty <http://rs.tdwg.org/dwc/terms/eventDate> ],
        [ a owl:Restriction ;
            owl:maxQualifiedCardinality 1 ;
            owl:onClass <https://w3id.org/biolink/biolinkml/meta/types/String> ;
            owl:onProperty <http://rs.tdwg.org/dwc/terms/sampleSizeUnit> ],
        [ a owl:Restriction ;
            owl:maxQualifiedCardinality 1 ;
            owl:onClass <https://w3id.org/biolink/biolinkml/meta/types/String> ;
            owl:onProperty <http://rs.tdwg.org/dwc/terms/Year> ],
        [ a owl:Restriction ;
            owl:maxQualifiedCardinality 1 ;
            owl:onClass <https://w3id.org/biolink/biolinkml/meta/types/String> ;
            owl:onProperty <http://rs.tdwg.org/dwc/terms/Sample_Size_Value> ],
        [ a owl:Restriction ;
            owl:maxQualifiedCardinality 1 ;
            owl:onClass <https://w3id.org/biolink/biolinkml/meta/types/String> ;
            owl:onProperty <http://rs.tdwg.org/dwc/terms/Parent_Event_ID> ],
        [ a owl:Restriction ;
            owl:maxQualifiedCardinality 1 ;
            owl:onClass <https://w3id.org/biolink/biolinkml/meta/types/String> ;
            owl:onProperty <http://rs.tdwg.org/dwc/terms/eventID> ],
        [ a owl:Restriction ;
            owl:maxQualifiedCardinality 1 ;
            owl:onClass <https://w3id.org/biolink/biolinkml/meta/types/String> ;
            owl:onProperty <http://rs.tdwg.org/dwc/terms/fieldNumber> ],
        [ a owl:Restriction ;
            owl:maxQualifiedCardinality 1 ;
            owl:onClass <https://w3id.org/biolink/biolinkml/meta/types/String> ;
            owl:onProperty <http://rs.tdwg.org/dwc/terms/endDayOfYear> ],
        [ a owl:Restriction ;
            owl:maxQualifiedCardinality 1 ;
            owl:onClass <https://w3id.org/biolink/biolinkml/meta/types/String> ;
            owl:onProperty <http://rs.tdwg.org/dwc/terms/sampleSizeValue> ],
        [ a owl:Restriction ;
            owl:maxQualifiedCardinality 1 ;
            owl:onClass <https://w3id.org/biolink/biolinkml/meta/types/String> ;
            owl:onProperty <http://rs.tdwg.org/dwc/terms/Event_Remarks> ] ;
    skos:altLabel "Event" ;
    skos:definition "An action that occurs at some location during some time." ;
    skos:exactMatch <http://rs.tdwg.org/dwc/terms/version/Event-2009-04-29> .

<http://rs.tdwg.org/dwc/terms/EventAttribute> a owl:Class,
        meta:ClassDefinition ;
    rdfs:label "Event Attribute" ;
    skos:altLabel "Event Attribute" ;
    skos:definition "Container class for information about attributes related to a given sampling event." .

<http://rs.tdwg.org/dwc/terms/EventMeasurement> a owl:Class,
        meta:ClassDefinition ;
    rdfs:label "Event Measurement" ;
    skos:altLabel "Event Measurement" ;
    skos:definition "The category of information pertaining to measurements associated with an event." .

<http://rs.tdwg.org/dwc/terms/Event_Attribute> a owl:ObjectProperty,
        meta:SlotDefinition ;
    rdfs:label "Event Attribute" ;
    rdfs:range <https://w3id.org/biolink/biolinkml/meta/types/String> ;
    skos:definition "The value of the measurement or characteristic of the sampling event." .

<http://rs.tdwg.org/dwc/terms/Event_Attribute_Accuracy> a owl:ObjectProperty,
        meta:SlotDefinition ;
    rdfs:label "Event Attribute Accuracy" ;
    rdfs:range <https://w3id.org/biolink/biolinkml/meta/types/String> ;
    skos:definition "The description of the error associated with the EventAttributeValue." .

<http://rs.tdwg.org/dwc/terms/Event_Attribute_Determined_By> a owl:ObjectProperty,
        meta:SlotDefinition ;
    rdfs:label "Event Attribute Determined By" ;
    rdfs:range <https://w3id.org/biolink/biolinkml/meta/types/String> ;
    skos:definition "The agent responsible for having determined the value of the measurement or characteristic of the sampling event." .

<http://rs.tdwg.org/dwc/terms/Event_Attribute_Determined_Date> a owl:ObjectProperty,
        meta:SlotDefinition ;
    rdfs:label "Event Attribute Determined Date" ;
    rdfs:range <https://w3id.org/biolink/biolinkml/meta/types/String> ;
    skos:definition "The date on which the the measurement or characteristic of the sampling event was made." .

<http://rs.tdwg.org/dwc/terms/Event_Attribute_ID> a owl:ObjectProperty,
        meta:SlotDefinition ;
    rdfs:label "Event Attribute ID" ;
    rdfs:range <https://w3id.org/biolink/biolinkml/meta/types/String> ;
    skos:definition "An identifier for the event attribute. May be a global unique identifier or an identifier specific to the data set." .

<http://rs.tdwg.org/dwc/terms/Event_Attribute_Remarks> a owl:ObjectProperty,
        meta:SlotDefinition ;
    rdfs:label "Event Attribute Remarks" ;
    rdfs:range <https://w3id.org/biolink/biolinkml/meta/types/String> ;
    skos:definition "Comments or notes accompanying the measurement or characteristic of the sampling event." .

<http://rs.tdwg.org/dwc/terms/Event_Attribute_Type> a owl:ObjectProperty,
        meta:SlotDefinition ;
    rdfs:label "Event Attribute Type" ;
    rdfs:range <https://w3id.org/biolink/biolinkml/meta/types/String> ;
    skos:definition "The nature of the measurement or characteristic of the sampling event. Recommended best practice is to use a controlled vocabulary." .

<http://rs.tdwg.org/dwc/terms/Event_Attribute_Unit> a owl:ObjectProperty,
        meta:SlotDefinition ;
    rdfs:label "Event Attribute Unit" ;
    rdfs:range <https://w3id.org/biolink/biolinkml/meta/types/String> ;
    skos:definition "The units for the value of the measurement or characteristic of the sampling event. Recommended best practice is to use International System of Units (SI) units." .

<http://rs.tdwg.org/dwc/terms/Event_Attributes> a owl:ObjectProperty,
        meta:SlotDefinition ;
    rdfs:label "Event Attributes" ;
    rdfs:range <https://w3id.org/biolink/biolinkml/meta/types/String> ;
    skos:definition "A list (concatenated and separated) of additional measurements or characteristics of the Event." .

<http://rs.tdwg.org/dwc/terms/Event_Measurement_Accuracy> a owl:ObjectProperty,
        meta:SlotDefinition ;
    rdfs:label "Event Measurement Accuracy" ;
    rdfs:range <https://w3id.org/biolink/biolinkml/meta/types/String> ;
    skos:definition "The description of the error associated with the EventAttributeValue." .

<http://rs.tdwg.org/dwc/terms/Event_Measurement_Determined_By> a owl:ObjectProperty,
        meta:SlotDefinition ;
    rdfs:label "Event Measurement Determined By" ;
    rdfs:range <https://w3id.org/biolink/biolinkml/meta/types/String> ;
    skos:definition "The agent responsible for having determined the value of the measurement or characteristic of the event." .

<http://rs.tdwg.org/dwc/terms/Event_Measurement_Determined_Date> a owl:ObjectProperty,
        meta:SlotDefinition ;
    rdfs:label "Event Measurement Determined Date" ;
    rdfs:range <https://w3id.org/biolink/biolinkml/meta/types/String> ;
    skos:definition "The date on which the the measurement or characteristic of the event was made. Recommended best practice is to use an encoding scheme, such as ISO 8601:2004(E)." .

<http://rs.tdwg.org/dwc/terms/Event_Measurement_ID> a owl:ObjectProperty,
        meta:SlotDefinition ;
    rdfs:label "Event Measurement ID" ;
    rdfs:range <https://w3id.org/biolink/biolinkml/meta/types/String> ;
    skos:definition "An identifier for the event attribute. May be a global unique identifier or an identifier specific to the data set." .

<http://rs.tdwg.org/dwc/terms/Event_Measurement_Remarks> a owl:ObjectProperty,
        meta:SlotDefinition ;
    rdfs:label "Event Measurement Remarks" ;
    rdfs:range <https://w3id.org/biolink/biolinkml/meta/types/String> ;
    skos:definition "Comments or notes accompanying the measurement or characteristic of the event." .

<http://rs.tdwg.org/dwc/terms/Event_Measurement_Type> a owl:ObjectProperty,
        meta:SlotDefinition ;
    rdfs:label "Event Measurement Type" ;
    rdfs:range <https://w3id.org/biolink/biolinkml/meta/types/String> ;
    skos:definition "The nature of the measurement or characteristic of the event. Recommended best practice is to use a controlled vocabulary." .

<http://rs.tdwg.org/dwc/terms/Event_Measurement_Unit> a owl:ObjectProperty,
        meta:SlotDefinition ;
    rdfs:label "Event Measurement Unit" ;
    rdfs:range <https://w3id.org/biolink/biolinkml/meta/types/String> ;
    skos:definition "The units for the value of the measurement or characteristic of the event. Recommended best practice is to use International System of Units (SI) units." .

<http://rs.tdwg.org/dwc/terms/Event_Measurement_Value> a owl:ObjectProperty,
        meta:SlotDefinition ;
    rdfs:label "Event Measurement Value" ;
    rdfs:range <https://w3id.org/biolink/biolinkml/meta/types/String> ;
    skos:definition "The value of the measurement or characteristic of the event." .

<http://rs.tdwg.org/dwc/terms/FieldNotes> a owl:ObjectProperty,
        meta:SlotDefinition ;
    rdfs:label "FieldNotes" ;
    rdfs:range <https://w3id.org/biolink/biolinkml/meta/types/String> ;
    skos:definition "A reference to, or flag marking the existence of notes taken in the field for the cataloged item." .

<http://rs.tdwg.org/dwc/terms/FieldNumber> a owl:ObjectProperty,
        meta:SlotDefinition ;
    rdfs:label "FieldNumber" ;
    rdfs:range <https://w3id.org/biolink/biolinkml/meta/types/String> ;
    skos:definition "An identifying string applied to a set of material that resulted from a single collecting event." .

<http://rs.tdwg.org/dwc/terms/FootprintSpatialFit> a owl:ObjectProperty,
        meta:SlotDefinition ;
    rdfs:label "FootprintSpatialFit" ;
    rdfs:range <https://w3id.org/biolink/biolinkml/meta/types/String> ;
    skos:definition "A measure of how well the geometry expressed in the footprint match the original spatial representation, as a ratio of the area of the footprint given to the area of the original spatial representation. Legal values are 0, greater than or equal to 1, or undefined. A value of 1 is an exact match or 100% overlap. A value of 0 should be used if the given georeference does not completely contain the original representation. The FootprintSpatialFit is undefined if the original representation is a point without uncertainty and the given georeference is not that same point (without uncertainty). If both the original and the given georeference are the same point, the FootprintSpatialFit is 1. Detailed explanations with graphical examples can be found in the Guide to Best Practices for Georeferencing (Chapman and Wieczorek, eds. 2006)." .

<http://rs.tdwg.org/dwc/terms/FootprintWKT> a owl:ObjectProperty,
        meta:SlotDefinition ;
    rdfs:label "FootprintWKT" ;
    rdfs:range <https://w3id.org/biolink/biolinkml/meta/types/String> ;
    skos:definition "A Well-Known Text (WKT; see http://en.wikipedia.org/wiki/Well-known_text) representation of the the shape (footprint, geometry) that defines the location of the occurrence. The same place may have both a point-radius representation (see DecimalLatitude) and a footprint representation, and they may differ from each other for the same occurrence. Example: the one-degree bounding box with opposite corners at (longitude=10, latitude=20) and (longitude=11, latitude=21) would be expressed in well-known text as POLYGON ((10 20, 11 20, 11 21, 10 21, 10 20))" .

<http://rs.tdwg.org/dwc/terms/Footprint_SRS> a owl:ObjectProperty,
        meta:SlotDefinition ;
    rdfs:label "Footprint SRS" ;
    rdfs:range <https://w3id.org/biolink/biolinkml/meta/types/String> ;
    skos:definition "A Well-Known Text (WKT) representation of the Spatial Reference System (SRS) for the footprintWKT of the Location. Do not use this term to describe the SRS of the decimalLatitude and decimalLongitude, even if it is the same as for the footprintWKT - use the geodeticDatum instead." .

<http://rs.tdwg.org/dwc/terms/Footprint_Spatial_Fit> a owl:ObjectProperty,
        meta:SlotDefinition ;
    rdfs:label "Footprint Spatial Fit" ;
    rdfs:range <https://w3id.org/biolink/biolinkml/meta/types/String> ;
    skos:definition "The ratio of the area of the footprint (footprintWKT) to the area of the true (original, or most specific) spatial representation of the Location. Legal values are 0, greater than or equal to 1, or undefined. A value of 1 is an exact match or 100% overlap. A value of 0 should be used if the given footprint does not completely contain the original representation. The footprintSpatialFit is undefined (and should be left blank) if the original representation is a point and the given georeference is not that same point. If both the original and the given georeference are the same point, the footprintSpatialFit is 1." .

<http://rs.tdwg.org/dwc/terms/Footprint_WKT> a owl:ObjectProperty,
        meta:SlotDefinition ;
    rdfs:label "Footprint WKT" ;
    rdfs:range <https://w3id.org/biolink/biolinkml/meta/types/String> ;
    skos:definition "A Well-Known Text (WKT) representation of the shape (footprint, geometry) that defines the Location. A Location may have both a point-radius representation (see decimalLatitude) and a footprint representation, and they may differ from each other." .

<http://rs.tdwg.org/dwc/terms/FossilSpecimen> a owl:Class,
        meta:ClassDefinition ;
    rdfs:label "Fossil Specimen",
        "FossilSpecimen" ;
    skos:altLabel "Fossil Specimen",
        "FossilSpecimen" ;
    skos:definition "A preserved specimen that is a fossil." ;
    skos:exactMatch <http://rs.tdwg.org/dwc/dwctype/version/FossilSpecimen-2011-10-16>,
        <http://rs.tdwg.org/dwc/dwctype/version/FossilSpecimen-2014-10-23> .

<http://rs.tdwg.org/dwc/terms/GenBankNum> a owl:ObjectProperty,
        meta:SlotDefinition ;
    rdfs:label "GenBankNum" ;
    rdfs:range <https://w3id.org/biolink/biolinkml/meta/types/String> ;
    skos:definition "GenBank Accession number." .

<http://rs.tdwg.org/dwc/terms/GenBankNumber> a owl:ObjectProperty,
        meta:SlotDefinition ;
    rdfs:label "GenBankNumber" ;
    rdfs:range <https://w3id.org/biolink/biolinkml/meta/types/String> ;
    skos:definition "GenBank Accession number(s) associated with the biological individual(s) referred to by the cataloged object." .

<http://rs.tdwg.org/dwc/terms/Generalizations> a owl:ObjectProperty,
        meta:SlotDefinition ;
    rdfs:label "Generalizations" ;
    rdfs:range <https://w3id.org/biolink/biolinkml/meta/types/String> ;
    skos:definition "Actions taken to make the data as shared less specific or complete than in its original form. Suggests that alternative data of highly quality may be available on request." .

<http://rs.tdwg.org/dwc/terms/GeodeticDatum> a owl:ObjectProperty,
        meta:SlotDefinition ;
    rdfs:label "GeodeticDatum" ;
    rdfs:range <https://w3id.org/biolink/biolinkml/meta/types/String> ;
    skos:definition "The geodetic datum to which the latitude and longitude refer. If not known, use \"not recorded\". This concept should be vocabulary-controlled. Example: \"WGS84\"" .

<http://rs.tdwg.org/dwc/terms/Geodetic_Datum> a owl:ObjectProperty,
        meta:SlotDefinition ;
    rdfs:label "Geodetic Datum" ;
    rdfs:range <https://w3id.org/biolink/biolinkml/meta/types/String> ;
    skos:definition "The ellipsoid, geodetic datum, or spatial reference system (SRS) upon which the geographic coordinates given in decimalLatitude and decimalLongitude as based. Recommended best practice is use the EPSG code as a controlled vocabulary to provide an SRS, if known. Otherwise use a controlled vocabulary for the name or code of the geodetic datum, if known. Otherwise use a controlled vocabulary for the name or code of the ellipsoid, if known. If none of these is known, use the value \"unknown\"." .

<http://rs.tdwg.org/dwc/terms/GeologicalContext> a owl:Class,
        meta:ClassDefinition ;
    rdfs:label "Geological Context",
        "GeologicalContext" ;
    rdfs:subClassOf [ a owl:Restriction ;
            owl:maxQualifiedCardinality 1 ;
            owl:onClass <https://w3id.org/biolink/biolinkml/meta/types/String> ;
            owl:onProperty <http://rs.tdwg.org/dwc/terms/formation> ],
        [ a owl:Restriction ;
            owl:maxQualifiedCardinality 1 ;
            owl:onClass <https://w3id.org/biolink/biolinkml/meta/types/String> ;
            owl:onProperty <http://rs.tdwg.org/dwc/terms/lithostratigraphicTerms> ],
        [ a owl:Restriction ;
            owl:maxQualifiedCardinality 1 ;
            owl:onClass <https://w3id.org/biolink/biolinkml/meta/types/String> ;
            owl:onProperty <http://rs.tdwg.org/dwc/terms/latestPeriodOrHighestSystem> ],
        [ a owl:Restriction ;
            owl:maxQualifiedCardinality 1 ;
            owl:onClass <https://w3id.org/biolink/biolinkml/meta/types/String> ;
            owl:onProperty <http://rs.tdwg.org/dwc/terms/Latest_AgeOr_Highest_Stage> ],
        [ a owl:Restriction ;
            owl:maxQualifiedCardinality 1 ;
            owl:onClass <https://w3id.org/biolink/biolinkml/meta/types/String> ;
            owl:onProperty <http://rs.tdwg.org/dwc/terms/Latest_Era_Or_Highest_Erathem> ],
        [ a owl:Restriction ;
            owl:maxQualifiedCardinality 1 ;
            owl:onClass <https://w3id.org/biolink/biolinkml/meta/types/String> ;
            owl:onProperty <http://rs.tdwg.org/dwc/terms/geologicalContextID> ],
        [ a owl:Restriction ;
            owl:maxQualifiedCardinality 1 ;
            owl:onClass <https://w3id.org/biolink/biolinkml/meta/types/String> ;
            owl:onProperty <http://rs.tdwg.org/dwc/terms/Latest_Period_Or_Highest_System> ],
        [ a owl:Restriction ;
            owl:maxQualifiedCardinality 1 ;
            owl:onClass <https://w3id.org/biolink/biolinkml/meta/types/String> ;
            owl:onProperty <http://rs.tdwg.org/dwc/terms/latestAgeOrHighestStage> ],
        [ a owl:Restriction ;
            owl:maxQualifiedCardinality 1 ;
            owl:onClass <https://w3id.org/biolink/biolinkml/meta/types/String> ;
            owl:onProperty <http://rs.tdwg.org/dwc/terms/Lowest_Biostratigraphic_Zone> ],
        [ a owl:Restriction ;
            owl:maxQualifiedCardinality 1 ;
            owl:onClass <https://w3id.org/biolink/biolinkml/meta/types/String> ;
            owl:onProperty <http://rs.tdwg.org/dwc/terms/Formation> ],
        [ a owl:Restriction ;
            owl:maxQualifiedCardinality 1 ;
            owl:onClass <https://w3id.org/biolink/biolinkml/meta/types/String> ;
            owl:onProperty <http://rs.tdwg.org/dwc/terms/lowestBiostratigraphicZone> ],
        [ a owl:Restriction ;
            owl:maxQualifiedCardinality 1 ;
            owl:onClass <https://w3id.org/biolink/biolinkml/meta/types/String> ;
            owl:onProperty <http://rs.tdwg.org/dwc/terms/group> ],
        [ a owl:Restriction ;
            owl:maxQualifiedCardinality 1 ;
            owl:onClass <https://w3id.org/biolink/biolinkml/meta/types/String> ;
            owl:onProperty <http://rs.tdwg.org/dwc/terms/earliestPeriodOrLowestSystem> ],
        [ a owl:Restriction ;
            owl:maxQualifiedCardinality 1 ;
            owl:onClass <https://w3id.org/biolink/biolinkml/meta/types/String> ;
            owl:onProperty <http://rs.tdwg.org/dwc/terms/earliestEpochOrLowestSeries> ],
        [ a owl:Restriction ;
            owl:maxQualifiedCardinality 1 ;
            owl:onClass <https://w3id.org/biolink/biolinkml/meta/types/String> ;
            owl:onProperty <http://rs.tdwg.org/dwc/terms/earliestEonOrLowestEonothem> ],
        [ a owl:Restriction ;
            owl:maxQualifiedCardinality 1 ;
            owl:onClass <https://w3id.org/biolink/biolinkml/meta/types/String> ;
            owl:onProperty <http://rs.tdwg.org/dwc/terms/latestEpochOrHighestSeries> ],
        [ a owl:Restriction ;
            owl:maxQualifiedCardinality 1 ;
            owl:onClass <https://w3id.org/biolink/biolinkml/meta/types/String> ;
            owl:onProperty <http://rs.tdwg.org/dwc/terms/earliestAgeOrLowestStage> ],
        [ a owl:Restriction ;
            owl:maxQualifiedCardinality 1 ;
            owl:onClass <https://w3id.org/biolink/biolinkml/meta/types/String> ;
            owl:onProperty <http://rs.tdwg.org/dwc/terms/Latest_Epoch_Or_Highest_Series> ],
        [ a owl:Restriction ;
            owl:maxQualifiedCardinality 1 ;
            owl:onClass <https://w3id.org/biolink/biolinkml/meta/types/String> ;
            owl:onProperty <http://rs.tdwg.org/dwc/terms/Earliest_Eon_Or_Lowest_Eonothem> ],
        [ a owl:Restriction ;
            owl:maxQualifiedCardinality 1 ;
            owl:onClass <https://w3id.org/biolink/biolinkml/meta/types/String> ;
            owl:onProperty <http://rs.tdwg.org/dwc/terms/highestBiostratigraphicZone> ],
        [ a owl:Restriction ;
            owl:maxQualifiedCardinality 1 ;
            owl:onClass <https://w3id.org/biolink/biolinkml/meta/types/String> ;
            owl:onProperty <http://rs.tdwg.org/dwc/terms/Earliest_Epoch_Or_Lowest_Series> ],
        [ a owl:Restriction ;
            owl:maxQualifiedCardinality 1 ;
            owl:onClass <https://w3id.org/biolink/biolinkml/meta/types/String> ;
            owl:onProperty <http://rs.tdwg.org/dwc/terms/Latest_Eon_Or_Highest_Eonothem> ],
        [ a owl:Restriction ;
            owl:maxQualifiedCardinality 1 ;
            owl:onClass <https://w3id.org/biolink/biolinkml/meta/types/String> ;
            owl:onProperty <http://rs.tdwg.org/dwc/terms/Earliest_Period_Or_Lowest_System> ],
        [ a owl:Restriction ;
            owl:maxQualifiedCardinality 1 ;
            owl:onClass <https://w3id.org/biolink/biolinkml/meta/types/String> ;
            owl:onProperty <http://rs.tdwg.org/dwc/terms/latestEonOrHighestEonothem> ],
        [ a owl:Restriction ;
            owl:maxQualifiedCardinality 1 ;
            owl:onClass <https://w3id.org/biolink/biolinkml/meta/types/String> ;
            owl:onProperty <http://rs.tdwg.org/dwc/terms/earliestEraOrLowestErathem> ],
        [ a owl:Restriction ;
            owl:maxQualifiedCardinality 1 ;
            owl:onClass <https://w3id.org/biolink/biolinkml/meta/types/String> ;
            owl:onProperty <http://rs.tdwg.org/dwc/terms/Bed> ],
        [ a owl:Restriction ;
            owl:maxQualifiedCardinality 1 ;
            owl:onClass <https://w3id.org/biolink/biolinkml/meta/types/String> ;
            owl:onProperty <http://rs.tdwg.org/dwc/terms/Geological_Context_ID> ],
        [ a owl:Restriction ;
            owl:maxQualifiedCardinality 1 ;
            owl:onClass <https://w3id.org/biolink/biolinkml/meta/types/String> ;
            owl:onProperty <http://rs.tdwg.org/dwc/terms/Group> ],
        [ a owl:Restriction ;
            owl:maxQualifiedCardinality 1 ;
            owl:onClass <https://w3id.org/biolink/biolinkml/meta/types/String> ;
            owl:onProperty <http://rs.tdwg.org/dwc/terms/Lithostratigraphic_Terms> ],
        [ a owl:Restriction ;
            owl:maxQualifiedCardinality 1 ;
            owl:onClass <https://w3id.org/biolink/biolinkml/meta/types/String> ;
            owl:onProperty <http://rs.tdwg.org/dwc/terms/Earliest_Age_Or_Lowest_Stage> ],
        [ a owl:Restriction ;
            owl:maxQualifiedCardinality 1 ;
            owl:onClass <https://w3id.org/biolink/biolinkml/meta/types/String> ;
            owl:onProperty <http://rs.tdwg.org/dwc/terms/latestEraOrHighestErathem> ],
        [ a owl:Restriction ;
            owl:maxQualifiedCardinality 1 ;
            owl:onClass <https://w3id.org/biolink/biolinkml/meta/types/String> ;
            owl:onProperty <http://rs.tdwg.org/dwc/terms/Member> ],
        [ a owl:Restriction ;
            owl:maxQualifiedCardinality 1 ;
            owl:onClass <https://w3id.org/biolink/biolinkml/meta/types/String> ;
            owl:onProperty <http://rs.tdwg.org/dwc/terms/member> ],
        [ a owl:Restriction ;
            owl:maxQualifiedCardinality 1 ;
            owl:onClass <https://w3id.org/biolink/biolinkml/meta/types/String> ;
            owl:onProperty <http://rs.tdwg.org/dwc/terms/Highest_Biostratigraphic_Zone> ],
        [ a owl:Restriction ;
            owl:maxQualifiedCardinality 1 ;
            owl:onClass <https://w3id.org/biolink/biolinkml/meta/types/String> ;
            owl:onProperty <http://rs.tdwg.org/dwc/terms/bed> ],
        [ a owl:Restriction ;
            owl:maxQualifiedCardinality 1 ;
            owl:onClass <https://w3id.org/biolink/biolinkml/meta/types/String> ;
            owl:onProperty <http://rs.tdwg.org/dwc/terms/Earliest_Era_Or_Lowest_Erathem> ] ;
    skos:altLabel "Geological Context",
        "GeologicalContext" ;
    skos:definition "Geological information, such as stratigraphy, that qualifies a region or place." ;
    skos:exactMatch <http://rs.tdwg.org/dwc/terms/version/GeologicalContext-2009-07-06>,
        <http://rs.tdwg.org/dwc/terms/version/GeologicalContext-2014-10-23> .

<http://rs.tdwg.org/dwc/terms/GeorefMethod> a owl:ObjectProperty,
        meta:SlotDefinition ;
    rdfs:label "GeorefMethod" ;
    rdfs:range <https://w3id.org/biolink/biolinkml/meta/types/String> ;
    skos:definition "A reference to the methods used for determining the coordinates and uncertainties." .

<http://rs.tdwg.org/dwc/terms/GeoreferenceProtocol> a owl:ObjectProperty,
        meta:SlotDefinition ;
    rdfs:label "GeoreferenceProtocol" ;
    rdfs:range <https://w3id.org/biolink/biolinkml/meta/types/String> ;
    skos:definition "A reference to the methods used for determining the coordinates and uncertainties. Example: \"http://manisnet.org/GeorefGuide.html\"." .

<http://rs.tdwg.org/dwc/terms/GeoreferenceRemarks> a owl:ObjectProperty,
        meta:SlotDefinition ;
    rdfs:label "GeoreferenceRemarks" ;
    rdfs:range <https://w3id.org/biolink/biolinkml/meta/types/String> ;
    skos:definition "Comments about the spatial description determination, explaining assumptions made in addition or opposition to the those formalized in the method referred to in GeoreferenceProtocol." .

<http://rs.tdwg.org/dwc/terms/GeoreferenceSources> a owl:ObjectProperty,
        meta:SlotDefinition ;
    rdfs:label "GeoreferenceSources" ;
    rdfs:range <https://w3id.org/biolink/biolinkml/meta/types/String> ;
    skos:definition "A list of maps, gazetteers or other resources used to georeference the locality. The content of this concept is meant to be specific enough to allow anyone in the future to use the same resource to georeference the same locality. Examples: \"USGS 1:24000 Florence Montana Quad\", \"Terrametrics 2008 on Google Earth\"" .

<http://rs.tdwg.org/dwc/terms/GeoreferenceVerificationStatus> a owl:ObjectProperty,
        meta:SlotDefinition ;
    rdfs:label "GeoreferenceVerificationStatus" ;
    rdfs:range <https://w3id.org/biolink/biolinkml/meta/types/String> ;
    skos:definition "A categorical description of the extent to which the georeference has been verified to represent the location where the specimen or observation was collected. This element should be vocabulary-controlled. Examples: \"requires verification\", \"verified by collector\", \"verified by curator\"." .

<http://rs.tdwg.org/dwc/terms/Georeference_Protocol> a owl:ObjectProperty,
        meta:SlotDefinition ;
    rdfs:label "Georeference Protocol" ;
    rdfs:range <https://w3id.org/biolink/biolinkml/meta/types/String> ;
    skos:definition "A description or reference to the methods used to determine the spatial footprint, coordinates, and uncertainties." .

<http://rs.tdwg.org/dwc/terms/Georeference_Remarks> a owl:ObjectProperty,
        meta:SlotDefinition ;
    rdfs:label "Georeference Remarks" ;
    rdfs:range <https://w3id.org/biolink/biolinkml/meta/types/String> ;
    skos:definition "Notes or comments about the spatial description determination, explaining assumptions made in addition or opposition to the those formalized in the method referred to in georeferenceProtocol." .

<http://rs.tdwg.org/dwc/terms/Georeference_Sources> a owl:ObjectProperty,
        meta:SlotDefinition ;
    rdfs:label "Georeference Sources" ;
    rdfs:range <https://w3id.org/biolink/biolinkml/meta/types/String> ;
    skos:definition "A list (concatenated and separated) of maps, gazetteers, or other resources used to georeference the Location, described specifically enough to allow anyone in the future to use the same resources." .

<http://rs.tdwg.org/dwc/terms/Georeference_Verification_Status> a owl:ObjectProperty,
        meta:SlotDefinition ;
    rdfs:label "Georeference Verification Status" ;
    rdfs:range <https://w3id.org/biolink/biolinkml/meta/types/String> ;
    skos:definition "A categorical description of the extent to which the georeference has been verified to represent the best possible spatial description. Recommended best practice is to use a controlled vocabulary." .

<http://rs.tdwg.org/dwc/terms/Georeferenced_By> a owl:ObjectProperty,
        meta:SlotDefinition ;
    rdfs:label "Georeferenced By" ;
    rdfs:range <https://w3id.org/biolink/biolinkml/meta/types/String> ;
    skos:definition "A list (concatenated and separated) of names of people, groups, or organizations who determined the georeference (spatial representation) for the Location." .

<http://rs.tdwg.org/dwc/terms/Georeferenced_Date> a owl:ObjectProperty,
        meta:SlotDefinition ;
    rdfs:label "Georeferenced Date" ;
    rdfs:range <https://w3id.org/biolink/biolinkml/meta/types/String> ;
    skos:definition "The date on which the Location was georeferenced. Recommended best practice is to use an encoding scheme, such as ISO 8601:2004(E)." .

<http://rs.tdwg.org/dwc/terms/GlobalUniqueIdentifier> a owl:ObjectProperty,
        meta:SlotDefinition ;
    rdfs:label "GlobalUniqueIdentifier" ;
    rdfs:range <https://w3id.org/biolink/biolinkml/meta/types/String> ;
    skos:definition "A Uniform Resource Name (URN) as a unique identifier for the specimen or observation record. In the absence of a persistent global unique identifier, construct one in the form: \"[InstitutionCode]:[CollectionCode]: [CatalogNumber]\" Examples: 1) urn:lsid:nhm.ku.edu:Herps:32 2) \"FMNH:Mammal:145732\"" .

<http://rs.tdwg.org/dwc/terms/HigherGeography> a owl:ObjectProperty,
        meta:SlotDefinition ;
    rdfs:label "HigherGeography" ;
    rdfs:range <https://w3id.org/biolink/biolinkml/meta/types/String> ;
    skos:definition "The names (concatenated and separated) of geographic elements less specific than the information in the Locality element. \"LIKE\" or \"contains\" substring query operations are meant to be used with this element to find matching geographic names. This can be useful if it is unclear in which element a name might be found, and in cases where there is no other appropriate geographic element. Example: \"South America, Argentina, Patagonia, Parque Nacional Nahuel Huapi, Neuqun, Los Lagos\" with accompanying values \"South America\" in Continent, \"Argentina\" in Country, \"Neuqun\" in StateProvince, and Los Lagos in County." .

<http://rs.tdwg.org/dwc/terms/HigherTaxon> a owl:ObjectProperty,
        meta:SlotDefinition ;
    rdfs:label "HigherTaxon" ;
    rdfs:range <https://w3id.org/biolink/biolinkml/meta/types/String> ;
    skos:definition "The names of taxonomic ranks less specific than SpecificEpithet concatenated and separated. \"LIKE\" or \"contains\" substring query operations are meant to be used with this element to find matching higher taxon names. This element may contain the list of scientific names of all of the supra-specific taxa in the classification used to identify (determine) the specimen or observation. Example: \"Animalia, Chordata, Vertebrata, Mammalia, Theria, Eutheria, Rodentia, Hystricognatha, Hystricognathi, Ctenomyidae, Ctenomyini, Ctenomys\"." .

<http://rs.tdwg.org/dwc/terms/Higher_Geography> a owl:ObjectProperty,
        meta:SlotDefinition ;
    rdfs:label "Higher Geography" ;
    rdfs:range <https://w3id.org/biolink/biolinkml/meta/types/String> ;
    skos:definition "A list (concatenated and separated) of geographic names less specific than the information captured in the locality term." .

<http://rs.tdwg.org/dwc/terms/Higher_Geography_ID> a owl:ObjectProperty,
        meta:SlotDefinition ;
    rdfs:label "Higher Geography ID" ;
    rdfs:range <https://w3id.org/biolink/biolinkml/meta/types/String> ;
    skos:definition "An identifier for the geographic region within which the Location occurred. Recommended best practice is to use an persistent identifier from a controlled vocabulary such as the Getty Thesaurus of Geographic Names." .

<http://rs.tdwg.org/dwc/terms/Higher_Taxon> a owl:ObjectProperty,
        meta:SlotDefinition ;
    rdfs:label "Higher Taxon" ;
    rdfs:range <https://w3id.org/biolink/biolinkml/meta/types/String> ;
    skos:definition "A list (concatenated and separated) of the names for the taxonomic ranks less specific than the ScientificName." .

<http://rs.tdwg.org/dwc/terms/Higher_Taxon_Concept_ID> a owl:ObjectProperty,
        meta:SlotDefinition ;
    rdfs:label "Higher Taxon Concept ID" ;
    rdfs:range <https://w3id.org/biolink/biolinkml/meta/types/String> ;
    skos:definition "A unique identifier for the taxon concept less specific than that given in the taxonConceptID." .

<http://rs.tdwg.org/dwc/terms/Higher_Taxon_ID> a owl:ObjectProperty,
        meta:SlotDefinition ;
    rdfs:label "Higher Taxon ID" ;
    rdfs:range <https://w3id.org/biolink/biolinkml/meta/types/String> ;
    skos:definition "A global unique identifier for the parent to the taxon." .

<http://rs.tdwg.org/dwc/terms/Higher_Taxon_Name> a owl:ObjectProperty,
        meta:SlotDefinition ;
    rdfs:label "Higher Taxon Name" ;
    rdfs:range <https://w3id.org/biolink/biolinkml/meta/types/String> ;
    skos:definition "A list (concatenated and separated) of the names for the taxonomic ranks less specific than that given in the scientificName." .

<http://rs.tdwg.org/dwc/terms/Higher_Taxon_Name_ID> a owl:ObjectProperty,
        meta:SlotDefinition ;
    rdfs:label "Higher Taxon Name ID" ;
    rdfs:range <https://w3id.org/biolink/biolinkml/meta/types/String> ;
    skos:definition "A unique identifier for the name of the next higher rank than the scientificName in a taxonomic classification. See higherTaxonName." .

<http://rs.tdwg.org/dwc/terms/HighestBiostratigraphicZone> a owl:ObjectProperty,
        meta:SlotDefinition ;
    rdfs:label "HighestBiostratigraphicZone" ;
    rdfs:range <https://w3id.org/biolink/biolinkml/meta/types/String> ;
    skos:definition "The full name of the highest possible geological biostratigraphic zone of the stratigraphic horizon from which the cataloged item was collected." .

<http://rs.tdwg.org/dwc/terms/HorizontalDatum> a owl:ObjectProperty,
        meta:SlotDefinition ;
    rdfs:label "HorizontalDatum" ;
    rdfs:range <https://w3id.org/biolink/biolinkml/meta/types/String> ;
    skos:definition "The horizontal geodetic datum to which the DecimalLatitude and DecimalLongitude refer." .

<http://rs.tdwg.org/dwc/terms/HumanObservation> a owl:Class,
        meta:ClassDefinition ;
    rdfs:label "Human Observation",
        "HumanObservation" ;
    skos:altLabel "Human Observation",
        "HumanObservation" ;
    skos:definition "An output of a human observation process." ;
    skos:exactMatch <http://rs.tdwg.org/dwc/dwctype/version/HumanObservation-2011-10-16>,
        <http://rs.tdwg.org/dwc/dwctype/version/HumanObservation-2014-10-23> .

<http://rs.tdwg.org/dwc/terms/Identification> a owl:Class,
        meta:ClassDefinition ;
    rdfs:label "Identification" ;
    rdfs:subClassOf [ a owl:Restriction ;
            owl:maxQualifiedCardinality 1 ;
            owl:onClass <https://w3id.org/biolink/biolinkml/meta/types/String> ;
            owl:onProperty <http://rs.tdwg.org/dwc/terms/typeStatus> ],
        [ a owl:Restriction ;
            owl:maxQualifiedCardinality 1 ;
            owl:onClass <https://w3id.org/biolink/biolinkml/meta/types/String> ;
            owl:onProperty <http://rs.tdwg.org/dwc/terms/identificationRemarks> ],
        [ a owl:Restriction ;
            owl:maxQualifiedCardinality 1 ;
            owl:onClass <https://w3id.org/biolink/biolinkml/meta/types/String> ;
            owl:onProperty <http://rs.tdwg.org/dwc/terms/Identification_Verification_Status> ],
        [ a owl:Restriction ;
            owl:maxQualifiedCardinality 1 ;
            owl:onClass <https://w3id.org/biolink/biolinkml/meta/types/String> ;
            owl:onProperty <http://rs.tdwg.org/dwc/terms/identificationID> ],
        [ a owl:Restriction ;
            owl:maxQualifiedCardinality 1 ;
            owl:onClass <https://w3id.org/biolink/biolinkml/meta/types/String> ;
            owl:onProperty <http://rs.tdwg.org/dwc/terms/identificationQualifier> ],
        [ a owl:Restriction ;
            owl:maxQualifiedCardinality 1 ;
            owl:onClass <https://w3id.org/biolink/biolinkml/meta/types/String> ;
            owl:onProperty <http://rs.tdwg.org/dwc/terms/Type_Status> ],
        [ a owl:Restriction ;
            owl:maxQualifiedCardinality 1 ;
            owl:onClass <https://w3id.org/biolink/biolinkml/meta/types/String> ;
            owl:onProperty <http://rs.tdwg.org/dwc/terms/identificationReferences> ],
        [ a owl:Restriction ;
            owl:maxQualifiedCardinality 1 ;
            owl:onClass <https://w3id.org/biolink/biolinkml/meta/types/String> ;
            owl:onProperty <http://rs.tdwg.org/dwc/terms/identifiedBy> ],
        [ a owl:Restriction ;
            owl:maxQualifiedCardinality 1 ;
            owl:onClass <https://w3id.org/biolink/biolinkml/meta/types/String> ;
            owl:onProperty <http://rs.tdwg.org/dwc/terms/identificationVerificationStatus> ],
        [ a owl:Restriction ;
            owl:maxQualifiedCardinality 1 ;
            owl:onClass <https://w3id.org/biolink/biolinkml/meta/types/String> ;
            owl:onProperty <http://rs.tdwg.org/dwc/terms/dateIdentified> ],
        [ a owl:Restriction ;
            owl:maxQualifiedCardinality 1 ;
            owl:onClass <https://w3id.org/biolink/biolinkml/meta/types/String> ;
            owl:onProperty <http://rs.tdwg.org/dwc/terms/Identification_References> ],
        [ a owl:Restriction ;
            owl:maxQualifiedCardinality 1 ;
            owl:onClass <https://w3id.org/biolink/biolinkml/meta/types/String> ;
            owl:onProperty <http://rs.tdwg.org/dwc/terms/Date_Identified> ],
        [ a owl:Restriction ;
            owl:maxQualifiedCardinality 1 ;
            owl:onClass <https://w3id.org/biolink/biolinkml/meta/types/String> ;
            owl:onProperty <http://rs.tdwg.org/dwc/terms/Identification_Qualifier> ],
        [ a owl:Restriction ;
            owl:maxQualifiedCardinality 1 ;
            owl:onClass <https://w3id.org/biolink/biolinkml/meta/types/String> ;
            owl:onProperty <http://rs.tdwg.org/dwc/terms/Identification_Remarks> ],
        [ a owl:Restriction ;
            owl:maxQualifiedCardinality 1 ;
            owl:onClass <https://w3id.org/biolink/biolinkml/meta/types/String> ;
            owl:onProperty <http://rs.tdwg.org/dwc/terms/Identification_ID> ],
        [ a owl:Restriction ;
            owl:maxQualifiedCardinality 1 ;
            owl:onClass <https://w3id.org/biolink/biolinkml/meta/types/String> ;
            owl:onProperty <http://rs.tdwg.org/dwc/terms/Identified_By> ] ;
    skos:altLabel "Identification" ;
    skos:definition "A taxonomic determination (e.g., the assignment to a taxon)." ;
    skos:exactMatch <http://rs.tdwg.org/dwc/terms/version/Identification-2008-11-19> .

<http://rs.tdwg.org/dwc/terms/IdentificationModifier> a owl:ObjectProperty,
        meta:SlotDefinition ;
    rdfs:label "IdentificationModifier" ;
    rdfs:range <https://w3id.org/biolink/biolinkml/meta/types/String> ;
    skos:definition "Additional information documenting the taxonomic determination of the cataloged item (e.g., \"cf.\", \"aff.\", \"subspecies in question\", etc.)." .

<http://rs.tdwg.org/dwc/terms/IdentificationQualifier> a owl:ObjectProperty,
        meta:SlotDefinition ;
    rdfs:label "IdentificationQualifier" ;
    rdfs:range <https://w3id.org/biolink/biolinkml/meta/types/String> ;
    skos:definition "A brief phrase or a standard term (\"cf.\", \"aff.\") to qualify the identification of the organism when doubts have arisen as to its taxonomic identity (determination). Examples: 1) For the determination \"Quercus aff. agrifolia var. oxyadenia\", IdentificationQualifier would be \"aff. agrifolia var. oxyadenia\" with accompanying values \"Quercus\" in Genus, \"agrifolia\" in SpecificEpithet, \"oxyadenia\" in InfraspecificEpithet, and \"var.\" in InfraspecificRank. 2) For the determination \"Quercus agrifolia cf. var. oxyadenia\", IdentificationQualifier would be \"cf. var. oxyadenia \" with accompanying values \"Quercus\" in Genus, \"agrifolia\" in SpecificEpithet, \"oxyadenia\" in InfraspecificEpithet, and \"var.\" in InfraspecificRank." .

<http://rs.tdwg.org/dwc/terms/Identification_Attributes> a owl:ObjectProperty,
        meta:SlotDefinition ;
    rdfs:label "Identification Attributes" ;
    rdfs:range <https://w3id.org/biolink/biolinkml/meta/types/String> ;
    skos:definition "A list (concatenated and separated) of additional measurements, facts, characteristics, or assertions about the Identification." .

<http://rs.tdwg.org/dwc/terms/IdentifiedBy> a owl:ObjectProperty,
        meta:SlotDefinition ;
    rdfs:label "IdentifiedBy" ;
    rdfs:range <https://w3id.org/biolink/biolinkml/meta/types/String> ;
    skos:definition "The name(s) of the person(s) who applied the currently accepted ScientificName to the cataloged item." .

<http://rs.tdwg.org/dwc/terms/ImageURL> a owl:ObjectProperty,
        meta:SlotDefinition ;
    rdfs:label "ImageURL" ;
    rdfs:range <https://w3id.org/biolink/biolinkml/meta/types/String> ;
    skos:definition "A Universal Resource Locator reference to digital images associated with the specimen or observation." .

<http://rs.tdwg.org/dwc/terms/IndividualCount> a owl:ObjectProperty,
        meta:SlotDefinition ;
    rdfs:label "IndividualCount" ;
    rdfs:range <https://w3id.org/biolink/biolinkml/meta/types/String> ;
    skos:definition "The number of individuals present in the lot or container referred to by the catalog number. Not an estimate of abundance or density at the collecting locality." .

<http://rs.tdwg.org/dwc/terms/Individual_ID> a owl:ObjectProperty,
        meta:SlotDefinition ;
    rdfs:label "Individual ID" ;
    rdfs:range <https://w3id.org/biolink/biolinkml/meta/types/String> ;
    skos:definition "An identifier for an individual or named group of individual organisms represented in the Occurrence. Meant to accommodate resampling of the same individual or group for monitoring purposes. May be a global unique identifier or an identifier specific to a data set." .

<http://rs.tdwg.org/dwc/terms/InformationWithheld> a owl:ObjectProperty,
        meta:SlotDefinition ;
    rdfs:label "InformationWithheld" ;
    rdfs:range <https://w3id.org/biolink/biolinkml/meta/types/String> ;
    skos:definition "Brief descriptions of additional information that may exist, but that has not been made public. Information about obtaining the withheld information should be sought from the administrative contact identified in the provider resource metadata (curator, collection manager). Examples: \"specific locality information given only to nearest county\", \"ask about tissue samples\", \"georeferences given only to nearest degree\"." .

<http://rs.tdwg.org/dwc/terms/Information_Withheld> a owl:ObjectProperty,
        meta:SlotDefinition ;
    rdfs:label "Information Withheld" ;
    rdfs:range <https://w3id.org/biolink/biolinkml/meta/types/String> ;
    skos:definition "Additional information that exists, but that has not been shared in the given record." .

<http://rs.tdwg.org/dwc/terms/InfraspecificEpithet> a owl:ObjectProperty,
        meta:SlotDefinition ;
    rdfs:label "InfraspecificEpithet" ;
    rdfs:range <https://w3id.org/biolink/biolinkml/meta/types/String> ;
    skos:definition "The infraspecific epithet of the scientific name applied to the organism." .

<http://rs.tdwg.org/dwc/terms/InfraspecificRank> a owl:ObjectProperty,
        meta:SlotDefinition ;
    rdfs:label "InfraspecificRank" ;
    rdfs:range <https://w3id.org/biolink/biolinkml/meta/types/String> ;
    skos:definition "The infraspecific rank (subspecies, variety, forma) of the InfraspecificEpithet. Examples: \"subsp.\", \"var.\", \"forma\"." .

<http://rs.tdwg.org/dwc/terms/InstitutionCode> a owl:ObjectProperty,
        meta:SlotDefinition ;
    rdfs:label "InstitutionCode" ;
    rdfs:range <https://w3id.org/biolink/biolinkml/meta/types/String> ;
    skos:definition "The code (or acronym) identifying the institution administering the collection in which the organism record is cataloged. No global registry exists for institutional codes; use the code that is \"standard\" at your institution or in your discipline." .

<http://rs.tdwg.org/dwc/terms/Institution_Code> a owl:ObjectProperty,
        meta:SlotDefinition ;
    rdfs:label "Institution Code" ;
    rdfs:range <https://w3id.org/biolink/biolinkml/meta/types/String> ;
    skos:definition "The name (or acronym) in use by the institution having custody of the object(s) or information referred to in the record." .

<http://rs.tdwg.org/dwc/terms/Institution_ID> a owl:ObjectProperty,
        meta:SlotDefinition ;
    rdfs:label "Institution ID" ;
    rdfs:range <https://w3id.org/biolink/biolinkml/meta/types/String> ;
    skos:definition "An identifier for the institution having custody of the object(s) or information referred to in the record." .

<http://rs.tdwg.org/dwc/terms/Island> a owl:ObjectProperty,
        meta:SlotDefinition ;
    rdfs:label "Island" ;
    rdfs:range <https://w3id.org/biolink/biolinkml/meta/types/String> ;
    skos:definition "The full, unabbreviated name of the island on which the organism was collected or observed." .

<http://rs.tdwg.org/dwc/terms/IslandGroup> a owl:ObjectProperty,
        meta:SlotDefinition ;
    rdfs:label "IslandGroup" ;
    rdfs:range <https://w3id.org/biolink/biolinkml/meta/types/String> ;
    skos:definition "The full, unabbreviated name of the island group in which the organism was collected or observed." .

<http://rs.tdwg.org/dwc/terms/Island_Group> a owl:ObjectProperty,
        meta:SlotDefinition ;
    rdfs:label "Island Group" ;
    rdfs:range <https://w3id.org/biolink/biolinkml/meta/types/String> ;
    skos:definition "The name of the island group in which the Location occurs. Recommended best practice is to use a controlled vocabulary such as the Getty Thesaurus of Geographic Names." .

<http://rs.tdwg.org/dwc/terms/JulianDay> a owl:ObjectProperty,
        meta:SlotDefinition ;
    rdfs:label "JulianDay" ;
    rdfs:range <https://w3id.org/biolink/biolinkml/meta/types/String> ;
    skos:definition "The ordinal day of the year (i.e., the number of days since December 31 of the previous year; January 1 is Julian Day 1) on which the cataloged item was collected. May be derived from the YearCollected, MonthCollected, and DayCollected by the provider." .

<http://rs.tdwg.org/dwc/terms/LatLongComments> a owl:ObjectProperty,
        meta:SlotDefinition ;
    rdfs:label "LatLongComments" ;
    rdfs:range <https://w3id.org/biolink/biolinkml/meta/types/String> ;
    skos:definition "Comments about the LatLong determination." .

<http://rs.tdwg.org/dwc/terms/LatestAgeOrHighestStage> a owl:ObjectProperty,
        meta:SlotDefinition ;
    rdfs:label "LatestAgeOrHighestStage" ;
    rdfs:range <https://w3id.org/biolink/biolinkml/meta/types/String> ;
    skos:definition "The full name of the latest possible geochronologic age or highest chronostratigraphic stage attributable to the stratigraphic horizon from which the cataloged item was collected." .

<http://rs.tdwg.org/dwc/terms/LatestDateCollected> a owl:ObjectProperty,
        meta:SlotDefinition ;
    rdfs:label "LatestDateCollected" ;
    rdfs:range <https://w3id.org/biolink/biolinkml/meta/types/String> ;
    skos:definition "The latest date-time (Common Era calendar) in a date-time period during which an organism or group of organisms was collected or observed. If the event is recorded as occurring at a single date-time, populate both EarliestDateCollected and LatestDateCollected with the same value." .

<http://rs.tdwg.org/dwc/terms/LatestEonOrHighestEonothem> a owl:ObjectProperty,
        meta:SlotDefinition ;
    rdfs:label "LatestEonOrHighestEonothem" ;
    rdfs:range <https://w3id.org/biolink/biolinkml/meta/types/String> ;
    skos:definition "The full name of the latest possible geochronologic eon or highest chrono-stratigraphic eonothem or the informal name (\"Precambrian\") attributable to the stratigraphic horizon from which the cataloged item was collected." .

<http://rs.tdwg.org/dwc/terms/LatestEpochOrHighestSeries> a owl:ObjectProperty,
        meta:SlotDefinition ;
    rdfs:label "LatestEpochOrHighestSeries" ;
    rdfs:range <https://w3id.org/biolink/biolinkml/meta/types/String> ;
    skos:definition "The full name of the latest possible geochronologic epoch or highest chronostratigraphic series attributable to the stratigraphic horizon from which the cataloged item was collected." .

<http://rs.tdwg.org/dwc/terms/LatestEraOrHighestErathem> a owl:ObjectProperty,
        meta:SlotDefinition ;
    rdfs:label "LatestEraOrHighestErathem" ;
    rdfs:range <https://w3id.org/biolink/biolinkml/meta/types/String> ;
    skos:definition "The full name of the latest possible geochronologic era or highest chronostratigraphic erathem attributable to the stratigraphic horizon from which the cataloged item was collected." .

<http://rs.tdwg.org/dwc/terms/LatestPeriodOrHighestSystem> a owl:ObjectProperty,
        meta:SlotDefinition ;
    rdfs:label "LatestPeriodOrHighestSystem" ;
    rdfs:range <https://w3id.org/biolink/biolinkml/meta/types/String> ;
    skos:definition "The full name of the latest possible geochronologic period or highest chronostratigraphic system attributable to the stratigraphic horizon from which the cataloged item was collected." .

<http://rs.tdwg.org/dwc/terms/Latest_Date_Collected> a owl:ObjectProperty,
        meta:SlotDefinition ;
    rdfs:label "Latest Date Collected" ;
    rdfs:range <https://w3id.org/biolink/biolinkml/meta/types/String> ;
    skos:definition "The latest date-time in a period during which a event occurred. If the event is recorded as occurring at a single date-time, populate both EarliestDateCollected and LatestDateCollected with the same value. Recommended best practice is to use an encoding scheme, such as ISO 8601:2004(E)." .

<http://rs.tdwg.org/dwc/terms/Latitude> a owl:ObjectProperty,
        meta:SlotDefinition ;
    rdfs:label "Latitude" ;
    rdfs:range <https://w3id.org/biolink/biolinkml/meta/types/String> ;
    skos:definition "The latitude of the location from which the specimen was collected. This value should be expressed in decimal degrees with a datum such as WGS-84" .

<http://rs.tdwg.org/dwc/terms/LifeStage> a owl:ObjectProperty,
        meta:SlotDefinition ;
    rdfs:label "LifeStage" ;
    rdfs:range <https://w3id.org/biolink/biolinkml/meta/types/String> ;
    skos:definition "The age class or life stage of the biological individual represented by the catalogued object or observation. Examples: \"adult\", \"mature\", \"juvenile\", \"eft\", \"nymph\", \"seedling\", \"seed\", \"egg\"" .

<http://rs.tdwg.org/dwc/terms/LithostratigraphicTerms> a owl:ObjectProperty,
        meta:SlotDefinition ;
    rdfs:label "LithostratigraphicTerms" ;
    rdfs:range <https://w3id.org/biolink/biolinkml/meta/types/String> ;
    skos:definition "The combination of all litho-stratigraphic names for the rock from which the cataloged item was collected." .

<http://rs.tdwg.org/dwc/terms/LivingSpecimen> a owl:Class,
        meta:ClassDefinition ;
    rdfs:label "Living Specimen",
        "LivingSpecimen" ;
    skos:altLabel "Living Specimen",
        "LivingSpecimen" ;
    skos:definition "A specimen that is alive." ;
    skos:exactMatch <http://rs.tdwg.org/dwc/dwctype/version/LivingSpecimen-2011-10-16>,
        <http://rs.tdwg.org/dwc/dwctype/version/LivingSpecimen-2014-10-23> .

<http://rs.tdwg.org/dwc/terms/Locality> a owl:ObjectProperty,
        meta:SlotDefinition ;
    rdfs:label "Locality" ;
    rdfs:range <https://w3id.org/biolink/biolinkml/meta/types/String> ;
    skos:definition "The specific natural language description of the place where the organism was collected or observed. This element need not contain less specific geographic information provided in other geographic elements (HigherGeography, Continent, Country, StateProvince, County, WaterBody, Island, IslandGroup). Though coordinate information can be contained in this concept, these data will be usable analytically only when shared through the concepts of the Geospatial Extension." .

<http://rs.tdwg.org/dwc/terms/Location> a owl:Class,
        meta:ClassDefinition ;
    rdfs:label "Location" ;
    skos:altLabel "Location" ;
    skos:definition "A resource describing an instance of the Location class." .

<http://rs.tdwg.org/dwc/terms/Location_According_To> a owl:ObjectProperty,
        meta:SlotDefinition ;
    rdfs:label "Location According To" ;
    rdfs:range <https://w3id.org/biolink/biolinkml/meta/types/String> ;
    skos:definition "Information about the source of this Location information. Could be a publication (gazetteer), institution, or team of individuals." .

<http://rs.tdwg.org/dwc/terms/Location_Attributes> a owl:ObjectProperty,
        meta:SlotDefinition ;
    rdfs:label "Location Attributes" ;
    rdfs:range <https://w3id.org/biolink/biolinkml/meta/types/String> ;
    skos:definition "A list (concatenated and separated) of additional measurements, facts, characteristics, or assertions about the location." .

<http://rs.tdwg.org/dwc/terms/Location_ID> a owl:ObjectProperty,
        meta:SlotDefinition ;
    rdfs:label "Location ID" ;
    rdfs:range <https://w3id.org/biolink/biolinkml/meta/types/String> ;
    skos:definition "An identifier for the set of location information (data associated with dcterms:Location). May be a global unique identifier or an identifier specific to the data set." .

<http://rs.tdwg.org/dwc/terms/Location_Remarks> a owl:ObjectProperty,
        meta:SlotDefinition ;
    rdfs:label "Location Remarks" ;
    rdfs:range <https://w3id.org/biolink/biolinkml/meta/types/String> ;
    skos:definition "Comments or notes about the Location." .

<http://rs.tdwg.org/dwc/terms/Longitude> a owl:ObjectProperty,
        meta:SlotDefinition ;
    rdfs:label "Longitude" ;
    rdfs:range <https://w3id.org/biolink/biolinkml/meta/types/String> ;
    skos:definition "The longitude of the location from which the specimen was collected. This value should be expressed in decimal degrees with a datum such as WGS-84" .

<http://rs.tdwg.org/dwc/terms/LowestBiostratigraphicZone> a owl:ObjectProperty,
        meta:SlotDefinition ;
    rdfs:label "LowestBiostratigraphicZone" ;
    rdfs:range <https://w3id.org/biolink/biolinkml/meta/types/String> ;
    skos:definition "The full name of the lowest possible geological biostratigraphic zone of the stratigraphic horizon from which the cataloged item was collected." .

<http://rs.tdwg.org/dwc/terms/MachineObservation> a owl:Class,
        meta:ClassDefinition ;
    rdfs:label "Machine Observation",
        "MachineObservation" ;
    skos:altLabel "Machine Observation",
        "MachineObservation" ;
    skos:definition "An output of a machine observation process." ;
    skos:exactMatch <http://rs.tdwg.org/dwc/dwctype/version/MachineObservation-2011-10-16>,
        <http://rs.tdwg.org/dwc/dwctype/version/MachineObservation-2014-10-23> .

<http://rs.tdwg.org/dwc/terms/MaterialSample> a owl:Class,
        meta:ClassDefinition ;
    rdfs:label "Material Sample",
        "MaterialSample" ;
    rdfs:subClassOf [ a owl:Restriction ;
            owl:maxQualifiedCardinality 1 ;
            owl:onClass <https://w3id.org/biolink/biolinkml/meta/types/String> ;
            owl:onProperty <http://rs.tdwg.org/dwc/terms/Material_Sample_ID> ],
        [ a owl:Restriction ;
            owl:maxQualifiedCardinality 1 ;
            owl:onClass <https://w3id.org/biolink/biolinkml/meta/types/String> ;
            owl:onProperty <http://rs.tdwg.org/dwc/terms/materialSampleID> ] ;
    skos:altLabel "Material Sample",
        "MaterialSample" ;
    skos:definition "A physical result of a sampling (or subsampling) event. In biological collections, the material sample is typically collected, and either preserved or destructively processed.",
        "A physical results of a sampling (or subsampling) event. In biological collections, the material sample is typically collected, and either preserved or destructively processed." ;
    skos:exactMatch <http://rs.tdwg.org/dwc/terms/version/MaterialSample-2013-03-28>,
        <http://rs.tdwg.org/dwc/terms/version/MaterialSample-2014-10-23> .

<http://rs.tdwg.org/dwc/terms/MaximumDepth> a owl:ObjectProperty,
        meta:SlotDefinition ;
    rdfs:label "MaximumDepth" ;
    rdfs:range <https://w3id.org/biolink/biolinkml/meta/types/String> ;
    skos:definition "The maximum distance in meters below the surface of the water at which the collection was made; all material collected was at most this deep. Positive below the surface, negative above (e.g. collecting above sea level in tidal areas)." .

<http://rs.tdwg.org/dwc/terms/MaximumDepthInMeters> a owl:ObjectProperty,
        meta:SlotDefinition ;
    rdfs:label "MaximumDepthInMeters" ;
    rdfs:range <https://w3id.org/biolink/biolinkml/meta/types/String> ;
    skos:definition "The maximum or actual depth at which the collection or observation was made. Use positive values for locations below the surface. Examples: 10 (for a depth of up to 10m). 100 (for a depth between 50m and 100m)." .

<http://rs.tdwg.org/dwc/terms/MaximumElevation> a owl:ObjectProperty,
        meta:SlotDefinition ;
    rdfs:label "MaximumElevation" ;
    rdfs:range <https://w3id.org/biolink/biolinkml/meta/types/String> ;
    skos:definition "The maximum distance in meters above (positive) or below sea level of the collecting locality." .

<http://rs.tdwg.org/dwc/terms/MaximumElevationInMeters> a owl:ObjectProperty,
        meta:SlotDefinition ;
    rdfs:label "MaximumElevationInMeters" ;
    rdfs:range <https://w3id.org/biolink/biolinkml/meta/types/String> ;
    skos:definition "The maximum or actual elevation at which the collection or observation was made. Use negative values for locations below sea level. Examples: Examples: 125 (for an elevation of 100 +- 25 meters). 200 (for an elevation between 100m and 200m)." .

<http://rs.tdwg.org/dwc/terms/Maximum_Depth_In_Meters> a owl:ObjectProperty,
        meta:SlotDefinition ;
    rdfs:label "Maximum Depth In Meters" ;
    rdfs:range <https://w3id.org/biolink/biolinkml/meta/types/String> ;
    skos:definition "The greater depth of a range of depth below the local surface, in meters." .

<http://rs.tdwg.org/dwc/terms/Maximum_Distance_Above_Surface_In_Meters> a owl:ObjectProperty,
        meta:SlotDefinition ;
    rdfs:label "Maximum Distance Above Surface In Meters" ;
    rdfs:range <https://w3id.org/biolink/biolinkml/meta/types/String> ;
    skos:definition "The greater distance in a range of distance from a reference surface in the vertical direction, in meters. Use positive values for locations above the surface, negative values for locations below. If depth measures are given, the reference surface is the location given by the depth, otherwise the reference surface is the location given by the elevation." .

<http://rs.tdwg.org/dwc/terms/Maximum_Elevation_In_Meters> a owl:ObjectProperty,
        meta:SlotDefinition ;
    rdfs:label "Maximum Elevation In Meters" ;
    rdfs:range <https://w3id.org/biolink/biolinkml/meta/types/String> ;
    skos:definition "The upper limit of the range of elevation (altitude, usually above sea level), in meters." .

<http://rs.tdwg.org/dwc/terms/MeasurementOrFact> a owl:Class,
        meta:ClassDefinition ;
    rdfs:label "Measurement Or Fact",
        "Measurement or Fact",
        "MeasurementOrFact" ;
    rdfs:subClassOf [ a owl:Restriction ;
            owl:maxQualifiedCardinality 1 ;
            owl:onClass <https://w3id.org/biolink/biolinkml/meta/types/String> ;
            owl:onProperty <http://rs.tdwg.org/dwc/terms/measurementUnit> ],
        [ a owl:Restriction ;
            owl:maxQualifiedCardinality 1 ;
            owl:onClass <https://w3id.org/biolink/biolinkml/meta/types/String> ;
            owl:onProperty <http://rs.tdwg.org/dwc/terms/measurementDeterminedDate> ],
        [ a owl:Restriction ;
            owl:maxQualifiedCardinality 1 ;
            owl:onClass <https://w3id.org/biolink/biolinkml/meta/types/String> ;
            owl:onProperty <http://rs.tdwg.org/dwc/terms/measurementType> ],
        [ a owl:Restriction ;
            owl:maxQualifiedCardinality 1 ;
            owl:onClass <https://w3id.org/biolink/biolinkml/meta/types/String> ;
            owl:onProperty <http://rs.tdwg.org/dwc/terms/Measurement_Determined_Date> ],
        [ a owl:Restriction ;
            owl:maxQualifiedCardinality 1 ;
            owl:onClass <https://w3id.org/biolink/biolinkml/meta/types/String> ;
            owl:onProperty <http://rs.tdwg.org/dwc/terms/Measurement_ID> ],
        [ a owl:Restriction ;
            owl:maxQualifiedCardinality 1 ;
            owl:onClass <https://w3id.org/biolink/biolinkml/meta/types/String> ;
            owl:onProperty <http://rs.tdwg.org/dwc/terms/Measurement_Value> ],
        [ a owl:Restriction ;
            owl:maxQualifiedCardinality 1 ;
            owl:onClass <https://w3id.org/biolink/biolinkml/meta/types/String> ;
            owl:onProperty <http://rs.tdwg.org/dwc/terms/measurementAccuracy> ],
        [ a owl:Restriction ;
            owl:maxQualifiedCardinality 1 ;
            owl:onClass <https://w3id.org/biolink/biolinkml/meta/types/String> ;
            owl:onProperty <http://rs.tdwg.org/dwc/terms/Measurement_Unit> ],
        [ a owl:Restriction ;
            owl:maxQualifiedCardinality 1 ;
            owl:onClass <https://w3id.org/biolink/biolinkml/meta/types/String> ;
            owl:onProperty <http://rs.tdwg.org/dwc/terms/measurementID> ],
        [ a owl:Restriction ;
            owl:maxQualifiedCardinality 1 ;
            owl:onClass <https://w3id.org/biolink/biolinkml/meta/types/String> ;
            owl:onProperty <http://rs.tdwg.org/dwc/terms/measurementDeterminedBy> ],
        [ a owl:Restriction ;
            owl:maxQualifiedCardinality 1 ;
            owl:onClass <https://w3id.org/biolink/biolinkml/meta/types/String> ;
            owl:onProperty <http://rs.tdwg.org/dwc/terms/Measurement_Remarks> ],
        [ a owl:Restriction ;
            owl:maxQualifiedCardinality 1 ;
            owl:onClass <https://w3id.org/biolink/biolinkml/meta/types/String> ;
            owl:onProperty <http://rs.tdwg.org/dwc/terms/Measurement_Method> ],
        [ a owl:Restriction ;
            owl:maxQualifiedCardinality 1 ;
            owl:onClass <https://w3id.org/biolink/biolinkml/meta/types/String> ;
            owl:onProperty <http://rs.tdwg.org/dwc/terms/measurementRemarks> ],
        [ a owl:Restriction ;
            owl:maxQualifiedCardinality 1 ;
            owl:onClass <https://w3id.org/biolink/biolinkml/meta/types/String> ;
            owl:onProperty <http://rs.tdwg.org/dwc/terms/measurementValue> ],
        [ a owl:Restriction ;
            owl:maxQualifiedCardinality 1 ;
            owl:onClass <https://w3id.org/biolink/biolinkml/meta/types/String> ;
            owl:onProperty <http://rs.tdwg.org/dwc/terms/Measurement_Accuracy> ],
        [ a owl:Restriction ;
            owl:maxQualifiedCardinality 1 ;
            owl:onClass <https://w3id.org/biolink/biolinkml/meta/types/String> ;
            owl:onProperty <http://rs.tdwg.org/dwc/terms/Measurement_Determined_By> ],
        [ a owl:Restriction ;
            owl:maxQualifiedCardinality 1 ;
            owl:onClass <https://w3id.org/biolink/biolinkml/meta/types/String> ;
            owl:onProperty <http://rs.tdwg.org/dwc/terms/measurementMethod> ],
        [ a owl:Restriction ;
            owl:maxQualifiedCardinality 1 ;
            owl:onClass <https://w3id.org/biolink/biolinkml/meta/types/String> ;
            owl:onProperty <http://rs.tdwg.org/dwc/terms/Measurement_Type> ] ;
    skos:altLabel "Measurement Or Fact",
        "Measurement or Fact",
        "MeasurementOrFact" ;
    skos:definition "A measurement of or fact about an rdfs:Resource (http://www.w3.org/2000/01/rdf-schema#Resource).",
        "The category of information pertaining to measurements, facts, characteristics, or assertions about a resource (instance of data record, such as Occurrence, Taxon, Location, Event)." ;
    skos:exactMatch <http://rs.tdwg.org/dwc/terms/version/EventMeasurement-2008-11-19>,
        <http://rs.tdwg.org/dwc/terms/version/MeasurementOrFact-2009-04-24>,
        <http://rs.tdwg.org/dwc/terms/version/MeasurementOrFact-2014-10-23>,
        <http://rs.tdwg.org/dwc/terms/version/OccurrenceMeasurement-2008-11-19> .

<http://rs.tdwg.org/dwc/terms/MinimumDepth> a owl:ObjectProperty,
        meta:SlotDefinition ;
    rdfs:label "MinimumDepth" ;
    rdfs:range <https://w3id.org/biolink/biolinkml/meta/types/String> ;
    skos:definition "The minimum distance in meters below the surface of the water at which the collection was made; all material collected was at least this deep. Positive below the surface, negative above (e.g. collecting above sea level in tidal areas)." .

<http://rs.tdwg.org/dwc/terms/MinimumDepthInMeters> a owl:ObjectProperty,
        meta:SlotDefinition ;
    rdfs:label "MinimumDepthInMeters" ;
    rdfs:range <https://w3id.org/biolink/biolinkml/meta/types/String> ;
    skos:definition "The minimum or actual depth at which the collection or observation was made. Use positive values for locations below the surface. Examples: 0 (for a depth of up to 10m). 50 (for a depth between 50m and 100m)." .

<http://rs.tdwg.org/dwc/terms/MinimumElevation> a owl:ObjectProperty,
        meta:SlotDefinition ;
    rdfs:label "MinimumElevation" ;
    rdfs:range <https://w3id.org/biolink/biolinkml/meta/types/String> ;
    skos:definition "The minimum distance in meters above (positive) or below sea level of the collecting locality." .

<http://rs.tdwg.org/dwc/terms/MinimumElevationInMeters> a owl:ObjectProperty,
        meta:SlotDefinition ;
    rdfs:label "MinimumElevationInMeters" ;
    rdfs:range <https://w3id.org/biolink/biolinkml/meta/types/String> ;
    skos:definition "The minimum or actual elevation at which the collection or observation was made. Use negative values for locations below sea level. Examples: 75 (for an elevation of 100 +- 25 meters). 100 (for an elevation between 100m and 200m)." .

<http://rs.tdwg.org/dwc/terms/Minimum_Depth_In_Meters> a owl:ObjectProperty,
        meta:SlotDefinition ;
    rdfs:label "Minimum Depth In Meters" ;
    rdfs:range <https://w3id.org/biolink/biolinkml/meta/types/String> ;
    skos:definition "The lesser depth of a range of depth below the local surface, in meters." .

<http://rs.tdwg.org/dwc/terms/Minimum_Distance_Above_Surface_In_Meters> a owl:ObjectProperty,
        meta:SlotDefinition ;
    rdfs:label "Minimum Distance Above Surface In Meters" ;
    rdfs:range <https://w3id.org/biolink/biolinkml/meta/types/String> ;
    skos:definition "The lesser distance in a range of distance from a reference surface in the vertical direction, in meters. Use positive values for locations above the surface, negative values for locations below. If depth measures are given, the reference surface is the location given by the depth, otherwise the reference surface is the location given by the elevation." .

<http://rs.tdwg.org/dwc/terms/Minimum_Elevation_In_Meters> a owl:ObjectProperty,
        meta:SlotDefinition ;
    rdfs:label "Minimum Elevation In Meters" ;
    rdfs:range <https://w3id.org/biolink/biolinkml/meta/types/String> ;
    skos:definition "The lower limit of the range of elevation (altitude, usually above sea level), in meters." .

<http://rs.tdwg.org/dwc/terms/MonthCollected> a owl:ObjectProperty,
        meta:SlotDefinition ;
    rdfs:label "MonthCollected" ;
    rdfs:range <https://w3id.org/biolink/biolinkml/meta/types/String> ;
    skos:definition "The two digit month of year in the Common Era calendar during which the cataloged item was collected from the field." .

<http://rs.tdwg.org/dwc/terms/MonthIdentified> a owl:ObjectProperty,
        meta:SlotDefinition ;
    rdfs:label "MonthIdentified" ;
    rdfs:range <https://w3id.org/biolink/biolinkml/meta/types/String> ;
    skos:definition "The two digit month in the Common Era calendar during which the cataloged item was identified." .

<http://rs.tdwg.org/dwc/terms/Municipality> a owl:ObjectProperty,
        meta:SlotDefinition ;
    rdfs:label "Municipality" ;
    rdfs:range <https://w3id.org/biolink/biolinkml/meta/types/String> ;
    skos:definition "The full, unabbreviated name of the next smaller administrative region than county (city, municipality, etc.) in which the Location occurs. Do not use this term for a nearby named place that does not contain the actual location." .

<http://rs.tdwg.org/dwc/terms/Name_Publication_ID> a owl:ObjectProperty,
        meta:SlotDefinition ;
    rdfs:label "Name Publication ID" ;
    rdfs:range <https://w3id.org/biolink/biolinkml/meta/types/String> ;
    skos:definition "A resolvable globally unique identifier for the original publication of the scientificName." .

<http://rs.tdwg.org/dwc/terms/NomenclaturalChecklist> a owl:Class,
        meta:ClassDefinition ;
    rdfs:label "NomenclaturalChecklist" ;
    skos:altLabel "NomenclaturalChecklist" ;
    skos:definition "A resource describing a nomenclatural checklist." .

<http://rs.tdwg.org/dwc/terms/NomenclaturalCode> a owl:ObjectProperty,
        meta:SlotDefinition ;
    rdfs:label "NomenclaturalCode" ;
    rdfs:range <https://w3id.org/biolink/biolinkml/meta/types/String> ;
    skos:definition "The nomenclatural code under which the ScientificName is constructed. Examples: \"ICBN\", \"ICZN\", \"BC\", \"ICNCP\", \"BioCode\"" .

<http://rs.tdwg.org/dwc/terms/Notes> a owl:ObjectProperty,
        meta:SlotDefinition ;
    rdfs:label "Notes" ;
    rdfs:range <https://w3id.org/biolink/biolinkml/meta/types/String> ;
    skos:definition "Free text notes attached to the specimen record" .

<http://rs.tdwg.org/dwc/terms/Occurrence> a owl:Class,
        meta:ClassDefinition ;
    rdfs:label "Occurrence" ;
    rdfs:subClassOf [ a owl:Restriction ;
            owl:maxQualifiedCardinality 1 ;
            owl:onClass <https://w3id.org/biolink/biolinkml/meta/types/String> ;
            owl:onProperty <http://rs.tdwg.org/dwc/terms/Occurrence_Remarks> ],
        [ a owl:Restriction ;
            owl:maxQualifiedCardinality 1 ;
            owl:onClass <https://w3id.org/biolink/biolinkml/meta/types/String> ;
            owl:onProperty <http://rs.tdwg.org/dwc/terms/Record_Number> ],
        [ a owl:Restriction ;
            owl:maxQualifiedCardinality 1 ;
            owl:onClass <https://w3id.org/biolink/biolinkml/meta/types/String> ;
            owl:onProperty <http://rs.tdwg.org/dwc/terms/associatedTaxa> ],
        [ a owl:Restriction ;
            owl:maxQualifiedCardinality 1 ;
            owl:onClass <https://w3id.org/biolink/biolinkml/meta/types/String> ;
            owl:onProperty <http://rs.tdwg.org/dwc/terms/Organism_Quantity_Type> ],
        [ a owl:Restriction ;
            owl:maxQualifiedCardinality 1 ;
            owl:onClass <https://w3id.org/biolink/biolinkml/meta/types/String> ;
            owl:onProperty <http://rs.tdwg.org/dwc/terms/Disposition> ],
        [ a owl:Restriction ;
            owl:maxQualifiedCardinality 1 ;
            owl:onClass <https://w3id.org/biolink/biolinkml/meta/types/String> ;
            owl:onProperty <http://rs.tdwg.org/dwc/terms/sex> ],
        [ a owl:Restriction ;
            owl:maxQualifiedCardinality 1 ;
            owl:onClass <https://w3id.org/biolink/biolinkml/meta/types/String> ;
            owl:onProperty <http://rs.tdwg.org/dwc/terms/Behavior> ],
        [ a owl:Restriction ;
            owl:maxQualifiedCardinality 1 ;
            owl:onClass <https://w3id.org/biolink/biolinkml/meta/types/String> ;
            owl:onProperty <http://rs.tdwg.org/dwc/terms/preparations> ],
        [ a owl:Restriction ;
            owl:maxQualifiedCardinality 1 ;
            owl:onClass <https://w3id.org/biolink/biolinkml/meta/types/String> ;
            owl:onProperty <http://rs.tdwg.org/dwc/terms/Establishment_Means> ],
        [ a owl:Restriction ;
            owl:maxQualifiedCardinality 1 ;
            owl:onClass <https://w3id.org/biolink/biolinkml/meta/types/String> ;
            owl:onProperty <http://rs.tdwg.org/dwc/terms/organismQuantity> ],
        [ a owl:Restriction ;
            owl:maxQualifiedCardinality 1 ;
            owl:onClass <https://w3id.org/biolink/biolinkml/meta/types/String> ;
            owl:onProperty <http://rs.tdwg.org/dwc/terms/Occurrence_Status> ],
        [ a owl:Restriction ;
            owl:maxQualifiedCardinality 1 ;
            owl:onClass <https://w3id.org/biolink/biolinkml/meta/types/String> ;
            owl:onProperty <http://rs.tdwg.org/dwc/terms/Sex> ],
        [ a owl:Restriction ;
            owl:maxQualifiedCardinality 1 ;
            owl:onClass <https://w3id.org/biolink/biolinkml/meta/types/String> ;
            owl:onProperty <http://rs.tdwg.org/dwc/terms/Associated_References> ],
        [ a owl:Restriction ;
            owl:maxQualifiedCardinality 1 ;
            owl:onClass <https://w3id.org/biolink/biolinkml/meta/types/String> ;
            owl:onProperty <http://rs.tdwg.org/dwc/terms/Occurrence_ID> ],
        [ a owl:Restriction ;
            owl:maxQualifiedCardinality 1 ;
            owl:onClass <https://w3id.org/biolink/biolinkml/meta/types/String> ;
            owl:onProperty <http://rs.tdwg.org/dwc/terms/associatedMedia> ],
        [ a owl:Restriction ;
            owl:maxQualifiedCardinality 1 ;
            owl:onClass <https://w3id.org/biolink/biolinkml/meta/types/String> ;
            owl:onProperty <http://rs.tdwg.org/dwc/terms/Life_Stage> ],
        [ a owl:Restriction ;
            owl:maxQualifiedCardinality 1 ;
            owl:onClass <https://w3id.org/biolink/biolinkml/meta/types/String> ;
            owl:onProperty <http://rs.tdwg.org/dwc/terms/Preparations> ],
        [ a owl:Restriction ;
            owl:maxQualifiedCardinality 1 ;
            owl:onClass <https://w3id.org/biolink/biolinkml/meta/types/String> ;
            owl:onProperty <http://rs.tdwg.org/dwc/terms/Other_Catalog_Numbers> ],
        [ a owl:Restriction ;
            owl:maxQualifiedCardinality 1 ;
            owl:onClass <https://w3id.org/biolink/biolinkml/meta/types/String> ;
            owl:onProperty <http://rs.tdwg.org/dwc/terms/Catalog_Number> ],
        [ a owl:Restriction ;
            owl:maxQualifiedCardinality 1 ;
            owl:onClass <https://w3id.org/biolink/biolinkml/meta/types/String> ;
            owl:onProperty <http://rs.tdwg.org/dwc/terms/disposition> ],
        [ a owl:Restriction ;
            owl:maxQualifiedCardinality 1 ;
            owl:onClass <https://w3id.org/biolink/biolinkml/meta/types/String> ;
            owl:onProperty <http://rs.tdwg.org/dwc/terms/individualCount> ],
        [ a owl:Restriction ;
            owl:maxQualifiedCardinality 1 ;
            owl:onClass <https://w3id.org/biolink/biolinkml/meta/types/String> ;
            owl:onProperty <http://rs.tdwg.org/dwc/terms/lifeStage> ],
        [ a owl:Restriction ;
            owl:maxQualifiedCardinality 1 ;
            owl:onClass <https://w3id.org/biolink/biolinkml/meta/types/String> ;
            owl:onProperty <http://rs.tdwg.org/dwc/terms/recordNumber> ],
        [ a owl:Restriction ;
            owl:maxQualifiedCardinality 1 ;
            owl:onClass <https://w3id.org/biolink/biolinkml/meta/types/String> ;
            owl:onProperty <http://rs.tdwg.org/dwc/terms/Associated_Media> ],
        [ a owl:Restriction ;
            owl:maxQualifiedCardinality 1 ;
            owl:onClass <https://w3id.org/biolink/biolinkml/meta/types/String> ;
            owl:onProperty <http://rs.tdwg.org/dwc/terms/catalogNumber> ],
        [ a owl:Restriction ;
            owl:maxQualifiedCardinality 1 ;
            owl:onClass <https://w3id.org/biolink/biolinkml/meta/types/String> ;
            owl:onProperty <http://rs.tdwg.org/dwc/terms/reproductiveCondition> ],
        [ a owl:Restriction ;
            owl:maxQualifiedCardinality 1 ;
            owl:onClass <https://w3id.org/biolink/biolinkml/meta/types/String> ;
            owl:onProperty <http://rs.tdwg.org/dwc/terms/Associated_Taxa> ],
        [ a owl:Restriction ;
            owl:maxQualifiedCardinality 1 ;
            owl:onClass <https://w3id.org/biolink/biolinkml/meta/types/String> ;
            owl:onProperty <http://rs.tdwg.org/dwc/terms/occurrenceID> ],
        [ a owl:Restriction ;
            owl:maxQualifiedCardinality 1 ;
            owl:onClass <https://w3id.org/biolink/biolinkml/meta/types/String> ;
            owl:onProperty <http://rs.tdwg.org/dwc/terms/occurrenceRemarks> ],
        [ a owl:Restriction ;
            owl:maxQualifiedCardinality 1 ;
            owl:onClass <https://w3id.org/biolink/biolinkml/meta/types/String> ;
            owl:onProperty <http://rs.tdwg.org/dwc/terms/occurrenceStatus> ],
        [ a owl:Restriction ;
            owl:maxQualifiedCardinality 1 ;
            owl:onClass <https://w3id.org/biolink/biolinkml/meta/types/String> ;
            owl:onProperty <http://rs.tdwg.org/dwc/terms/organismQuantityType> ],
        [ a owl:Restriction ;
            owl:maxQualifiedCardinality 1 ;
            owl:onClass <https://w3id.org/biolink/biolinkml/meta/types/String> ;
            owl:onProperty <http://rs.tdwg.org/dwc/terms/Reproductive_Condition> ],
        [ a owl:Restriction ;
            owl:maxQualifiedCardinality 1 ;
            owl:onClass <https://w3id.org/biolink/biolinkml/meta/types/String> ;
            owl:onProperty <http://rs.tdwg.org/dwc/terms/Individual_Count> ],
        [ a owl:Restriction ;
            owl:maxQualifiedCardinality 1 ;
            owl:onClass <https://w3id.org/biolink/biolinkml/meta/types/String> ;
            owl:onProperty <http://rs.tdwg.org/dwc/terms/otherCatalogNumbers> ],
        [ a owl:Restriction ;
            owl:maxQualifiedCardinality 1 ;
            owl:onClass <https://w3id.org/biolink/biolinkml/meta/types/String> ;
            owl:onProperty <http://rs.tdwg.org/dwc/terms/recordedBy> ],
        [ a owl:Restriction ;
            owl:maxQualifiedCardinality 1 ;
            owl:onClass <https://w3id.org/biolink/biolinkml/meta/types/String> ;
            owl:onProperty <http://rs.tdwg.org/dwc/terms/establishmentMeans> ],
        [ a owl:Restriction ;
            owl:maxQualifiedCardinality 1 ;
            owl:onClass <https://w3id.org/biolink/biolinkml/meta/types/String> ;
            owl:onProperty <http://rs.tdwg.org/dwc/terms/Organism_Quantity> ],
        [ a owl:Restriction ;
            owl:maxQualifiedCardinality 1 ;
            owl:onClass <https://w3id.org/biolink/biolinkml/meta/types/String> ;
            owl:onProperty <http://rs.tdwg.org/dwc/terms/Associated_Sequences> ],
        [ a owl:Restriction ;
            owl:maxQualifiedCardinality 1 ;
            owl:onClass <https://w3id.org/biolink/biolinkml/meta/types/String> ;
            owl:onProperty <http://rs.tdwg.org/dwc/terms/associatedReferences> ],
        [ a owl:Restriction ;
            owl:maxQualifiedCardinality 1 ;
            owl:onClass <https://w3id.org/biolink/biolinkml/meta/types/String> ;
            owl:onProperty <http://rs.tdwg.org/dwc/terms/associatedSequences> ],
        [ a owl:Restriction ;
            owl:maxQualifiedCardinality 1 ;
            owl:onClass <https://w3id.org/biolink/biolinkml/meta/types/String> ;
            owl:onProperty <http://rs.tdwg.org/dwc/terms/behavior> ],
        [ a owl:Restriction ;
            owl:maxQualifiedCardinality 1 ;
            owl:onClass <https://w3id.org/biolink/biolinkml/meta/types/String> ;
            owl:onProperty <http://rs.tdwg.org/dwc/terms/Recorded_By> ] ;
    skos:altLabel "Occurrence" ;
    skos:definition "A resource describing an instance of the Occurrence class." ;
    skos:exactMatch <http://rs.tdwg.org/dwc/dwctype/version/Occurrence-2009-04-24> .

<http://rs.tdwg.org/dwc/terms/OccurrenceMeasurement> a owl:Class,
        meta:ClassDefinition ;
    rdfs:label "Occurrence Measurement" ;
    skos:altLabel "Occurrence Measurement" ;
    skos:definition "The category of information pertaining to measurements accociated with an occurrence." .

<http://rs.tdwg.org/dwc/terms/Occurrence_Attributes> a owl:ObjectProperty,
        meta:SlotDefinition ;
    rdfs:label "Occurrence Attributes" ;
    rdfs:range <https://w3id.org/biolink/biolinkml/meta/types/String> ;
    skos:definition "A list (concatenated and separated) of additional measurements, facts, characteristics, or assertions about the Occurrence." .

<http://rs.tdwg.org/dwc/terms/Occurrence_Details> a owl:ObjectProperty,
        meta:SlotDefinition ;
    rdfs:label "Occurrence Details" ;
    rdfs:range <https://w3id.org/biolink/biolinkml/meta/types/String> ;
    skos:definition "A reference (publication, URI) to the most detailed information available about the Occurrence." .

<http://rs.tdwg.org/dwc/terms/Occurrence_Measurement_Accuracy> a owl:ObjectProperty,
        meta:SlotDefinition ;
    rdfs:label "Occurrence Measurement Accuracy" ;
    rdfs:range <https://w3id.org/biolink/biolinkml/meta/types/String> ;
    skos:definition "The description of the error associated with the occurrenceAttributeValue." .

<http://rs.tdwg.org/dwc/terms/Occurrence_Measurement_Determined_By> a owl:ObjectProperty,
        meta:SlotDefinition ;
    rdfs:label "Occurrence Measurement Determined By" ;
    rdfs:range <https://w3id.org/biolink/biolinkml/meta/types/String> ;
    skos:definition "The agent responsible for having determined the value of the measurement or characteristic of the occurrence." .

<http://rs.tdwg.org/dwc/terms/Occurrence_Measurement_Determined_Date> a owl:ObjectProperty,
        meta:SlotDefinition ;
    rdfs:label "Occurrence Measurement Determined Date" ;
    rdfs:range <https://w3id.org/biolink/biolinkml/meta/types/String> ;
    skos:definition "The date on which the the measurement or characteristic of the occurrence was made. Recommended best practice is to use an encoding scheme, such as ISO 8601:2004(E)." .

<http://rs.tdwg.org/dwc/terms/Occurrence_Measurement_ID> a owl:ObjectProperty,
        meta:SlotDefinition ;
    rdfs:label "Occurrence Measurement ID" ;
    rdfs:range <https://w3id.org/biolink/biolinkml/meta/types/String> ;
    skos:definition "An identifier for the occurrence attribute. May be a global unique identifier or an identifier specific to the data set." .

<http://rs.tdwg.org/dwc/terms/Occurrence_Measurement_Remarks> a owl:ObjectProperty,
        meta:SlotDefinition ;
    rdfs:label "Occurrence Measurement Remarks" ;
    rdfs:range <https://w3id.org/biolink/biolinkml/meta/types/String> ;
    skos:definition "Comments or notes accompanying the measurement or characteristic of the occurrence." .

<http://rs.tdwg.org/dwc/terms/Occurrence_Measurement_Type> a owl:ObjectProperty,
        meta:SlotDefinition ;
    rdfs:label "Occurrence Measurement Type" ;
    rdfs:range <https://w3id.org/biolink/biolinkml/meta/types/String> ;
    skos:definition "The nature of the measurement or characteristic of the occurrence. Recommended best practice is to use a controlled vocabulary." .

<http://rs.tdwg.org/dwc/terms/Occurrence_Measurement_Unit> a owl:ObjectProperty,
        meta:SlotDefinition ;
    rdfs:label "Occurrence Measurement Unit" ;
    rdfs:range <https://w3id.org/biolink/biolinkml/meta/types/String> ;
    skos:definition "The units for the value of the measurement or characteristic of the occurrence. Recommended best practice is to use International System of Units (SI) units." .

<http://rs.tdwg.org/dwc/terms/Occurrence_Measurement_Value> a owl:ObjectProperty,
        meta:SlotDefinition ;
    rdfs:label "Occurrence Measurement Value" ;
    rdfs:range <https://w3id.org/biolink/biolinkml/meta/types/String> ;
    skos:definition "The value of the measurement or characteristic of the occurrence." .

<http://rs.tdwg.org/dwc/terms/Organism> a owl:Class,
        meta:ClassDefinition ;
    rdfs:label "Organism" ;
    rdfs:subClassOf [ a owl:Restriction ;
            owl:maxQualifiedCardinality 1 ;
            owl:onClass <https://w3id.org/biolink/biolinkml/meta/types/String> ;
            owl:onProperty <http://rs.tdwg.org/dwc/terms/organismScope> ],
        [ a owl:Restriction ;
            owl:maxQualifiedCardinality 1 ;
            owl:onClass <https://w3id.org/biolink/biolinkml/meta/types/String> ;
            owl:onProperty <http://rs.tdwg.org/dwc/terms/Organism_Name> ],
        [ a owl:Restriction ;
            owl:maxQualifiedCardinality 1 ;
            owl:onClass <https://w3id.org/biolink/biolinkml/meta/types/String> ;
            owl:onProperty <http://rs.tdwg.org/dwc/terms/organismRemarks> ],
        [ a owl:Restriction ;
            owl:maxQualifiedCardinality 1 ;
            owl:onClass <https://w3id.org/biolink/biolinkml/meta/types/String> ;
            owl:onProperty <http://rs.tdwg.org/dwc/terms/previousIdentifications> ],
        [ a owl:Restriction ;
            owl:maxQualifiedCardinality 1 ;
            owl:onClass <https://w3id.org/biolink/biolinkml/meta/types/String> ;
            owl:onProperty <http://rs.tdwg.org/dwc/terms/associatedOrganisms> ],
        [ a owl:Restriction ;
            owl:maxQualifiedCardinality 1 ;
            owl:onClass <https://w3id.org/biolink/biolinkml/meta/types/String> ;
            owl:onProperty <http://rs.tdwg.org/dwc/terms/Organism_ID> ],
        [ a owl:Restriction ;
            owl:maxQualifiedCardinality 1 ;
            owl:onClass <https://w3id.org/biolink/biolinkml/meta/types/String> ;
            owl:onProperty <http://rs.tdwg.org/dwc/terms/Organism_Scope> ],
        [ a owl:Restriction ;
            owl:maxQualifiedCardinality 1 ;
            owl:onClass <https://w3id.org/biolink/biolinkml/meta/types/String> ;
            owl:onProperty <http://rs.tdwg.org/dwc/terms/organismName> ],
        [ a owl:Restriction ;
            owl:maxQualifiedCardinality 1 ;
            owl:onClass <https://w3id.org/biolink/biolinkml/meta/types/String> ;
            owl:onProperty <http://rs.tdwg.org/dwc/terms/Associated_Occurrences> ],
        [ a owl:Restriction ;
            owl:maxQualifiedCardinality 1 ;
            owl:onClass <https://w3id.org/biolink/biolinkml/meta/types/String> ;
            owl:onProperty <http://rs.tdwg.org/dwc/terms/associatedOccurrences> ],
        [ a owl:Restriction ;
            owl:maxQualifiedCardinality 1 ;
            owl:onClass <https://w3id.org/biolink/biolinkml/meta/types/String> ;
            owl:onProperty <http://rs.tdwg.org/dwc/terms/Organism_Remarks> ],
        [ a owl:Restriction ;
            owl:maxQualifiedCardinality 1 ;
            owl:onClass <https://w3id.org/biolink/biolinkml/meta/types/String> ;
            owl:onProperty <http://rs.tdwg.org/dwc/terms/organismID> ],
        [ a owl:Restriction ;
            owl:maxQualifiedCardinality 1 ;
            owl:onClass <https://w3id.org/biolink/biolinkml/meta/types/String> ;
            owl:onProperty <http://rs.tdwg.org/dwc/terms/Previous_Identifications> ],
        [ a owl:Restriction ;
            owl:maxQualifiedCardinality 1 ;
            owl:onClass <https://w3id.org/biolink/biolinkml/meta/types/String> ;
            owl:onProperty <http://rs.tdwg.org/dwc/terms/Associated_Organisms> ] ;
    skos:altLabel "Organism" ;
    skos:definition "A particular organism or defined group of organisms considered to be taxonomically homogeneous." .

<http://rs.tdwg.org/dwc/terms/OriginalCoordinateSystem> a owl:ObjectProperty,
        meta:SlotDefinition ;
    rdfs:label "OriginalCoordinateSystem" ;
    rdfs:range <https://w3id.org/biolink/biolinkml/meta/types/String> ;
    skos:definition "The name of the system in which the original geographic coordinates were recorded (e.g., \"decimal degrees\", \"degrees minutes seconds\", \"UTM\", etc.)." .

<http://rs.tdwg.org/dwc/terms/OtherCatalogNumbers> a owl:ObjectProperty,
        meta:SlotDefinition ;
    rdfs:label "OtherCatalogNumbers" ;
    rdfs:range <https://w3id.org/biolink/biolinkml/meta/types/String> ;
    skos:definition "A list of previous or alternative fully qualified catalog numbers of the cataloged item whether in the current collection or in any other." .

<http://rs.tdwg.org/dwc/terms/Owner_Institution_Code> a owl:ObjectProperty,
        meta:SlotDefinition ;
    rdfs:label "Owner Institution Code" ;
    rdfs:range <https://w3id.org/biolink/biolinkml/meta/types/String> ;
    skos:definition "The name (or acronym) in use by the institution having ownership of the object(s) or information referred to in the record." .

<http://rs.tdwg.org/dwc/terms/PointRadiusSpatialFit> a owl:ObjectProperty,
        meta:SlotDefinition ;
    rdfs:label "PointRadiusSpatialFit" ;
    rdfs:range <https://w3id.org/biolink/biolinkml/meta/types/String> ;
    skos:definition "A measure of how well the circle defined by the coordinates and uncertainty match the original spatial representation, as a ratio of the area of the circle to the area of the original spatial representation. Legal values are 0, greater than or equal to 1, or undefined. A value of 1 is an exact match or 100% overlap. A value of 0 should be used if the given georeference does not completely contain the original representation. The PointRadiusSpatialFit is undefined if the original representation is a point without uncertainty and the given georeference is not that same point (without uncertainty). If both the original and the given georeference are the same point, the PointRadiusSpatialFit is 1. Detailed explanations with graphical examples can be found in the Guide to Best Practices for Georeferencing (Chapman and Wieczorek, eds. 2006)." .

<http://rs.tdwg.org/dwc/terms/Point_Radius_Spatial_Fit> a owl:ObjectProperty,
        meta:SlotDefinition ;
    rdfs:label "Point Radius Spatial Fit" ;
    rdfs:range <https://w3id.org/biolink/biolinkml/meta/types/String> ;
    skos:definition "The ratio of the area of the point-radius (decimalLatitude, decimalLongitude, coordinateUncertaintyInMeters) to the area of the true (original, or most specific) spatial representation of the Location. Legal values are 0, greater than or equal to 1, or undefined. A value of 1 is an exact match or 100% overlap. A value of 0 should be used if the given point-radius does not completely contain the original representation. The pointRadiusSpatialFit is undefined (and should be left blank) if the original representation is a point without uncertainty and the given georeference is not that same point (without uncertainty). If both the original and the given georeference are the same point, the pointRadiusSpatialFit is 1." .

<http://rs.tdwg.org/dwc/terms/PreparationType> a owl:ObjectProperty,
        meta:SlotDefinition ;
    rdfs:label "PreparationType" ;
    rdfs:range <https://w3id.org/biolink/biolinkml/meta/types/String> ;
    skos:definition "The type of preparation (skin. slide, etc). Probably best to add this as a record element rather than access point. Should be a list of preparations for a single collection record." .

<http://rs.tdwg.org/dwc/terms/PreservedSpecimen> a owl:Class,
        meta:ClassDefinition ;
    rdfs:label "Preserved Specimen",
        "PreservedSpecimen" ;
    skos:altLabel "Preserved Specimen",
        "PreservedSpecimen" ;
    skos:definition "A specimen that has been preserved." ;
    skos:exactMatch <http://rs.tdwg.org/dwc/dwctype/version/PreservedSpecimen-2011-10-16>,
        <http://rs.tdwg.org/dwc/dwctype/version/PreservedSpecimen-2014-10-23> .

<http://rs.tdwg.org/dwc/terms/PreviousCatalogNumber> a owl:ObjectProperty,
        meta:SlotDefinition ;
    rdfs:label "PreviousCatalogNumber" ;
    rdfs:range <https://w3id.org/biolink/biolinkml/meta/types/String> ;
    skos:definition "The previous (fully qualified) catalog number of the Cataloged Item if the item earlier identified by another Catalog Number, either in the current catalog or another Institution / catalog. A fully qualified Catalog Number is preceded by Institution Code and Collection Code, with a space separating the each subelement. Referencing a previous Catalog Number does not imply that a record for the referenced item is or is not present in the corresponding catalog, or even that the referenced catalog still exists. This access point is intended to provide a way to retrieve this record by previously used identifier, which may used in the literature. In future versions of this schema this attribute should be set-valued." .

<http://rs.tdwg.org/dwc/terms/RelatedCatalogItem> a owl:ObjectProperty,
        meta:SlotDefinition ;
    rdfs:label "RelatedCatalogItem" ;
    rdfs:range <https://w3id.org/biolink/biolinkml/meta/types/String> ;
    skos:definition "The fully qualified identifier of a related Catalog Item (a reference to another specimen); Institution Code, Collection Code, and Catalog Number of the related Cataloged Item, where a space separates the three subelements." .

<http://rs.tdwg.org/dwc/terms/RelatedCatalogedItems> a owl:ObjectProperty,
        meta:SlotDefinition ;
    rdfs:label "RelatedCatalogedItems" ;
    rdfs:range <https://w3id.org/biolink/biolinkml/meta/types/String> ;
    skos:definition "The fully qualified identifier (Institution Code + \" \" + Collection Code + \" \" + Catalog Number) of the related Cataloged Item, preceded by the nature of the relationship (e.g., (sibling of) MVZ Mamm 1234)." .

<http://rs.tdwg.org/dwc/terms/RelatedInformation> a owl:ObjectProperty,
        meta:SlotDefinition ;
    rdfs:label "RelatedInformation" ;
    rdfs:range <https://w3id.org/biolink/biolinkml/meta/types/String> ;
    skos:definition "Free text references to information not delivered via the conceptual schema, including URLs to specimen details, publications, bibliographic references, etc." .

<http://rs.tdwg.org/dwc/terms/Related_Basis_of_Record> a owl:ObjectProperty,
        meta:SlotDefinition ;
    rdfs:label "Related Basis of Record" ;
    rdfs:range <https://w3id.org/biolink/biolinkml/meta/types/String> ;
    skos:definition "The nature of the related resource. Recommended best practice is to use the same controlled vocabulary as for basisOfRecord." .

<http://rs.tdwg.org/dwc/terms/Related_Resource_Type> a owl:ObjectProperty,
        meta:SlotDefinition ;
    rdfs:label "Related Resource Type" ;
    rdfs:range <https://w3id.org/biolink/biolinkml/meta/types/String> ;
    skos:definition "The type of the related resource. Recommended best practice is to use a controlled vocabulary." .

<http://rs.tdwg.org/dwc/terms/RelationshipType> a owl:ObjectProperty,
        meta:SlotDefinition ;
    rdfs:label "RelationshipType" ;
    rdfs:range <https://w3id.org/biolink/biolinkml/meta/types/String> ;
    skos:definition "A named or coded valued that identifies the kind relationship between this Collection Item and the referenced Collection Item. Named values include: \"parasite of\", \"epiphyte on\", \"progeny of\", etc. In future versions of this schema this attribute should be set-valued." .

<http://rs.tdwg.org/dwc/terms/Remarks> a owl:ObjectProperty,
        meta:SlotDefinition ;
    rdfs:label "Remarks" ;
    rdfs:range <https://w3id.org/biolink/biolinkml/meta/types/String> ;
    skos:definition "Free text comments accompanying the object or observation record." .

<http://rs.tdwg.org/dwc/terms/ResourceRelationship> a owl:Class,
        meta:ClassDefinition ;
    rdfs:label "Resource Relationship",
        "ResourceRelationship" ;
    rdfs:subClassOf [ a owl:Restriction ;
            owl:maxQualifiedCardinality 1 ;
            owl:onClass <https://w3id.org/biolink/biolinkml/meta/types/String> ;
            owl:onProperty <http://rs.tdwg.org/dwc/terms/Related_Resource_ID> ],
        [ a owl:Restriction ;
            owl:maxQualifiedCardinality 1 ;
            owl:onClass <https://w3id.org/biolink/biolinkml/meta/types/String> ;
            owl:onProperty <http://rs.tdwg.org/dwc/terms/relationshipOfResource> ],
        [ a owl:Restriction ;
            owl:maxQualifiedCardinality 1 ;
            owl:onClass <https://w3id.org/biolink/biolinkml/meta/types/String> ;
            owl:onProperty <http://rs.tdwg.org/dwc/terms/relationshipRemarks> ],
        [ a owl:Restriction ;
            owl:maxQualifiedCardinality 1 ;
            owl:onClass <https://w3id.org/biolink/biolinkml/meta/types/String> ;
            owl:onProperty <http://rs.tdwg.org/dwc/terms/relatedResourceID> ],
        [ a owl:Restriction ;
            owl:maxQualifiedCardinality 1 ;
            owl:onClass <https://w3id.org/biolink/biolinkml/meta/types/String> ;
            owl:onProperty <http://rs.tdwg.org/dwc/terms/Relationship_Established_Date> ],
        [ a owl:Restriction ;
            owl:maxQualifiedCardinality 1 ;
            owl:onClass <https://w3id.org/biolink/biolinkml/meta/types/String> ;
            owl:onProperty <http://rs.tdwg.org/dwc/terms/Relationship_Remarks> ],
        [ a owl:Restriction ;
            owl:maxQualifiedCardinality 1 ;
            owl:onClass <https://w3id.org/biolink/biolinkml/meta/types/String> ;
            owl:onProperty <http://rs.tdwg.org/dwc/terms/relationshipEstablishedDate> ],
        [ a owl:Restriction ;
            owl:maxQualifiedCardinality 1 ;
            owl:onClass <https://w3id.org/biolink/biolinkml/meta/types/String> ;
            owl:onProperty <http://rs.tdwg.org/dwc/terms/Resource_ID> ],
        [ a owl:Restriction ;
            owl:maxQualifiedCardinality 1 ;
            owl:onClass <https://w3id.org/biolink/biolinkml/meta/types/String> ;
            owl:onProperty <http://rs.tdwg.org/dwc/terms/Relationship_According_To> ],
        [ a owl:Restriction ;
            owl:maxQualifiedCardinality 1 ;
            owl:onClass <https://w3id.org/biolink/biolinkml/meta/types/String> ;
            owl:onProperty <http://rs.tdwg.org/dwc/terms/Relationship_Of_Resource> ],
        [ a owl:Restriction ;
            owl:maxQualifiedCardinality 1 ;
            owl:onClass <https://w3id.org/biolink/biolinkml/meta/types/String> ;
            owl:onProperty <http://rs.tdwg.org/dwc/terms/relationshipAccordingTo> ],
        [ a owl:Restriction ;
            owl:maxQualifiedCardinality 1 ;
            owl:onClass <https://w3id.org/biolink/biolinkml/meta/types/String> ;
            owl:onProperty <http://rs.tdwg.org/dwc/terms/resourceID> ],
        [ a owl:Restriction ;
            owl:maxQualifiedCardinality 1 ;
            owl:onClass <https://w3id.org/biolink/biolinkml/meta/types/String> ;
            owl:onProperty <http://rs.tdwg.org/dwc/terms/resourceRelationshipID> ],
        [ a owl:Restriction ;
            owl:maxQualifiedCardinality 1 ;
            owl:onClass <https://w3id.org/biolink/biolinkml/meta/types/String> ;
            owl:onProperty <http://rs.tdwg.org/dwc/terms/Resource_Relationship_ID> ] ;
    skos:altLabel "Resource Relationship",
        "ResourceRelationship" ;
    skos:definition "A relationship of one rdfs:Resource (http://www.w3.org/2000/01/rdf-schema#Resource) to another." ;
    skos:exactMatch <http://rs.tdwg.org/dwc/terms/version/ResourceRelationship-2009-01-21>,
        <http://rs.tdwg.org/dwc/terms/version/ResourceRelationship-2014-10-23> .

<http://rs.tdwg.org/dwc/terms/Sample> a owl:Class,
        meta:ClassDefinition ;
    rdfs:label "Sample" ;
    skos:altLabel "Sample" ;
    skos:definition "Container class for information about the results of a sampling event (specimen, observation, etc.)" .

<http://rs.tdwg.org/dwc/terms/SampleAttribute> a owl:Class,
        meta:ClassDefinition ;
    rdfs:label "Sample Attribute" ;
    skos:altLabel "Sample Attribute" ;
    skos:definition "Container class for information about attributes related to a given sample." .

<http://rs.tdwg.org/dwc/terms/Sample_Attribute_Accuracy> a owl:ObjectProperty,
        meta:SlotDefinition ;
    rdfs:label "Sample Attribute Accuracy" ;
    rdfs:range <https://w3id.org/biolink/biolinkml/meta/types/String> ;
    skos:definition "The description of the error associated with the SampleAttributeValue." .

<http://rs.tdwg.org/dwc/terms/Sample_Attribute_Determined_By> a owl:ObjectProperty,
        meta:SlotDefinition ;
    rdfs:label "Sample Attribute Determined By" ;
    rdfs:range <https://w3id.org/biolink/biolinkml/meta/types/String> ;
    skos:definition "The agent responsible for having determined the value of the measurement or characteristic of the sample." .

<http://rs.tdwg.org/dwc/terms/Sample_Attribute_Determined_Date> a owl:ObjectProperty,
        meta:SlotDefinition ;
    rdfs:label "Sample Attribute Determined Date" ;
    rdfs:range <https://w3id.org/biolink/biolinkml/meta/types/String> ;
    skos:definition "The date on which the the measurement or characteristic of the sample was made." .

<http://rs.tdwg.org/dwc/terms/Sample_Attribute_ID> a owl:ObjectProperty,
        meta:SlotDefinition ;
    rdfs:label "Sample Attribute ID" ;
    rdfs:range <https://w3id.org/biolink/biolinkml/meta/types/String> ;
    skos:definition "An identifier for the sampling attribute. May be a global unique identifier or an identifier specific to the data set." .

<http://rs.tdwg.org/dwc/terms/Sample_Attribute_Remarks> a owl:ObjectProperty,
        meta:SlotDefinition ;
    rdfs:label "Sample Attribute Remarks" ;
    rdfs:range <https://w3id.org/biolink/biolinkml/meta/types/String> ;
    skos:definition "Comments or notes accompanying the measurement or characteristic of the sample." .

<http://rs.tdwg.org/dwc/terms/Sample_Attribute_Type> a owl:ObjectProperty,
        meta:SlotDefinition ;
    rdfs:label "Sample Attribute Type" ;
    rdfs:range <https://w3id.org/biolink/biolinkml/meta/types/String> ;
    skos:definition "The nature of the measurement or characteristic of the sample. Recommended best practice is to use a controlled vocabulary." .

<http://rs.tdwg.org/dwc/terms/Sample_Attribute_Unit> a owl:ObjectProperty,
        meta:SlotDefinition ;
    rdfs:label "Sample Attribute Unit" ;
    rdfs:range <https://w3id.org/biolink/biolinkml/meta/types/String> ;
    skos:definition "The units for the value of the measurement or characteristic of the sample. Recommended best practice is to use International System of Units (SI) units." .

<http://rs.tdwg.org/dwc/terms/Sample_Attribute_Value> a owl:ObjectProperty,
        meta:SlotDefinition ;
    rdfs:label "Sample Attribute Value" ;
    rdfs:range <https://w3id.org/biolink/biolinkml/meta/types/String> ;
    skos:definition "The value of the measurement or characteristic of the sample." .

<http://rs.tdwg.org/dwc/terms/Sample_Remarks> a owl:ObjectProperty,
        meta:SlotDefinition ;
    rdfs:label "Sample Remarks" ;
    rdfs:range <https://w3id.org/biolink/biolinkml/meta/types/String> ;
    skos:definition "Comments or notes about the sample or record." .

<http://rs.tdwg.org/dwc/terms/SamplingEvent> a owl:Class,
        meta:ClassDefinition ;
    rdfs:label "Sampling Event" ;
    skos:altLabel "Sampling Event" ;
    skos:definition "Container class for information about the conditions and methods of acquisition of samples." .

<http://rs.tdwg.org/dwc/terms/SamplingLocation> a owl:Class,
        meta:ClassDefinition ;
    rdfs:label "Sampling Location" ;
    skos:altLabel "Sampling Location" ;
    skos:definition "Container class for information about the location where a sampling event occurred." .

<http://rs.tdwg.org/dwc/terms/Sampling_Event_Attributes> a owl:ObjectProperty,
        meta:SlotDefinition ;
    rdfs:label "Sampling Event Attributes" ;
    rdfs:range <https://w3id.org/biolink/biolinkml/meta/types/String> ;
    skos:definition "A list (concatenated and separated) of additional measurements or characteristics of the sampling event." .

<http://rs.tdwg.org/dwc/terms/Sampling_Event_ID> a owl:ObjectProperty,
        meta:SlotDefinition ;
    rdfs:label "Sampling Event ID" ;
    rdfs:range <https://w3id.org/biolink/biolinkml/meta/types/String> ;
    skos:definition "An identifier for the sampling event. May be a global unique identifier or an identifier specific to the data set." .

<http://rs.tdwg.org/dwc/terms/Sampling_Event_Remarks> a owl:ObjectProperty,
        meta:SlotDefinition ;
    rdfs:label "Sampling Event Remarks" ;
    rdfs:range <https://w3id.org/biolink/biolinkml/meta/types/String> ;
    skos:definition "Comments or notes about the sampling event." .

<http://rs.tdwg.org/dwc/terms/Sampling_Location_ID> a owl:ObjectProperty,
        meta:SlotDefinition ;
    rdfs:label "Sampling Location ID" ;
    rdfs:range <https://w3id.org/biolink/biolinkml/meta/types/String> ;
    skos:definition "An identifier for the sampling location. May be a global unique identifier or an identifier specific to the data set." .

<http://rs.tdwg.org/dwc/terms/Sampling_Location_Remarks> a owl:ObjectProperty,
        meta:SlotDefinition ;
    rdfs:label "Sampling Location Remarks" ;
    rdfs:range <https://w3id.org/biolink/biolinkml/meta/types/String> ;
    skos:definition "Comments or notes about the sampling location." .

<http://rs.tdwg.org/dwc/terms/ScientificName> a owl:ObjectProperty,
        meta:SlotDefinition ;
    rdfs:label "ScientificName" ;
    rdfs:range <https://w3id.org/biolink/biolinkml/meta/types/String> ;
    skos:definition "The full name of the lowest level taxon to which the organism has been identified in the most recent accepted determination, specified as precisely as possible, including name-author, year or authorship, sensu or sec. (according to or following) author, and indication of uncertainty. Conceptually equivalent to a full taxonomic identification as given by the identifier (verbatim). Does not include the identifier name or date of identification. Examples: \"Coleoptera\" (an Order), \"Vespertilionidae\" (a Family), \"Manis\" (a Genus), \"Ctenomys sociabilis\" (Genus + SpecificEpithet), \"Ambystoma tigrinum diaboli\" (Genus + SpecificEpithet + SubspecificEpithet), \"Quercus agrifolia var. oxyadenia (Torr.) J.T. Howell\" (Genus + SpecificEpithet + InfraspecificRank + InfraspecificEpithet + AuthorYearOfScientificName)." .

<http://rs.tdwg.org/dwc/terms/ScientificNameAuthor> a owl:ObjectProperty,
        meta:SlotDefinition ;
    rdfs:label "ScientificNameAuthor" ;
    rdfs:range <https://w3id.org/biolink/biolinkml/meta/types/String> ;
    skos:definition "The author of the ScientificName. Can be more than one author in a concatenated string. Should be formatted according to the conventions of the applicable taxonomic discipline." .

<http://rs.tdwg.org/dwc/terms/Scientific_Name_Rank> a owl:ObjectProperty,
        meta:SlotDefinition ;
    rdfs:label "Scientific Name Rank" ;
    rdfs:range <https://w3id.org/biolink/biolinkml/meta/types/String> ;
    skos:definition "The taxonomic rank of the most specific name in the scientificName. Recommended best practice is to use a controlled vocabulary." .

<http://rs.tdwg.org/dwc/terms/Species> a owl:ObjectProperty,
        meta:SlotDefinition ;
    rdfs:label "Species" ;
    rdfs:range <https://w3id.org/biolink/biolinkml/meta/types/String> ;
    skos:definition "The phylogenetic specific epithet of the cataloged item." .

<http://rs.tdwg.org/dwc/terms/SpecificEpithet> a owl:ObjectProperty,
        meta:SlotDefinition ;
    rdfs:label "SpecificEpithet" ;
    rdfs:range <https://w3id.org/biolink/biolinkml/meta/types/String> ;
    skos:definition "The specific epithet of the scientific name applied to the organism." .

<http://rs.tdwg.org/dwc/terms/Start_Time_of_Day> a owl:ObjectProperty,
        meta:SlotDefinition ;
    rdfs:label "Start Time of Day" ;
    rdfs:range <https://w3id.org/biolink/biolinkml/meta/types/String> ;
    skos:definition "The time of day when the event began, expressed as decimal hours from midnight, local time." .

<http://rs.tdwg.org/dwc/terms/StateProvince> a owl:ObjectProperty,
        meta:SlotDefinition ;
    rdfs:label "StateProvince" ;
    rdfs:range <https://w3id.org/biolink/biolinkml/meta/types/String> ;
    skos:definition "The full, unabbreviated name of the state, province, or region (i.e., the next smaller political region than Country) in which the organism was collected or observed." .

<http://rs.tdwg.org/dwc/terms/State_Province> a owl:ObjectProperty,
        meta:SlotDefinition ;
    rdfs:label "State Province" ;
    rdfs:range <https://w3id.org/biolink/biolinkml/meta/types/String> ;
    skos:definition "The name of the next smaller administrative region than country (state, province, canton, department, region, etc.) in which the Location occurs." .

<http://rs.tdwg.org/dwc/terms/Subspecies> a owl:ObjectProperty,
        meta:SlotDefinition ;
    rdfs:label "Subspecies" ;
    rdfs:range <https://w3id.org/biolink/biolinkml/meta/types/String> ;
    skos:definition "The phylogenetic subspecific epithet of the cataloged item." .

<http://rs.tdwg.org/dwc/terms/Taxon> a owl:Class,
        meta:ClassDefinition ;
    rdfs:label "Taxon" ;
    rdfs:subClassOf [ a owl:Restriction ;
            owl:maxQualifiedCardinality 1 ;
            owl:onClass <https://w3id.org/biolink/biolinkml/meta/types/String> ;
            owl:onProperty <http://rs.tdwg.org/dwc/terms/Taxon_Concept_ID> ],
        [ a owl:Restriction ;
            owl:maxQualifiedCardinality 1 ;
            owl:onClass <https://w3id.org/biolink/biolinkml/meta/types/String> ;
            owl:onProperty <http://rs.tdwg.org/dwc/terms/Nomenclatural_Code> ],
        [ a owl:Restriction ;
            owl:maxQualifiedCardinality 1 ;
            owl:onClass <https://w3id.org/biolink/biolinkml/meta/types/String> ;
            owl:onProperty <http://rs.tdwg.org/dwc/terms/Taxon_ID> ],
        [ a owl:Restriction ;
            owl:maxQualifiedCardinality 1 ;
            owl:onClass <https://w3id.org/biolink/biolinkml/meta/types/String> ;
            owl:onProperty <http://rs.tdwg.org/dwc/terms/taxonID> ],
        [ a owl:Restriction ;
            owl:maxQualifiedCardinality 1 ;
            owl:onClass <https://w3id.org/biolink/biolinkml/meta/types/String> ;
            owl:onProperty <http://rs.tdwg.org/dwc/terms/Vernacular_Name> ],
        [ a owl:Restriction ;
            owl:maxQualifiedCardinality 1 ;
            owl:onClass <https://w3id.org/biolink/biolinkml/meta/types/String> ;
            owl:onProperty <http://rs.tdwg.org/dwc/terms/Name_According_To> ],
        [ a owl:Restriction ;
            owl:maxQualifiedCardinality 1 ;
            owl:onClass <https://w3id.org/biolink/biolinkml/meta/types/String> ;
            owl:onProperty <http://rs.tdwg.org/dwc/terms/Subgenus> ],
        [ a owl:Restriction ;
            owl:maxQualifiedCardinality 1 ;
            owl:onClass <https://w3id.org/biolink/biolinkml/meta/types/String> ;
            owl:onProperty <http://rs.tdwg.org/dwc/terms/kingdom> ],
        [ a owl:Restriction ;
            owl:maxQualifiedCardinality 1 ;
            owl:onClass <https://w3id.org/biolink/biolinkml/meta/types/String> ;
            owl:onProperty <http://rs.tdwg.org/dwc/terms/Kingdom> ],
        [ a owl:Restriction ;
            owl:maxQualifiedCardinality 1 ;
            owl:onClass <https://w3id.org/biolink/biolinkml/meta/types/String> ;
            owl:onProperty <http://rs.tdwg.org/dwc/terms/Scientific_Name_Authorship> ],
        [ a owl:Restriction ;
            owl:maxQualifiedCardinality 1 ;
            owl:onClass <https://w3id.org/biolink/biolinkml/meta/types/String> ;
            owl:onProperty <http://rs.tdwg.org/dwc/terms/Class> ],
        [ a owl:Restriction ;
            owl:maxQualifiedCardinality 1 ;
            owl:onClass <https://w3id.org/biolink/biolinkml/meta/types/String> ;
            owl:onProperty <http://rs.tdwg.org/dwc/terms/Parent_Name_Usage> ],
        [ a owl:Restriction ;
            owl:maxQualifiedCardinality 1 ;
            owl:onClass <https://w3id.org/biolink/biolinkml/meta/types/String> ;
            owl:onProperty <http://rs.tdwg.org/dwc/terms/Name_Published_In_ID> ],
        [ a owl:Restriction ;
            owl:maxQualifiedCardinality 1 ;
            owl:onClass <https://w3id.org/biolink/biolinkml/meta/types/String> ;
            owl:onProperty <http://rs.tdwg.org/dwc/terms/Nomenclatural_Status> ],
        [ a owl:Restriction ;
            owl:maxQualifiedCardinality 1 ;
            owl:onClass <https://w3id.org/biolink/biolinkml/meta/types/String> ;
            owl:onProperty <http://rs.tdwg.org/dwc/terms/Phylum> ],
        [ a owl:Restriction ;
            owl:maxQualifiedCardinality 1 ;
            owl:onClass <https://w3id.org/biolink/biolinkml/meta/types/String> ;
            owl:onProperty <http://rs.tdwg.org/dwc/terms/nomenclaturalStatus> ],
        [ a owl:Restriction ;
            owl:maxQualifiedCardinality 1 ;
            owl:onClass <https://w3id.org/biolink/biolinkml/meta/types/String> ;
            owl:onProperty <http://rs.tdwg.org/dwc/terms/Accepted_Name_Usage> ],
        [ a owl:Restriction ;
            owl:maxQualifiedCardinality 1 ;
            owl:onClass <https://w3id.org/biolink/biolinkml/meta/types/String> ;
            owl:onProperty <http://rs.tdwg.org/dwc/terms/taxonomicStatus> ],
        [ a owl:Restriction ;
            owl:maxQualifiedCardinality 1 ;
            owl:onClass <https://w3id.org/biolink/biolinkml/meta/types/String> ;
            owl:onProperty <http://rs.tdwg.org/dwc/terms/Verbatim_Taxon_Rank> ],
        [ a owl:Restriction ;
            owl:maxQualifiedCardinality 1 ;
            owl:onClass <https://w3id.org/biolink/biolinkml/meta/types/String> ;
            owl:onProperty <http://rs.tdwg.org/dwc/terms/Original_Name_Usage_ID> ],
        [ a owl:Restriction ;
            owl:maxQualifiedCardinality 1 ;
            owl:onClass <https://w3id.org/biolink/biolinkml/meta/types/String> ;
            owl:onProperty <http://rs.tdwg.org/dwc/terms/taxonRemarks> ],
        [ a owl:Restriction ;
            owl:maxQualifiedCardinality 1 ;
            owl:onClass <https://w3id.org/biolink/biolinkml/meta/types/String> ;
            owl:onProperty <http://rs.tdwg.org/dwc/terms/Taxon_Remarks> ],
        [ a owl:Restriction ;
            owl:maxQualifiedCardinality 1 ;
            owl:onClass <https://w3id.org/biolink/biolinkml/meta/types/String> ;
            owl:onProperty <http://rs.tdwg.org/dwc/terms/originalNameUsageID> ],
        [ a owl:Restriction ;
            owl:maxQualifiedCardinality 1 ;
            owl:onClass <https://w3id.org/biolink/biolinkml/meta/types/String> ;
            owl:onProperty <http://rs.tdwg.org/dwc/terms/acceptedNameUsage> ],
        [ a owl:Restriction ;
            owl:maxQualifiedCardinality 1 ;
            owl:onClass <https://w3id.org/biolink/biolinkml/meta/types/String> ;
            owl:onProperty <http://rs.tdwg.org/dwc/terms/order> ],
        [ a owl:Restriction ;
            owl:maxQualifiedCardinality 1 ;
            owl:onClass <https://w3id.org/biolink/biolinkml/meta/types/String> ;
            owl:onProperty <http://rs.tdwg.org/dwc/terms/scientificNameID> ],
        [ a owl:Restriction ;
            owl:maxQualifiedCardinality 1 ;
            owl:onClass <https://w3id.org/biolink/biolinkml/meta/types/String> ;
            owl:onProperty <http://rs.tdwg.org/dwc/terms/taxonConceptID> ],
        [ a owl:Restriction ;
            owl:maxQualifiedCardinality 1 ;
            owl:onClass <https://w3id.org/biolink/biolinkml/meta/types/String> ;
            owl:onProperty <http://rs.tdwg.org/dwc/terms/Name_According_To_ID> ],
        [ a owl:Restriction ;
            owl:maxQualifiedCardinality 1 ;
            owl:onClass <https://w3id.org/biolink/biolinkml/meta/types/String> ;
            owl:onProperty <http://rs.tdwg.org/dwc/terms/Original_Name_Usage> ],
        [ a owl:Restriction ;
            owl:maxQualifiedCardinality 1 ;
            owl:onClass <https://w3id.org/biolink/biolinkml/meta/types/String> ;
            owl:onProperty <http://rs.tdwg.org/dwc/terms/specificEpithet> ],
        [ a owl:Restriction ;
            owl:maxQualifiedCardinality 1 ;
            owl:onClass <https://w3id.org/biolink/biolinkml/meta/types/String> ;
            owl:onProperty <http://rs.tdwg.org/dwc/terms/Scientific_Name_ID> ],
        [ a owl:Restriction ;
            owl:maxQualifiedCardinality 1 ;
            owl:onClass <https://w3id.org/biolink/biolinkml/meta/types/String> ;
            owl:onProperty <http://rs.tdwg.org/dwc/terms/Name_Published_In> ],
        [ a owl:Restriction ;
            owl:maxQualifiedCardinality 1 ;
            owl:onClass <https://w3id.org/biolink/biolinkml/meta/types/String> ;
            owl:onProperty <http://rs.tdwg.org/dwc/terms/Scientific_Name> ],
        [ a owl:Restriction ;
            owl:maxQualifiedCardinality 1 ;
            owl:onClass <https://w3id.org/biolink/biolinkml/meta/types/String> ;
            owl:onProperty <http://rs.tdwg.org/dwc/terms/class> ],
        [ a owl:Restriction ;
            owl:maxQualifiedCardinality 1 ;
            owl:onClass <https://w3id.org/biolink/biolinkml/meta/types/String> ;
            owl:onProperty <http://rs.tdwg.org/dwc/terms/Genus> ],
        [ a owl:Restriction ;
            owl:maxQualifiedCardinality 1 ;
            owl:onClass <https://w3id.org/biolink/biolinkml/meta/types/String> ;
            owl:onProperty <http://rs.tdwg.org/dwc/terms/Family> ],
        [ a owl:Restriction ;
            owl:maxQualifiedCardinality 1 ;
            owl:onClass <https://w3id.org/biolink/biolinkml/meta/types/String> ;
            owl:onProperty <http://rs.tdwg.org/dwc/terms/infraspecificEpithet> ],
        [ a owl:Restriction ;
            owl:maxQualifiedCardinality 1 ;
            owl:onClass <https://w3id.org/biolink/biolinkml/meta/types/String> ;
            owl:onProperty <http://rs.tdwg.org/dwc/terms/taxonRank> ],
        [ a owl:Restriction ;
            owl:maxQualifiedCardinality 1 ;
            owl:onClass <https://w3id.org/biolink/biolinkml/meta/types/String> ;
            owl:onProperty <http://rs.tdwg.org/dwc/terms/scientificNameAuthorship> ],
        [ a owl:Restriction ;
            owl:maxQualifiedCardinality 1 ;
            owl:onClass <https://w3id.org/biolink/biolinkml/meta/types/String> ;
            owl:onProperty <http://rs.tdwg.org/dwc/terms/Name_Published_In_Year> ],
        [ a owl:Restriction ;
            owl:maxQualifiedCardinality 1 ;
            owl:onClass <https://w3id.org/biolink/biolinkml/meta/types/String> ;
            owl:onProperty <http://rs.tdwg.org/dwc/terms/originalNameUsage> ],
        [ a owl:Restriction ;
            owl:maxQualifiedCardinality 1 ;
            owl:onClass <https://w3id.org/biolink/biolinkml/meta/types/String> ;
            owl:onProperty <http://rs.tdwg.org/dwc/terms/nameAccordingTo> ],
        [ a owl:Restriction ;
            owl:maxQualifiedCardinality 1 ;
            owl:onClass <https://w3id.org/biolink/biolinkml/meta/types/String> ;
            owl:onProperty <http://rs.tdwg.org/dwc/terms/Specific_Epithet> ],
        [ a owl:Restriction ;
            owl:maxQualifiedCardinality 1 ;
            owl:onClass <https://w3id.org/biolink/biolinkml/meta/types/String> ;
            owl:onProperty <http://rs.tdwg.org/dwc/terms/Accepted_Name_Usage_ID> ],
        [ a owl:Restriction ;
            owl:maxQualifiedCardinality 1 ;
            owl:onClass <https://w3id.org/biolink/biolinkml/meta/types/String> ;
            owl:onProperty <http://rs.tdwg.org/dwc/terms/nameAccordingToID> ],
        [ a owl:Restriction ;
            owl:maxQualifiedCardinality 1 ;
            owl:onClass <https://w3id.org/biolink/biolinkml/meta/types/String> ;
            owl:onProperty <http://rs.tdwg.org/dwc/terms/Taxon_Rank> ],
        [ a owl:Restriction ;
            owl:maxQualifiedCardinality 1 ;
            owl:onClass <https://w3id.org/biolink/biolinkml/meta/types/String> ;
            owl:onProperty <http://rs.tdwg.org/dwc/terms/higherClassification> ],
        [ a owl:Restriction ;
            owl:maxQualifiedCardinality 1 ;
            owl:onClass <https://w3id.org/biolink/biolinkml/meta/types/String> ;
            owl:onProperty <http://rs.tdwg.org/dwc/terms/Parent_Name_Usage_ID> ],
        [ a owl:Restriction ;
            owl:maxQualifiedCardinality 1 ;
            owl:onClass <https://w3id.org/biolink/biolinkml/meta/types/String> ;
            owl:onProperty <http://rs.tdwg.org/dwc/terms/Taxonomic_Status> ],
        [ a owl:Restriction ;
            owl:maxQualifiedCardinality 1 ;
            owl:onClass <https://w3id.org/biolink/biolinkml/meta/types/String> ;
            owl:onProperty <http://rs.tdwg.org/dwc/terms/scientificName> ],
        [ a owl:Restriction ;
            owl:maxQualifiedCardinality 1 ;
            owl:onClass <https://w3id.org/biolink/biolinkml/meta/types/String> ;
            owl:onProperty <http://rs.tdwg.org/dwc/terms/acceptedNameUsageID> ],
        [ a owl:Restriction ;
            owl:maxQualifiedCardinality 1 ;
            owl:onClass <https://w3id.org/biolink/biolinkml/meta/types/String> ;
            owl:onProperty <http://rs.tdwg.org/dwc/terms/namePublishedIn> ],
        [ a owl:Restriction ;
            owl:maxQualifiedCardinality 1 ;
            owl:onClass <https://w3id.org/biolink/biolinkml/meta/types/String> ;
            owl:onProperty <http://rs.tdwg.org/dwc/terms/family> ],
        [ a owl:Restriction ;
            owl:maxQualifiedCardinality 1 ;
            owl:onClass <https://w3id.org/biolink/biolinkml/meta/types/String> ;
            owl:onProperty <http://rs.tdwg.org/dwc/terms/parentNameUsageID> ],
        [ a owl:Restriction ;
            owl:maxQualifiedCardinality 1 ;
            owl:onClass <https://w3id.org/biolink/biolinkml/meta/types/String> ;
            owl:onProperty <http://rs.tdwg.org/dwc/terms/Infraspecific_Epithet> ],
        [ a owl:Restriction ;
            owl:maxQualifiedCardinality 1 ;
            owl:onClass <https://w3id.org/biolink/biolinkml/meta/types/String> ;
            owl:onProperty <http://rs.tdwg.org/dwc/terms/namePublishedInID> ],
        [ a owl:Restriction ;
            owl:maxQualifiedCardinality 1 ;
            owl:onClass <https://w3id.org/biolink/biolinkml/meta/types/String> ;
            owl:onProperty <http://rs.tdwg.org/dwc/terms/parentNameUsage> ],
        [ a owl:Restriction ;
            owl:maxQualifiedCardinality 1 ;
            owl:onClass <https://w3id.org/biolink/biolinkml/meta/types/String> ;
            owl:onProperty <http://rs.tdwg.org/dwc/terms/vernacularName> ],
        [ a owl:Restriction ;
            owl:maxQualifiedCardinality 1 ;
            owl:onClass <https://w3id.org/biolink/biolinkml/meta/types/String> ;
            owl:onProperty <http://rs.tdwg.org/dwc/terms/phylum> ],
        [ a owl:Restriction ;
            owl:maxQualifiedCardinality 1 ;
            owl:onClass <https://w3id.org/biolink/biolinkml/meta/types/String> ;
            owl:onProperty <http://rs.tdwg.org/dwc/terms/Order> ],
        [ a owl:Restriction ;
            owl:maxQualifiedCardinality 1 ;
            owl:onClass <https://w3id.org/biolink/biolinkml/meta/types/String> ;
            owl:onProperty <http://rs.tdwg.org/dwc/terms/nomenclaturalCode> ],
        [ a owl:Restriction ;
            owl:maxQualifiedCardinality 1 ;
            owl:onClass <https://w3id.org/biolink/biolinkml/meta/types/String> ;
            owl:onProperty <http://rs.tdwg.org/dwc/terms/Higher_Classification> ],
        [ a owl:Restriction ;
            owl:maxQualifiedCardinality 1 ;
            owl:onClass <https://w3id.org/biolink/biolinkml/meta/types/String> ;
            owl:onProperty <http://rs.tdwg.org/dwc/terms/genus> ],
        [ a owl:Restriction ;
            owl:maxQualifiedCardinality 1 ;
            owl:onClass <https://w3id.org/biolink/biolinkml/meta/types/String> ;
            owl:onProperty <http://rs.tdwg.org/dwc/terms/verbatimTaxonRank> ],
        [ a owl:Restriction ;
            owl:maxQualifiedCardinality 1 ;
            owl:onClass <https://w3id.org/biolink/biolinkml/meta/types/String> ;
            owl:onProperty <http://rs.tdwg.org/dwc/terms/namePublishedInYear> ],
        [ a owl:Restriction ;
            owl:maxQualifiedCardinality 1 ;
            owl:onClass <https://w3id.org/biolink/biolinkml/meta/types/String> ;
            owl:onProperty <http://rs.tdwg.org/dwc/terms/subgenus> ] ;
    skos:altLabel "Taxon" ;
    skos:definition "A resource describing an instance of the Taxon class." .

<http://rs.tdwg.org/dwc/terms/Taxon_According_To> a owl:ObjectProperty,
        meta:SlotDefinition ;
    rdfs:label "Taxon According To" ;
    rdfs:range <https://w3id.org/biolink/biolinkml/meta/types/String> ;
    skos:definition "Information about the authorship of this taxon concept which uses the scientificName in their sense (secundum, sensu). Could be a publication (identification key), institution or team of individuals." .

<http://rs.tdwg.org/dwc/terms/Taxon_Attributes> a owl:ObjectProperty,
        meta:SlotDefinition ;
    rdfs:label "Taxon Attributes" ;
    rdfs:range <https://w3id.org/biolink/biolinkml/meta/types/String> ;
    skos:definition "A list (concatenated and separated) of additional measurements, facts, characteristics, or assertions about the taxon." .

<http://rs.tdwg.org/dwc/terms/Taxon_Name_ID> a owl:ObjectProperty,
        meta:SlotDefinition ;
    rdfs:label "Taxon Name ID" ;
    rdfs:range <https://w3id.org/biolink/biolinkml/meta/types/String> ;
    skos:definition "A unique identifier for the scientificName." .

<http://rs.tdwg.org/dwc/terms/TimeCollected> a owl:ObjectProperty,
        meta:SlotDefinition ;
    rdfs:label "TimeCollected" ;
    rdfs:range <https://w3id.org/biolink/biolinkml/meta/types/String> ;
    skos:definition "The time of day the cataloged item was collected, expressed as decimal hours from midnight, local time (e.g., 12.0 = noon, 13.5 = 1:30pm)." .

<http://rs.tdwg.org/dwc/terms/TimeOfDay> a owl:ObjectProperty,
        meta:SlotDefinition ;
    rdfs:label "TimeOfDay" ;
    rdfs:range <https://w3id.org/biolink/biolinkml/meta/types/String> ;
    skos:definition "The time of day a specimen was collected expressed as decimal hours from midnight local time (e.g. 12.0 = mid day, 13.5 = 1:30pm)" .

<http://rs.tdwg.org/dwc/terms/Tissues> a owl:ObjectProperty,
        meta:SlotDefinition ;
    rdfs:label "Tissues" ;
    rdfs:range <https://w3id.org/biolink/biolinkml/meta/types/String> ;
    skos:definition "A concatenated list of tissues and preservation methods (whole (frozen), liver (EDTA), etc.) for the cataloged item." .

<http://rs.tdwg.org/dwc/terms/TypeStatus> a owl:ObjectProperty,
        meta:SlotDefinition ;
    rdfs:label "TypeStatus" ;
    rdfs:range <https://w3id.org/biolink/biolinkml/meta/types/String> ;
    skos:definition "A list of one or more nomenclatural types that the cataloged item represents (e.g., \"holotype of Ctenomys sociabilis. Pearson O. P., and M. I. Christie. 1985. Historia Natural, 5(37):388.\")." .

<http://rs.tdwg.org/dwc/terms/UseWithIRI> a owl:Class,
        meta:ClassDefinition ;
    rdfs:label "UseWithIRI" ;
    skos:altLabel "UseWithIRI" ;
    skos:definition "The category of terms that are recommended to have an IRI as a value." .

<http://rs.tdwg.org/dwc/terms/ValidDistributionFlag> a owl:ObjectProperty,
        meta:SlotDefinition ;
    rdfs:label "ValidDistributionFlag" ;
    rdfs:range <https://w3id.org/biolink/biolinkml/meta/types/String> ;
    skos:definition "A flag (\"true\" or \"false\") that indicates whether the locality information represents a valid distribution occurrence for a specimen. Specimens taken from captivity and showing the captive location should use the value \"false\"." .

<http://rs.tdwg.org/dwc/terms/VerbatimCollectingDate> a owl:ObjectProperty,
        meta:SlotDefinition ;
    rdfs:label "VerbatimCollectingDate" ;
    rdfs:range <https://w3id.org/biolink/biolinkml/meta/types/String> ;
    skos:definition "The verbatim original representation of the date information for the collecting event." .

<http://rs.tdwg.org/dwc/terms/VerbatimCoordinateSystem> a owl:ObjectProperty,
        meta:SlotDefinition ;
    rdfs:label "VerbatimCoordinateSystem" ;
    rdfs:range <https://w3id.org/biolink/biolinkml/meta/types/String> ;
    skos:definition "The name of the system in which the verbatim geographic coordinates were recorded. Examples: \"decimal degrees\", \"degrees minutes seconds\", \"degrees decimal minutes\", \"UTM\"" .

<http://rs.tdwg.org/dwc/terms/VerbatimCoordinates> a owl:ObjectProperty,
        meta:SlotDefinition ;
    rdfs:label "VerbatimCoordinates" ;
    rdfs:range <https://w3id.org/biolink/biolinkml/meta/types/String> ;
    skos:definition "A text representation of the coordinate data (Latitude/ Longitude, UTM, TRS, etc.) from its original source if it cannot be separated into its component parts. Example: \"470999 1234300\"." .

<http://rs.tdwg.org/dwc/terms/VerbatimDepth> a owl:ObjectProperty,
        meta:SlotDefinition ;
    rdfs:label "VerbatimDepth" ;
    rdfs:range <https://w3id.org/biolink/biolinkml/meta/types/String> ;
    skos:definition "A text representation of the Depth in its original format in the source database." .

<http://rs.tdwg.org/dwc/terms/VerbatimElevation> a owl:ObjectProperty,
        meta:SlotDefinition ;
    rdfs:label "VerbatimElevation" ;
    rdfs:range <https://w3id.org/biolink/biolinkml/meta/types/String> ;
    skos:definition "A text representation of the Elevation in its original format in the source database." .

<http://rs.tdwg.org/dwc/terms/VerbatimLatitude> a owl:ObjectProperty,
        meta:SlotDefinition ;
    rdfs:label "VerbatimLatitude" ;
    rdfs:range <https://w3id.org/biolink/biolinkml/meta/types/String> ;
    skos:definition "A text representation of the Latitude part of the coordinate data from its original source. Example: 47d09'99\"N" .

<http://rs.tdwg.org/dwc/terms/VerbatimLongitude> a owl:ObjectProperty,
        meta:SlotDefinition ;
    rdfs:label "VerbatimLongitude" ;
    rdfs:range <https://w3id.org/biolink/biolinkml/meta/types/String> ;
    skos:definition "A text representation of the Longitude part of the coordinate data from its original source. Example: -122.43254" .

<http://rs.tdwg.org/dwc/terms/Verbatim_Coordinate_System> a owl:ObjectProperty,
        meta:SlotDefinition ;
    rdfs:label "Verbatim Coordinate System" ;
    rdfs:range <https://w3id.org/biolink/biolinkml/meta/types/String> ;
    skos:definition "The spatial coordinate system for the verbatimLatitude and verbatimLongitude or the verbatimCoordinates of the Location. Recommended best practice is to use a controlled vocabulary." .

<http://rs.tdwg.org/dwc/terms/Verbatim_Coordinates> a owl:ObjectProperty,
        meta:SlotDefinition ;
    rdfs:label "Verbatim Coordinates" ;
    rdfs:range <https://w3id.org/biolink/biolinkml/meta/types/String> ;
    skos:definition "The verbatim original spatial coordinates of the Location. The coordinate ellipsoid, geodeticDatum, or full Spatial Reference System (SRS) for these coordinates should be stored in verbatimSRS and the coordinate system should be stored in verbatimCoordinateSystem." .

<http://rs.tdwg.org/dwc/terms/Verbatim_Depth> a owl:ObjectProperty,
        meta:SlotDefinition ;
    rdfs:label "Verbatim Depth" ;
    rdfs:range <https://w3id.org/biolink/biolinkml/meta/types/String> ;
    skos:definition "The original description of the depth below the local surface." .

<http://rs.tdwg.org/dwc/terms/Verbatim_Elevation> a owl:ObjectProperty,
        meta:SlotDefinition ;
    rdfs:label "Verbatim Elevation" ;
    rdfs:range <https://w3id.org/biolink/biolinkml/meta/types/String> ;
    skos:definition "The original description of the elevation (altitude, usually above sea level) of the Location." .

<http://rs.tdwg.org/dwc/terms/Verbatim_Latitude> a owl:ObjectProperty,
        meta:SlotDefinition ;
    rdfs:label "Verbatim Latitude" ;
    rdfs:range <https://w3id.org/biolink/biolinkml/meta/types/String> ;
    skos:definition "The verbatim original latitude of the Location. The coordinate ellipsoid, geodeticDatum, or full Spatial Reference System (SRS) for these coordinates should be stored in verbatimSRS and the coordinate system should be stored in verbatimCoordinateSystem." .

<http://rs.tdwg.org/dwc/terms/Verbatim_Locality> a owl:ObjectProperty,
        meta:SlotDefinition ;
    rdfs:label "Verbatim Locality" ;
    rdfs:range <https://w3id.org/biolink/biolinkml/meta/types/String> ;
    skos:definition "The original textual description of the place." .

<http://rs.tdwg.org/dwc/terms/Verbatim_Longitude> a owl:ObjectProperty,
        meta:SlotDefinition ;
    rdfs:label "Verbatim Longitude" ;
    rdfs:range <https://w3id.org/biolink/biolinkml/meta/types/String> ;
    skos:definition "The verbatim original longitude of the Location. The coordinate ellipsoid, geodeticDatum, or full Spatial Reference System (SRS) for these coordinates should be stored in verbatimSRS and the coordinate system should be stored in verbatimCoordinateSystem." .

<http://rs.tdwg.org/dwc/terms/Verbatim_SRS> a owl:ObjectProperty,
        meta:SlotDefinition ;
    rdfs:label "Verbatim SRS" ;
    rdfs:range <https://w3id.org/biolink/biolinkml/meta/types/String> ;
    skos:definition "The ellipsoid, geodetic datum, or spatial reference system (SRS) upon which coordinates given in verbatimLatitude and verbatimLongitude, or verbatimCoordinates are based. Recommended best practice is use the EPSG code as a controlled vocabulary to provide an SRS, if known. Otherwise use a controlled vocabulary for the name or code of the geodetic datum, if known. Otherwise use a controlled vocabulary for the name or code of the ellipsoid, if known. If none of these is known, use the value \"unknown\"." .

<http://rs.tdwg.org/dwc/terms/Verbatim_Scientific_Name_Rank> a owl:ObjectProperty,
        meta:SlotDefinition ;
    rdfs:label "Verbatim Scientific Name Rank" ;
    rdfs:range <https://w3id.org/biolink/biolinkml/meta/types/String> ;
    skos:definition "The taxonomic rank of the most specific name in the scientificName as it appears in the original record." .

<http://rs.tdwg.org/dwc/terms/WaterBody> a owl:ObjectProperty,
        meta:SlotDefinition ;
    rdfs:label "WaterBody" ;
    rdfs:range <https://w3id.org/biolink/biolinkml/meta/types/String> ;
    skos:definition "The full, unabbreviated name of the body of water in or over which the organism was collected or observed." .

<http://rs.tdwg.org/dwc/terms/Water_Body> a owl:ObjectProperty,
        meta:SlotDefinition ;
    rdfs:label "Water Body" ;
    rdfs:range <https://w3id.org/biolink/biolinkml/meta/types/String> ;
    skos:definition "The name of the water body in which the Location occurs. Recommended best practice is to use a controlled vocabulary such as the Getty Thesaurus of Geographic Names." .

<http://rs.tdwg.org/dwc/terms/YearCollected> a owl:ObjectProperty,
        meta:SlotDefinition ;
    rdfs:label "YearCollected" ;
    rdfs:range <https://w3id.org/biolink/biolinkml/meta/types/String> ;
    skos:definition "The four digit year in the Common Era calendar in which the cataloged item was collected." .

<http://rs.tdwg.org/dwc/terms/YearIdentified> a owl:ObjectProperty,
        meta:SlotDefinition ;
    rdfs:label "YearIdentified" ;
    rdfs:range <https://w3id.org/biolink/biolinkml/meta/types/String> ;
    skos:definition "The four digit year in the Common Era calendar in which the cataloged item was identified as having the ScientificName." .

<http://rs.tdwg.org/dwc/terms/accessRights> a owl:ObjectProperty,
        meta:SlotDefinition ;
    rdfs:label "accessRights" ;
    rdfs:range <https://w3id.org/biolink/biolinkml/meta/types/String> ;
    skos:definition "Information about who can access the resource or an indication of its security status. Access Rights may include information regarding access or restrictions based on privacy, security, or other policies." .

<http://rs.tdwg.org/dwc/terms/basisOfRecord> a owl:ObjectProperty,
        meta:SlotDefinition ;
    rdfs:label "basisOfRecord" ;
    rdfs:range <https://w3id.org/biolink/biolinkml/meta/types/String> ;
    skos:definition "The specific nature of the data record." .

<http://rs.tdwg.org/dwc/terms/bibliographicCitation> a owl:ObjectProperty,
        meta:SlotDefinition ;
    rdfs:label "bibliographicCitation" ;
    rdfs:range <https://w3id.org/biolink/biolinkml/meta/types/String> ;
    skos:definition "A bibliographic reference for the resource as a statement indicating how this record should be cited (attributed) when used." .

<http://rs.tdwg.org/dwc/terms/collectionCode> a owl:ObjectProperty,
        meta:SlotDefinition ;
    rdfs:label "collectionCode" ;
    rdfs:range <https://w3id.org/biolink/biolinkml/meta/types/String> ;
    skos:definition "The name, acronym, coden, or initialism identifying the collection or data set from which the record was derived." .

<http://rs.tdwg.org/dwc/terms/collectionID> a owl:ObjectProperty,
        meta:SlotDefinition ;
    rdfs:label "collectionID" ;
    rdfs:range <https://w3id.org/biolink/biolinkml/meta/types/String> ;
    skos:definition "An identifier for the collection or dataset from which the record was derived." .

<http://rs.tdwg.org/dwc/terms/continent> a owl:ObjectProperty,
        meta:SlotDefinition ;
    rdfs:label "continent" ;
    rdfs:range <https://w3id.org/biolink/biolinkml/meta/types/String> ;
    skos:definition "The name of the continent in which the Location occurs." .

<http://rs.tdwg.org/dwc/terms/coordinatePrecision> a owl:ObjectProperty,
        meta:SlotDefinition ;
    rdfs:label "coordinatePrecision" ;
    rdfs:range <https://w3id.org/biolink/biolinkml/meta/types/String> ;
    skos:definition "A decimal representation of the precision of the coordinates given in the decimalLatitude and decimalLongitude." .

<http://rs.tdwg.org/dwc/terms/coordinateUncertaintyInMeters> a owl:ObjectProperty,
        meta:SlotDefinition ;
    rdfs:label "coordinateUncertaintyInMeters" ;
    rdfs:range <https://w3id.org/biolink/biolinkml/meta/types/String> ;
    skos:definition "The horizontal distance (in meters) from the given decimalLatitude and decimalLongitude describing the smallest circle containing the whole of the Location. Leave the value empty if the uncertainty is unknown, cannot be estimated, or is not applicable (because there are no coordinates). Zero is not a valid value for this term." .

<http://rs.tdwg.org/dwc/terms/country> a owl:ObjectProperty,
        meta:SlotDefinition ;
    rdfs:label "country" ;
    rdfs:range <https://w3id.org/biolink/biolinkml/meta/types/String> ;
    skos:definition "The name of the country or major administrative unit in which the Location occurs." .

<http://rs.tdwg.org/dwc/terms/countryCode> a owl:ObjectProperty,
        meta:SlotDefinition ;
    rdfs:label "countryCode" ;
    rdfs:range <https://w3id.org/biolink/biolinkml/meta/types/String> ;
    skos:definition "The standard code for the country in which the Location occurs." .

<http://rs.tdwg.org/dwc/terms/county> a owl:ObjectProperty,
        meta:SlotDefinition ;
    rdfs:label "county" ;
    rdfs:range <https://w3id.org/biolink/biolinkml/meta/types/String> ;
    skos:definition "The full, unabbreviated name of the next smaller administrative region than stateProvince (county, shire, department, etc.) in which the Location occurs." .

<http://rs.tdwg.org/dwc/terms/dataGeneralizations> a owl:ObjectProperty,
        meta:SlotDefinition ;
    rdfs:label "dataGeneralizations" ;
    rdfs:range <https://w3id.org/biolink/biolinkml/meta/types/String> ;
    skos:definition "Actions taken to make the shared data less specific or complete than in its original form. Suggests that alternative data of higher quality may be available on request." .

<http://rs.tdwg.org/dwc/terms/datasetID> a owl:ObjectProperty,
        meta:SlotDefinition ;
    rdfs:label "datasetID" ;
    rdfs:range <https://w3id.org/biolink/biolinkml/meta/types/String> ;
    skos:definition "An identifier for the set of data. May be a global unique identifier or an identifier specific to a collection or institution." .

<http://rs.tdwg.org/dwc/terms/datasetName> a owl:ObjectProperty,
        meta:SlotDefinition ;
    rdfs:label "datasetName" ;
    rdfs:range <https://w3id.org/biolink/biolinkml/meta/types/String> ;
    skos:definition "The name identifying the data set from which the record was derived." .

<http://rs.tdwg.org/dwc/terms/decimalLatitude> a owl:ObjectProperty,
        meta:SlotDefinition ;
    rdfs:label "decimalLatitude" ;
    rdfs:range <https://w3id.org/biolink/biolinkml/meta/types/String> ;
    skos:definition "The geographic latitude (in decimal degrees, using the spatial reference system given in geodeticDatum) of the geographic center of a Location. Positive values are north of the Equator, negative values are south of it. Legal values lie between -90 and 90, inclusive." .

<http://rs.tdwg.org/dwc/terms/decimalLongitude> a owl:ObjectProperty,
        meta:SlotDefinition ;
    rdfs:label "decimalLongitude" ;
    rdfs:range <https://w3id.org/biolink/biolinkml/meta/types/String> ;
    skos:definition "The geographic longitude (in decimal degrees, using the spatial reference system given in geodeticDatum) of the geographic center of a Location. Positive values are east of the Greenwich Meridian, negative values are west of it. Legal values lie between -180 and 180, inclusive." .

<http://rs.tdwg.org/dwc/terms/dynamicProperties> a owl:ObjectProperty,
        meta:SlotDefinition ;
    rdfs:label "dynamicProperties" ;
    rdfs:range <https://w3id.org/biolink/biolinkml/meta/types/String> ;
    skos:definition "A list of additional measurements, facts, characteristics, or assertions about the record. Meant to provide a mechanism for structured content." .

<http://rs.tdwg.org/dwc/terms/earliestGeochronologicalEra> a owl:ObjectProperty,
        meta:SlotDefinition ;
    rdfs:label "earliestGeochronologicalEra" ;
    rdfs:range <https://w3id.org/biolink/biolinkml/meta/types/String> ;
    skos:definition "Use to link a dwc:GeologicalContext instance to chronostratigraphic time periods at the lowest possible level in a standardized hierarchy.   Use this property to point to the earliest possible geological time period from which the cataloged item was collected." .

<http://rs.tdwg.org/dwc/terms/footprintSRS> a owl:ObjectProperty,
        meta:SlotDefinition ;
    rdfs:label "footprintSRS" ;
    rdfs:range <https://w3id.org/biolink/biolinkml/meta/types/String> ;
    skos:definition "A Well-Known Text (WKT) representation of the Spatial Reference System (SRS) for the footprintWKT of the Location. Do not use this term to describe the SRS of the decimalLatitude and decimalLongitude, even if it is the same as for the footprintWKT - use the geodeticDatum instead." .

<http://rs.tdwg.org/dwc/terms/footprintSpatialFit> a owl:ObjectProperty,
        meta:SlotDefinition ;
    rdfs:label "footprintSpatialFit" ;
    rdfs:range <https://w3id.org/biolink/biolinkml/meta/types/String> ;
    skos:definition "The ratio of the area of the footprint (footprintWKT) to the area of the true (original, or most specific) spatial representation of the Location. Legal values are 0, greater than or equal to 1, or undefined. A value of 1 is an exact match or 100% overlap. A value of 0 should be used if the given footprint does not completely contain the original representation. The footprintSpatialFit is undefined (and should be left blank) if the original representation is a point and the given georeference is not that same point. If both the original and the given georeference are the same point, the footprintSpatialFit is 1." .

<http://rs.tdwg.org/dwc/terms/footprintWKT> a owl:ObjectProperty,
        meta:SlotDefinition ;
    rdfs:label "footprintWKT" ;
    rdfs:range <https://w3id.org/biolink/biolinkml/meta/types/String> ;
    skos:definition "A Well-Known Text (WKT) representation of the shape (footprint, geometry) that defines the Location. A Location may have both a point-radius representation (see decimalLatitude) and a footprint representation, and they may differ from each other." .

<http://rs.tdwg.org/dwc/terms/fromLithostratigraphicUnit> a owl:ObjectProperty,
        meta:SlotDefinition ;
    rdfs:label "fromLithostratigraphicUnit" ;
    rdfs:range <https://w3id.org/biolink/biolinkml/meta/types/String> ;
    skos:definition "Use to link a dwc:GeologicalContext instance to an IRI-identified lithostratigraphic unit at the lowest possible level in a hierarchy." .

<http://rs.tdwg.org/dwc/terms/geodeticDatum> a owl:ObjectProperty,
        meta:SlotDefinition ;
    rdfs:label "geodeticDatum" ;
    rdfs:range <https://w3id.org/biolink/biolinkml/meta/types/String> ;
    skos:definition "The ellipsoid, geodetic datum, or spatial reference system (SRS) upon which the geographic coordinates given in decimalLatitude and decimalLongitude as based." .

<http://rs.tdwg.org/dwc/terms/georeferenceProtocol> a owl:ObjectProperty,
        meta:SlotDefinition ;
    rdfs:label "georeferenceProtocol" ;
    rdfs:range <https://w3id.org/biolink/biolinkml/meta/types/String> ;
    skos:definition "A description or reference to the methods used to determine the spatial footprint, coordinates, and uncertainties." .

<http://rs.tdwg.org/dwc/terms/georeferenceRemarks> a owl:ObjectProperty,
        meta:SlotDefinition ;
    rdfs:label "georeferenceRemarks" ;
    rdfs:range <https://w3id.org/biolink/biolinkml/meta/types/String> ;
    skos:definition "Notes or comments about the spatial description determination, explaining assumptions made in addition or opposition to the those formalized in the method referred to in georeferenceProtocol." .

<http://rs.tdwg.org/dwc/terms/georeferenceSources> a owl:ObjectProperty,
        meta:SlotDefinition ;
    rdfs:label "georeferenceSources" ;
    rdfs:range <https://w3id.org/biolink/biolinkml/meta/types/String> ;
    skos:definition "A list (concatenated and separated) of maps, gazetteers, or other resources used to georeference the Location, described specifically enough to allow anyone in the future to use the same resources." .

<http://rs.tdwg.org/dwc/terms/georeferenceVerificationStatus> a owl:ObjectProperty,
        meta:SlotDefinition ;
    rdfs:label "georeferenceVerificationStatus" ;
    rdfs:range <https://w3id.org/biolink/biolinkml/meta/types/String> ;
    skos:definition "A categorical description of the extent to which the georeference has been verified to represent the best possible spatial description." .

<http://rs.tdwg.org/dwc/terms/georeferencedBy> a owl:ObjectProperty,
        meta:SlotDefinition ;
    rdfs:label "georeferencedBy" ;
    rdfs:range <https://w3id.org/biolink/biolinkml/meta/types/String> ;
    skos:definition "A list (concatenated and separated) of names of people, groups, or organizations who determined the georeference (spatial representation) for the Location." .

<http://rs.tdwg.org/dwc/terms/georeferencedDate> a owl:ObjectProperty,
        meta:SlotDefinition ;
    rdfs:label "georeferencedDate" ;
    rdfs:range <https://w3id.org/biolink/biolinkml/meta/types/String> ;
    skos:definition "The date on which the Location was georeferenced." .

<http://rs.tdwg.org/dwc/terms/higherGeography> a owl:ObjectProperty,
        meta:SlotDefinition ;
    rdfs:label "higherGeography" ;
    rdfs:range <https://w3id.org/biolink/biolinkml/meta/types/String> ;
    skos:definition "A list (concatenated and separated) of geographic names less specific than the information captured in the locality term." .

<http://rs.tdwg.org/dwc/terms/higherGeographyID> a owl:ObjectProperty,
        meta:SlotDefinition ;
    rdfs:label "higherGeographyID" ;
    rdfs:range <https://w3id.org/biolink/biolinkml/meta/types/String> ;
    skos:definition "An identifier for the geographic region within which the Location occurred." .

<http://rs.tdwg.org/dwc/terms/inCollection> a owl:ObjectProperty,
        meta:SlotDefinition ;
    rdfs:label "inCollection" ;
    rdfs:range <https://w3id.org/biolink/biolinkml/meta/types/String> ;
    skos:definition "Use to link any subject resource that is part of a collection to the collection containing the resource." .

<http://rs.tdwg.org/dwc/terms/inDataset> a owl:ObjectProperty,
        meta:SlotDefinition ;
    rdfs:label "inDataset" ;
    rdfs:range <https://w3id.org/biolink/biolinkml/meta/types/String> ;
    skos:definition "Use to link a subject dataset record to the dataset which contains it." .

<http://rs.tdwg.org/dwc/terms/inDescribedPlace> a owl:ObjectProperty,
        meta:SlotDefinition ;
    rdfs:label "inDescribedPlace" ;
    rdfs:range <https://w3id.org/biolink/biolinkml/meta/types/String> ;
    skos:definition "Use to link a dcterms:Location instance subject to the lowest level standardized hierarchically-described resource." .

<http://rs.tdwg.org/dwc/terms/informationWithheld> a owl:ObjectProperty,
        meta:SlotDefinition ;
    rdfs:label "informationWithheld" ;
    rdfs:range <https://w3id.org/biolink/biolinkml/meta/types/String> ;
    skos:definition "Additional information that exists, but that has not been shared in the given record." .

<http://rs.tdwg.org/dwc/terms/institutionCode> a owl:ObjectProperty,
        meta:SlotDefinition ;
    rdfs:label "institutionCode" ;
    rdfs:range <https://w3id.org/biolink/biolinkml/meta/types/String> ;
    skos:definition "The name (or acronym) in use by the institution having custody of the object(s) or information referred to in the record." .

<http://rs.tdwg.org/dwc/terms/institutionID> a owl:ObjectProperty,
        meta:SlotDefinition ;
    rdfs:label "institutionID" ;
    rdfs:range <https://w3id.org/biolink/biolinkml/meta/types/String> ;
    skos:definition "An identifier for the institution having custody of the object(s) or information referred to in the record." .

<http://rs.tdwg.org/dwc/terms/island> a owl:ObjectProperty,
        meta:SlotDefinition ;
    rdfs:label "island" ;
    rdfs:range <https://w3id.org/biolink/biolinkml/meta/types/String> ;
    skos:definition "The name of the island on or near which the Location occurs." .

<http://rs.tdwg.org/dwc/terms/islandGroup> a owl:ObjectProperty,
        meta:SlotDefinition ;
    rdfs:label "islandGroup" ;
    rdfs:range <https://w3id.org/biolink/biolinkml/meta/types/String> ;
    skos:definition "The name of the island group in which the Location occurs." .

<http://rs.tdwg.org/dwc/terms/language> a owl:ObjectProperty,
        meta:SlotDefinition ;
    rdfs:label "language" ;
    rdfs:range <https://w3id.org/biolink/biolinkml/meta/types/String> ;
    skos:definition "A language of the resource." .

<http://rs.tdwg.org/dwc/terms/latestGeochronologicalEra> a owl:ObjectProperty,
        meta:SlotDefinition ;
    rdfs:label "latestGeochronologicalEra" ;
    rdfs:range <https://w3id.org/biolink/biolinkml/meta/types/String> ;
    skos:definition "Use to link a dwc:GeologicalContext instance to chronostratigraphic time periods at the lowest possible level in a standardized hierarchy.   Use this property to point to the latest possible geological time period from which the cataloged item was collected." .

<http://rs.tdwg.org/dwc/terms/license> a owl:ObjectProperty,
        meta:SlotDefinition ;
    rdfs:label "license" ;
    rdfs:range <https://w3id.org/biolink/biolinkml/meta/types/String> ;
    skos:definition "A legal document giving official permission to do something with the resource." .

<http://rs.tdwg.org/dwc/terms/locality> a owl:ObjectProperty,
        meta:SlotDefinition ;
    rdfs:label "locality" ;
    rdfs:range <https://w3id.org/biolink/biolinkml/meta/types/String> ;
    skos:definition "The specific description of the place. Less specific geographic information can be provided in other geographic terms (higherGeography, continent, country, stateProvince, county, municipality, waterBody, island, islandGroup). This term may contain information modified from the original to correct perceived errors or standardize the description." .

<http://rs.tdwg.org/dwc/terms/locationAccordingTo> a owl:ObjectProperty,
        meta:SlotDefinition ;
    rdfs:label "locationAccordingTo" ;
    rdfs:range <https://w3id.org/biolink/biolinkml/meta/types/String> ;
    skos:definition "Information about the source of this Location information. Could be a publication (gazetteer), institution, or team of individuals." .

<http://rs.tdwg.org/dwc/terms/locationID> a owl:ObjectProperty,
        meta:SlotDefinition ;
    rdfs:label "locationID" ;
    rdfs:range <https://w3id.org/biolink/biolinkml/meta/types/String> ;
    skos:definition "An identifier for the set of location information (data associated with dcterms:Location). May be a global unique identifier or an identifier specific to the data set." .

<http://rs.tdwg.org/dwc/terms/locationRemarks> a owl:ObjectProperty,
        meta:SlotDefinition ;
    rdfs:label "locationRemarks" ;
    rdfs:range <https://w3id.org/biolink/biolinkml/meta/types/String> ;
    skos:definition "Comments or notes about the Location." .

<http://rs.tdwg.org/dwc/terms/maximumDepthInMeters> a owl:ObjectProperty,
        meta:SlotDefinition ;
    rdfs:label "maximumDepthInMeters" ;
    rdfs:range <https://w3id.org/biolink/biolinkml/meta/types/String> ;
    skos:definition "The greater depth of a range of depth below the local surface, in meters." .

<http://rs.tdwg.org/dwc/terms/maximumDistanceAboveSurfaceInMeters> a owl:ObjectProperty,
        meta:SlotDefinition ;
    rdfs:label "maximumDistanceAboveSurfaceInMeters" ;
    rdfs:range <https://w3id.org/biolink/biolinkml/meta/types/String> ;
    skos:definition "The greater distance in a range of distance from a reference surface in the vertical direction, in meters. Use positive values for locations above the surface, negative values for locations below. If depth measures are given, the reference surface is the location given by the depth, otherwise the reference surface is the location given by the elevation." .

<http://rs.tdwg.org/dwc/terms/maximumElevationInMeters> a owl:ObjectProperty,
        meta:SlotDefinition ;
    rdfs:label "maximumElevationInMeters" ;
    rdfs:range <https://w3id.org/biolink/biolinkml/meta/types/String> ;
    skos:definition "The upper limit of the range of elevation (altitude, usually above sea level), in meters." .

<http://rs.tdwg.org/dwc/terms/minimumDepthInMeters> a owl:ObjectProperty,
        meta:SlotDefinition ;
    rdfs:label "minimumDepthInMeters" ;
    rdfs:range <https://w3id.org/biolink/biolinkml/meta/types/String> ;
    skos:definition "The lesser depth of a range of depth below the local surface, in meters." .

<http://rs.tdwg.org/dwc/terms/minimumDistanceAboveSurfaceInMeters> a owl:ObjectProperty,
        meta:SlotDefinition ;
    rdfs:label "minimumDistanceAboveSurfaceInMeters" ;
    rdfs:range <https://w3id.org/biolink/biolinkml/meta/types/String> ;
    skos:definition "The lesser distance in a range of distance from a reference surface in the vertical direction, in meters. Use positive values for locations above the surface, negative values for locations below. If depth measures are given, the reference surface is the location given by the depth, otherwise the reference surface is the location given by the elevation." .

<http://rs.tdwg.org/dwc/terms/minimumElevationInMeters> a owl:ObjectProperty,
        meta:SlotDefinition ;
    rdfs:label "minimumElevationInMeters" ;
    rdfs:range <https://w3id.org/biolink/biolinkml/meta/types/String> ;
    skos:definition "The lower limit of the range of elevation (altitude, usually above sea level), in meters." .

<http://rs.tdwg.org/dwc/terms/modified> a owl:ObjectProperty,
        meta:SlotDefinition ;
    rdfs:label "modified" ;
    rdfs:range <https://w3id.org/biolink/biolinkml/meta/types/String> ;
    skos:definition "The most recent date-time on which the resource was changed." .

<http://rs.tdwg.org/dwc/terms/municipality> a owl:ObjectProperty,
        meta:SlotDefinition ;
    rdfs:label "municipality" ;
    rdfs:range <https://w3id.org/biolink/biolinkml/meta/types/String> ;
    skos:definition "The full, unabbreviated name of the next smaller administrative region than county (city, municipality, etc.) in which the Location occurs. Do not use this term for a nearby named place that does not contain the actual location." .

<http://rs.tdwg.org/dwc/terms/ownerInstitutionCode> a owl:ObjectProperty,
        meta:SlotDefinition ;
    rdfs:label "ownerInstitutionCode" ;
    rdfs:range <https://w3id.org/biolink/biolinkml/meta/types/String> ;
    skos:definition "The name (or acronym) in use by the institution having ownership of the object(s) or information referred to in the record." .

<http://rs.tdwg.org/dwc/terms/pointRadiusSpatialFit> a owl:ObjectProperty,
        meta:SlotDefinition ;
    rdfs:label "pointRadiusSpatialFit" ;
    rdfs:range <https://w3id.org/biolink/biolinkml/meta/types/String> ;
    skos:definition "The ratio of the area of the point-radius (decimalLatitude, decimalLongitude, coordinateUncertaintyInMeters) to the area of the true (original, or most specific) spatial representation of the Location. Legal values are 0, greater than or equal to 1, or undefined. A value of 1 is an exact match or 100% overlap. A value of 0 should be used if the given point-radius does not completely contain the original representation. The pointRadiusSpatialFit is undefined (and should be left blank) if the original representation is a point without uncertainty and the given georeference is not that same point (without uncertainty). If both the original and the given georeference are the same point, the pointRadiusSpatialFit is 1." .

<http://rs.tdwg.org/dwc/terms/references> a owl:ObjectProperty,
        meta:SlotDefinition ;
    rdfs:label "references" ;
    rdfs:range <https://w3id.org/biolink/biolinkml/meta/types/String> ;
    skos:definition "A related resource that is referenced, cited, or otherwise pointed to by the described resource." .

<http://rs.tdwg.org/dwc/terms/rightsHolder> a owl:ObjectProperty,
        meta:SlotDefinition ;
    rdfs:label "rightsHolder" ;
    rdfs:range <https://w3id.org/biolink/biolinkml/meta/types/String> ;
    skos:definition "A person or organization owning or managing rights over the resource." .

<http://rs.tdwg.org/dwc/terms/source_mat_id> a owl:ObjectProperty,
        meta:SlotDefinition ;
    rdfs:label "source_mat_id" ;
    rdfs:range <https://w3id.org/biolink/biolinkml/meta/types/String> ;
    skos:definition "A unique identifier assigned to a material sample (as defined by http://rs.tdwg.org/dwc/terms/MaterialSampleID, and as opposed to a particular digital record of a material sample) used for extracting nucleic acids, and subsequent sequencing. The identifier can refer either to the original material collected or to any derived sub-samples. The INSDC qualifiers /specimen_voucher, /bio_material, or /culture_collection provide additional context and suggested syntax for this identifier for data submitted to INSDC databases." .

<http://rs.tdwg.org/dwc/terms/stateProvince> a owl:ObjectProperty,
        meta:SlotDefinition ;
    rdfs:label "stateProvince" ;
    rdfs:range <https://w3id.org/biolink/biolinkml/meta/types/String> ;
    skos:definition "The name of the next smaller administrative region than country (state, province, canton, department, region, etc.) in which the Location occurs." .

<http://rs.tdwg.org/dwc/terms/toTaxon> a owl:ObjectProperty,
        meta:SlotDefinition ;
    rdfs:label "toTaxon" ;
    rdfs:range <https://w3id.org/biolink/biolinkml/meta/types/String> ;
    skos:definition "Use to link a dwc:Identification instance subject to a taxonomic entity such as a taxon, taxon concept, or taxon name use." .

<http://rs.tdwg.org/dwc/terms/type> a owl:ObjectProperty,
        meta:SlotDefinition ;
    rdfs:label "type" ;
    rdfs:range <https://w3id.org/biolink/biolinkml/meta/types/String> ;
    skos:definition "The nature or genre of the resource." .

<http://rs.tdwg.org/dwc/terms/verbatimCoordinateSystem> a owl:ObjectProperty,
        meta:SlotDefinition ;
    rdfs:label "verbatimCoordinateSystem" ;
    rdfs:range <https://w3id.org/biolink/biolinkml/meta/types/String> ;
    skos:definition "The spatial coordinate system for the verbatimLatitude and verbatimLongitude or the verbatimCoordinates of the Location." .

<http://rs.tdwg.org/dwc/terms/verbatimCoordinates> a owl:ObjectProperty,
        meta:SlotDefinition ;
    rdfs:label "verbatimCoordinates" ;
    rdfs:range <https://w3id.org/biolink/biolinkml/meta/types/String> ;
    skos:definition "The verbatim original spatial coordinates of the Location. The coordinate ellipsoid, geodeticDatum, or full Spatial Reference System (SRS) for these coordinates should be stored in verbatimSRS and the coordinate system should be stored in verbatimCoordinateSystem." .

<http://rs.tdwg.org/dwc/terms/verbatimDepth> a owl:ObjectProperty,
        meta:SlotDefinition ;
    rdfs:label "verbatimDepth" ;
    rdfs:range <https://w3id.org/biolink/biolinkml/meta/types/String> ;
    skos:definition "The original description of the depth below the local surface." .

<http://rs.tdwg.org/dwc/terms/verbatimElevation> a owl:ObjectProperty,
        meta:SlotDefinition ;
    rdfs:label "verbatimElevation" ;
    rdfs:range <https://w3id.org/biolink/biolinkml/meta/types/String> ;
    skos:definition "The original description of the elevation (altitude, usually above sea level) of the Location." .

<http://rs.tdwg.org/dwc/terms/verbatimLatitude> a owl:ObjectProperty,
        meta:SlotDefinition ;
    rdfs:label "verbatimLatitude" ;
    rdfs:range <https://w3id.org/biolink/biolinkml/meta/types/String> ;
    skos:definition "The verbatim original latitude of the Location. The coordinate ellipsoid, geodeticDatum, or full Spatial Reference System (SRS) for these coordinates should be stored in verbatimSRS and the coordinate system should be stored in verbatimCoordinateSystem." .

<http://rs.tdwg.org/dwc/terms/verbatimLocality> a owl:ObjectProperty,
        meta:SlotDefinition ;
    rdfs:label "verbatimLocality" ;
    rdfs:range <https://w3id.org/biolink/biolinkml/meta/types/String> ;
    skos:definition "The original textual description of the place." .

<http://rs.tdwg.org/dwc/terms/verbatimLongitude> a owl:ObjectProperty,
        meta:SlotDefinition ;
    rdfs:label "verbatimLongitude" ;
    rdfs:range <https://w3id.org/biolink/biolinkml/meta/types/String> ;
    skos:definition "The verbatim original longitude of the Location. The coordinate ellipsoid, geodeticDatum, or full Spatial Reference System (SRS) for these coordinates should be stored in verbatimSRS and the coordinate system should be stored in verbatimCoordinateSystem." .

<http://rs.tdwg.org/dwc/terms/verbatimSRS> a owl:ObjectProperty,
        meta:SlotDefinition ;
    rdfs:label "verbatimSRS" ;
    rdfs:range <https://w3id.org/biolink/biolinkml/meta/types/String> ;
    skos:definition "The ellipsoid, geodetic datum, or spatial reference system (SRS) upon which coordinates given in verbatimLatitude and verbatimLongitude, or verbatimCoordinates are based." .

<http://rs.tdwg.org/dwc/terms/waterBody> a owl:ObjectProperty,
        meta:SlotDefinition ;
    rdfs:label "waterBody" ;
    rdfs:range <https://w3id.org/biolink/biolinkml/meta/types/String> ;
    skos:definition "The name of the water body in which the Location occurs." .

meta:SubsetDefinition a owl:Class ;
    rdfs:label "subset_definition" ;
    skos:definition "the name and description of a subset" .

<https://w3id.org/biolink/biolinkml/meta/types/Boolean> a owl:Class,
        meta:TypeDefinition ;
    rdfs:label "boolean" ;
    rdfs:subClassOf [ a owl:Restriction ;
            owl:onDataRange xsd:boolean ;
            owl:onProperty meta:topValue ;
            owl:qualifiedCardinality 1 ] ;
    skos:definition "A binary (true or false) value" .

<https://w3id.org/biolink/biolinkml/meta/types/Date> a owl:Class,
        meta:TypeDefinition ;
    rdfs:label "date" ;
    rdfs:subClassOf [ a owl:Restriction ;
            owl:onDataRange xsd:date ;
            owl:onProperty meta:topValue ;
            owl:qualifiedCardinality 1 ] ;
    skos:definition "a date (year, month and day) in an idealized calendar" ;
    skos:editorialNote "URI is dateTime because OWL reasoners don't work with straight date or time" .

<https://w3id.org/biolink/biolinkml/meta/types/Datetime> a owl:Class,
        meta:TypeDefinition ;
    rdfs:label "datetime" ;
    rdfs:subClassOf [ a owl:Restriction ;
            owl:onDataRange xsd:dateTime ;
            owl:onProperty meta:topValue ;
            owl:qualifiedCardinality 1 ] ;
    skos:definition "The combination of a date and time" .

<https://w3id.org/biolink/biolinkml/meta/types/Decimal> a owl:Class,
        meta:TypeDefinition ;
    rdfs:label "decimal" ;
    rdfs:subClassOf [ a owl:Restriction ;
            owl:onDataRange xsd:decimal ;
            owl:onProperty meta:topValue ;
            owl:qualifiedCardinality 1 ] ;
    skos:definition "A real number with arbitrary precision that conforms to the xsd:decimal specification" .

<https://w3id.org/biolink/biolinkml/meta/types/Double> a owl:Class,
        meta:TypeDefinition ;
    rdfs:label "double" ;
    rdfs:subClassOf [ a owl:Restriction ;
            owl:onDataRange xsd:double ;
            owl:onProperty meta:topValue ;
            owl:qualifiedCardinality 1 ] ;
    skos:definition "A real number that conforms to the xsd:double specification" .

<https://w3id.org/biolink/biolinkml/meta/types/Float> a owl:Class,
        meta:TypeDefinition ;
    rdfs:label "float" ;
    rdfs:subClassOf [ a owl:Restriction ;
            owl:onDataRange xsd:float ;
            owl:onProperty meta:topValue ;
            owl:qualifiedCardinality 1 ] ;
    skos:definition "A real number that conforms to the xsd:float specification" .

<https://w3id.org/biolink/biolinkml/meta/types/Integer> a owl:Class,
        meta:TypeDefinition ;
    rdfs:label "integer" ;
    rdfs:subClassOf [ a owl:Restriction ;
            owl:onDataRange xsd:integer ;
            owl:onProperty meta:topValue ;
            owl:qualifiedCardinality 1 ] ;
    skos:definition "An integer" .

<https://w3id.org/biolink/biolinkml/meta/types/Ncname> a owl:Class,
        meta:TypeDefinition ;
    rdfs:label "ncname" ;
    rdfs:subClassOf [ a owl:Restriction ;
            owl:onDataRange xsd:string ;
            owl:onProperty meta:topValue ;
            owl:qualifiedCardinality 1 ] ;
    skos:definition "Prefix part of CURIE" .

<https://w3id.org/biolink/biolinkml/meta/types/Nodeidentifier> a owl:Class,
        meta:TypeDefinition ;
    rdfs:label "nodeidentifier" ;
    rdfs:subClassOf [ a owl:Restriction ;
            owl:onDataRange <http://www.w3.org/ns/shex#nonLiteral> ;
            owl:onProperty meta:topValue ;
            owl:qualifiedCardinality 1 ] ;
    skos:definition "A URI, CURIE or BNODE that represents a node in a model." .

<https://w3id.org/biolink/biolinkml/meta/types/Objectidentifier> a owl:Class,
        meta:TypeDefinition ;
    rdfs:label "objectidentifier" ;
    rdfs:subClassOf [ a owl:Restriction ;
            owl:onDataRange <http://www.w3.org/ns/shex#iri> ;
            owl:onProperty meta:topValue ;
            owl:qualifiedCardinality 1 ] ;
    skos:definition "A URI or CURIE that represents an object in the model." ;
    skos:note "Used for inheritence and type checking" .

<https://w3id.org/biolink/biolinkml/meta/types/Time> a owl:Class,
        meta:TypeDefinition ;
    rdfs:label "time" ;
    rdfs:subClassOf [ a owl:Restriction ;
            owl:onDataRange xsd:dateTime ;
            owl:onProperty meta:topValue ;
            owl:qualifiedCardinality 1 ] ;
    skos:definition "A time object represents a (local) time of day, independent of any particular day" ;
    skos:editorialNote "URI is dateTime because OWL reasoners don't work with straight date or time" .

<https://w3id.org/biolink/biolinkml/meta/types/Uri> a owl:Class,
        meta:TypeDefinition ;
    rdfs:label "uri" ;
    rdfs:subClassOf [ a owl:Restriction ;
            owl:onDataRange xsd:anyURI ;
            owl:onProperty meta:topValue ;
            owl:qualifiedCardinality 1 ] ;
    skos:definition "a complete URI" .

<https://w3id.org/biolink/biolinkml/meta/types/Uriorcurie> a owl:Class,
        meta:TypeDefinition ;
    rdfs:label "uriorcurie" ;
    rdfs:subClassOf [ a owl:Restriction ;
            owl:onDataRange xsd:anyURI ;
            owl:onProperty meta:topValue ;
            owl:qualifiedCardinality 1 ] ;
    skos:definition "a URI or a CURIE" .

<http://rs.tdwg.org/dwc/terms/Accepted_Name_Usage> a owl:ObjectProperty,
        meta:SlotDefinition ;
    rdfs:label "Accepted Name Usage" ;
    rdfs:range <https://w3id.org/biolink/biolinkml/meta/types/String> ;
    skos:definition "The full name, with authorship and date information if known, of the currently valid (zoological) or accepted (botanical) taxon." .

<http://rs.tdwg.org/dwc/terms/Accepted_Name_Usage_ID> a owl:ObjectProperty,
        meta:SlotDefinition ;
    rdfs:label "Accepted Name Usage ID" ;
    rdfs:range <https://w3id.org/biolink/biolinkml/meta/types/String> ;
    skos:definition "An identifier for the name usage (documented meaning of the name according to a source) of the currently valid (zoological) or accepted (botanical) taxon." .

<http://rs.tdwg.org/dwc/terms/Associated_Media> a owl:ObjectProperty,
        meta:SlotDefinition ;
    rdfs:label "Associated Media" ;
    rdfs:range <https://w3id.org/biolink/biolinkml/meta/types/String> ;
    skos:definition "A list (concatenated and separated) of identifiers (publication, global unique identifier, URI) of media associated with the Occurrence." .

<http://rs.tdwg.org/dwc/terms/Associated_Occurrences> a owl:ObjectProperty,
        meta:SlotDefinition ;
    rdfs:label "Associated Occurrences" ;
    rdfs:range <https://w3id.org/biolink/biolinkml/meta/types/String> ;
    skos:definition "A list (concatenated and separated) of identifiers of other Occurrence records and their associations to this Occurrence." .

<http://rs.tdwg.org/dwc/terms/Associated_Organisms> a owl:ObjectProperty,
        meta:SlotDefinition ;
    rdfs:label "Associated Organisms" ;
    rdfs:range <https://w3id.org/biolink/biolinkml/meta/types/String> ;
    skos:definition "A list (concatenated and separated) of identifiers of other Organisms and their associations to this Organism." .

<http://rs.tdwg.org/dwc/terms/Associated_References> a owl:ObjectProperty,
        meta:SlotDefinition ;
    rdfs:label "Associated References" ;
    rdfs:range <https://w3id.org/biolink/biolinkml/meta/types/String> ;
    skos:definition "A list (concatenated and separated) of identifiers (publication, bibliographic reference, global unique identifier, URI) of literature associated with the Occurrence." .

<http://rs.tdwg.org/dwc/terms/Associated_Sequences> a owl:ObjectProperty,
        meta:SlotDefinition ;
    rdfs:label "Associated Sequences" ;
    rdfs:range <https://w3id.org/biolink/biolinkml/meta/types/String> ;
    skos:definition "A list (concatenated and separated) of identifiers (publication, global unique identifier, URI) of genetic sequence information associated with the Occurrence." .

<http://rs.tdwg.org/dwc/terms/Associated_Taxa> a owl:ObjectProperty,
        meta:SlotDefinition ;
    rdfs:label "Associated Taxa" ;
    rdfs:range <https://w3id.org/biolink/biolinkml/meta/types/String> ;
    skos:definition "A list (concatenated and separated) of identifiers or names of taxa and their associations with the Occurrence." .

<http://rs.tdwg.org/dwc/terms/Bed> a owl:ObjectProperty,
        meta:SlotDefinition ;
    rdfs:label "Bed" ;
    rdfs:range <https://w3id.org/biolink/biolinkml/meta/types/String> ;
    skos:definition "The full name of the lithostratigraphic bed from which the cataloged item was collected." .

<http://rs.tdwg.org/dwc/terms/Behavior> a owl:ObjectProperty,
        meta:SlotDefinition ;
    rdfs:label "Behavior" ;
    rdfs:range <https://w3id.org/biolink/biolinkml/meta/types/String> ;
    skos:definition "A description of the behavior shown by the subject at the time the Occurrence was recorded. Recommended best practice is to use a controlled vocabulary." .

<http://rs.tdwg.org/dwc/terms/Catalog_Number> a owl:ObjectProperty,
        meta:SlotDefinition ;
    rdfs:label "Catalog Number" ;
    rdfs:range <https://w3id.org/biolink/biolinkml/meta/types/String> ;
    skos:definition "An identifier (preferably unique) for the record within the data set or collection." .

<http://rs.tdwg.org/dwc/terms/Class> a owl:ObjectProperty,
        meta:SlotDefinition ;
    rdfs:label "Class" ;
    rdfs:range <https://w3id.org/biolink/biolinkml/meta/types/String> ;
    skos:definition "The name of the class in which the organism is classified." .

<http://rs.tdwg.org/dwc/terms/Date_Identified> a owl:ObjectProperty,
        meta:SlotDefinition ;
    rdfs:label "Date Identified" ;
    rdfs:range <https://w3id.org/biolink/biolinkml/meta/types/String> ;
    skos:definition "The date on which the subject was identified as representing the Taxon. Recommended best practice is to use an encoding scheme, such as ISO 8601:2004(E)." .

<http://rs.tdwg.org/dwc/terms/Day> a owl:ObjectProperty,
        meta:SlotDefinition ;
    rdfs:label "Day" ;
    rdfs:range <https://w3id.org/biolink/biolinkml/meta/types/String> ;
    skos:definition "The integer day of the month on which the Event occurred." .

<http://rs.tdwg.org/dwc/terms/Disposition> a owl:ObjectProperty,
        meta:SlotDefinition ;
    rdfs:label "Disposition" ;
    rdfs:range <https://w3id.org/biolink/biolinkml/meta/types/String> ;
    skos:definition "The current disposition of the cataloged item. Examples: \"in collection\", \"missing\", \"voucher elsewhere\", \"duplicates elsewhere\"." .

<http://rs.tdwg.org/dwc/terms/Earliest_Age_Or_Lowest_Stage> a owl:ObjectProperty,
        meta:SlotDefinition ;
    rdfs:label "Earliest Age Or Lowest Stage" ;
    rdfs:range <https://w3id.org/biolink/biolinkml/meta/types/String> ;
    skos:definition "The full name of the earliest possible geochronologic age or lowest chronostratigraphic stage attributable to the stratigraphic horizon from which the cataloged item was collected." .

<http://rs.tdwg.org/dwc/terms/Earliest_Eon_Or_Lowest_Eonothem> a owl:ObjectProperty,
        meta:SlotDefinition ;
    rdfs:label "Earliest Eon Or Lowest Eonothem" ;
    rdfs:range <https://w3id.org/biolink/biolinkml/meta/types/String> ;
    skos:definition "The full name of the earliest possible geochronologic eon or lowest chrono-stratigraphic eonothem or the informal name (\"Precambrian\") attributable to the stratigraphic horizon from which the cataloged item was collected." .

<http://rs.tdwg.org/dwc/terms/Earliest_Epoch_Or_Lowest_Series> a owl:ObjectProperty,
        meta:SlotDefinition ;
    rdfs:label "Earliest Epoch Or Lowest Series" ;
    rdfs:range <https://w3id.org/biolink/biolinkml/meta/types/String> ;
    skos:definition "The full name of the earliest possible geochronologic epoch or lowest chronostratigraphic series attributable to the stratigraphic horizon from which the cataloged item was collected." .

<http://rs.tdwg.org/dwc/terms/Earliest_Era_Or_Lowest_Erathem> a owl:ObjectProperty,
        meta:SlotDefinition ;
    rdfs:label "Earliest Era Or Lowest Erathem" ;
    rdfs:range <https://w3id.org/biolink/biolinkml/meta/types/String> ;
    skos:definition "The full name of the earliest possible geochronologic era or lowest chronostratigraphic erathem attributable to the stratigraphic horizon from which the cataloged item was collected." .

<http://rs.tdwg.org/dwc/terms/Earliest_Period_Or_Lowest_System> a owl:ObjectProperty,
        meta:SlotDefinition ;
    rdfs:label "Earliest Period Or Lowest System" ;
    rdfs:range <https://w3id.org/biolink/biolinkml/meta/types/String> ;
    skos:definition "The full name of the earliest possible geochronologic period or lowest chronostratigraphic system attributable to the stratigraphic horizon from which the cataloged item was collected." .

<http://rs.tdwg.org/dwc/terms/End_Day_Of_Year> a owl:ObjectProperty,
        meta:SlotDefinition ;
    rdfs:label "End Day Of Year" ;
    rdfs:range <https://w3id.org/biolink/biolinkml/meta/types/String> ;
    skos:definition "The latest ordinal day of the year on which the Event occurred (1 for January 1, 365 for December 31, except in a leap year, in which case it is 366)." .

<http://rs.tdwg.org/dwc/terms/Establishment_Means> a owl:ObjectProperty,
        meta:SlotDefinition ;
    rdfs:label "Establishment Means" ;
    rdfs:range <https://w3id.org/biolink/biolinkml/meta/types/String> ;
    skos:definition "The process by which the biological individual(s) represented in the Occurrence became established at the location. Recommended best practice is to use a controlled vocabulary." .

<http://rs.tdwg.org/dwc/terms/Event_Date> a owl:ObjectProperty,
        meta:SlotDefinition ;
    rdfs:label "Event Date" ;
    rdfs:range <https://w3id.org/biolink/biolinkml/meta/types/String> ;
    skos:definition "The date-time or interval during which an Event occurred. For occurrences, this is the date-time when the event was recorded. Not suitable for a time in a geological context. Recommended best practice is to use an encoding scheme, such as ISO 8601:2004(E)." .

<http://rs.tdwg.org/dwc/terms/Event_ID> a owl:ObjectProperty,
        meta:SlotDefinition ;
    rdfs:label "Event ID" ;
    rdfs:range <https://w3id.org/biolink/biolinkml/meta/types/String> ;
    skos:definition "An identifier for the set of information associated with an Event (something that occurs at a place and time). May be a global unique identifier or an identifier specific to the data set." .

<http://rs.tdwg.org/dwc/terms/Event_Remarks> a owl:ObjectProperty,
        meta:SlotDefinition ;
    rdfs:label "Event Remarks" ;
    rdfs:range <https://w3id.org/biolink/biolinkml/meta/types/String> ;
    skos:definition "Comments or notes about the Event." .

<http://rs.tdwg.org/dwc/terms/Event_Time> a owl:ObjectProperty,
        meta:SlotDefinition ;
    rdfs:label "Event Time" ;
    rdfs:range <https://w3id.org/biolink/biolinkml/meta/types/String> ;
    skos:definition "The time or interval during which an Event occurred. Recommended best practice is to use an encoding scheme, such as ISO 8601:2004(E)." .

<http://rs.tdwg.org/dwc/terms/Family> a owl:ObjectProperty,
        meta:SlotDefinition ;
    rdfs:label "Family" ;
    rdfs:range <https://w3id.org/biolink/biolinkml/meta/types/String> ;
    skos:definition "The name of the family in which the organism is classified." .

<http://rs.tdwg.org/dwc/terms/Field_Notes> a owl:ObjectProperty,
        meta:SlotDefinition ;
    rdfs:label "Field Notes" ;
    rdfs:range <https://w3id.org/biolink/biolinkml/meta/types/String> ;
    skos:definition "One of a) an indicator of the existence of, b) a reference to (publication, URI), or c) the text of notes taken in the field about the Event." .

<http://rs.tdwg.org/dwc/terms/Field_Number> a owl:ObjectProperty,
        meta:SlotDefinition ;
    rdfs:label "Field Number" ;
    rdfs:range <https://w3id.org/biolink/biolinkml/meta/types/String> ;
    skos:definition "An identifier given to the event in the field. Often serves as a link between field notes and the Event." .

<http://rs.tdwg.org/dwc/terms/Formation> a owl:ObjectProperty,
        meta:SlotDefinition ;
    rdfs:label "Formation" ;
    rdfs:range <https://w3id.org/biolink/biolinkml/meta/types/String> ;
    skos:definition "The full name of the lithostratigraphic formation from which the cataloged item was collected." .

<http://rs.tdwg.org/dwc/terms/Genus> a owl:ObjectProperty,
        meta:SlotDefinition ;
    rdfs:label "Genus" ;
    rdfs:range <https://w3id.org/biolink/biolinkml/meta/types/String> ;
    skos:definition "The name of the genus in which the organism is classified." .

<http://rs.tdwg.org/dwc/terms/Geological_Context_ID> a owl:ObjectProperty,
        meta:SlotDefinition ;
    rdfs:label "Geological Context ID" ;
    rdfs:range <https://w3id.org/biolink/biolinkml/meta/types/String> ;
    skos:definition "An identifier for the set of information associated with a GeologicalContext (the location within a geological context, such as stratigraphy). May be a global unique identifier or an identifier specific to the data set." .

<http://rs.tdwg.org/dwc/terms/Group> a owl:ObjectProperty,
        meta:SlotDefinition ;
    rdfs:label "Group" ;
    rdfs:range <https://w3id.org/biolink/biolinkml/meta/types/String> ;
    skos:definition "The full name of the lithostratigraphic group from which the cataloged item was collected." .

<http://rs.tdwg.org/dwc/terms/Habitat> a owl:ObjectProperty,
        meta:SlotDefinition ;
    rdfs:label "Habitat" ;
    rdfs:range <https://w3id.org/biolink/biolinkml/meta/types/String> ;
    skos:definition "A category or description of the habitat in which the Event occurred." .

<http://rs.tdwg.org/dwc/terms/Higher_Classification> a owl:ObjectProperty,
        meta:SlotDefinition ;
    rdfs:label "Higher Classification" ;
    rdfs:range <https://w3id.org/biolink/biolinkml/meta/types/String> ;
    skos:definition "A list (concatenated and separated) of taxa names terminating at the rank immediately superior to the taxon referenced in the taxon record." .

<http://rs.tdwg.org/dwc/terms/Highest_Biostratigraphic_Zone> a owl:ObjectProperty,
        meta:SlotDefinition ;
    rdfs:label "Highest Biostratigraphic Zone" ;
    rdfs:range <https://w3id.org/biolink/biolinkml/meta/types/String> ;
    skos:definition "The full name of the highest possible geological biostratigraphic zone of the stratigraphic horizon from which the cataloged item was collected." .

<http://rs.tdwg.org/dwc/terms/Identification_ID> a owl:ObjectProperty,
        meta:SlotDefinition ;
    rdfs:label "Identification ID" ;
    rdfs:range <https://w3id.org/biolink/biolinkml/meta/types/String> ;
    skos:definition "An identifier for the Identification (the body of information associated with the assignment of a scientific name). May be a global unique identifier or an identifier specific to the data set." .

<http://rs.tdwg.org/dwc/terms/Identification_Qualifier> a owl:ObjectProperty,
        meta:SlotDefinition ;
    rdfs:label "Identification Qualifier" ;
    rdfs:range <https://w3id.org/biolink/biolinkml/meta/types/String> ;
    skos:definition "A brief phrase or a standard term (\"cf.\", \"aff.\") to express the determiner's doubts about the Identification." .

<http://rs.tdwg.org/dwc/terms/Identification_References> a owl:ObjectProperty,
        meta:SlotDefinition ;
    rdfs:label "Identification References" ;
    rdfs:range <https://w3id.org/biolink/biolinkml/meta/types/String> ;
    skos:definition "A list (concatenated and separated) of references (publication, global unique identifier, URI) used in the Identification." .

<http://rs.tdwg.org/dwc/terms/Identification_Remarks> a owl:ObjectProperty,
        meta:SlotDefinition ;
    rdfs:label "Identification Remarks" ;
    rdfs:range <https://w3id.org/biolink/biolinkml/meta/types/String> ;
    skos:definition "Comments or notes about the Identification." .

<http://rs.tdwg.org/dwc/terms/Identification_Verification_Status> a owl:ObjectProperty,
        meta:SlotDefinition ;
    rdfs:label "Identification Verification Status" ;
    rdfs:range <https://w3id.org/biolink/biolinkml/meta/types/String> ;
    skos:definition "A categorical indicator of the extent to which the taxonomic identification has been verified to be correct. Recommended best practice is to use a controlled vocabulary such as that used in HISPID/ABCD." .

<http://rs.tdwg.org/dwc/terms/Identified_By> a owl:ObjectProperty,
        meta:SlotDefinition ;
    rdfs:label "Identified By" ;
    rdfs:range <https://w3id.org/biolink/biolinkml/meta/types/String> ;
    skos:definition "A list (concatenated and separated) of names of people, groups, or organizations who assigned the Taxon to the subject." .

<http://rs.tdwg.org/dwc/terms/Individual_Count> a owl:ObjectProperty,
        meta:SlotDefinition ;
    rdfs:label "Individual Count" ;
    rdfs:range <https://w3id.org/biolink/biolinkml/meta/types/String> ;
    skos:definition "The number of individuals represented present at the time of the Occurrence." .

<http://rs.tdwg.org/dwc/terms/Infraspecific_Epithet> a owl:ObjectProperty,
        meta:SlotDefinition ;
    rdfs:label "Infraspecific Epithet" ;
    rdfs:range <https://w3id.org/biolink/biolinkml/meta/types/String> ;
    skos:definition "The name of the lowest or terminal infraspecific epithet of the scientificName, excluding any rank designation." .

<http://rs.tdwg.org/dwc/terms/Kingdom> a owl:ObjectProperty,
        meta:SlotDefinition ;
    rdfs:label "Kingdom" ;
    rdfs:range <https://w3id.org/biolink/biolinkml/meta/types/String> ;
    skos:definition "The name of the kingdom in which the organism is classified." .

<http://rs.tdwg.org/dwc/terms/Latest_AgeOr_Highest_Stage> a owl:ObjectProperty,
        meta:SlotDefinition ;
    rdfs:label "Latest AgeOr Highest Stage" ;
    rdfs:range <https://w3id.org/biolink/biolinkml/meta/types/String> ;
    skos:definition "The full name of the latest possible geochronologic age or highest chronostratigraphic stage attributable to the stratigraphic horizon from which the cataloged item was collected." .

<http://rs.tdwg.org/dwc/terms/Latest_Eon_Or_Highest_Eonothem> a owl:ObjectProperty,
        meta:SlotDefinition ;
    rdfs:label "Latest Eon Or Highest Eonothem" ;
    rdfs:range <https://w3id.org/biolink/biolinkml/meta/types/String> ;
    skos:definition "The full name of the latest possible geochronologic eon or highest chrono-stratigraphic eonothem or the informal name (\"Precambrian\") attributable to the stratigraphic horizon from which the cataloged item was collected." .

<http://rs.tdwg.org/dwc/terms/Latest_Epoch_Or_Highest_Series> a owl:ObjectProperty,
        meta:SlotDefinition ;
    rdfs:label "Latest Epoch Or Highest Series" ;
    rdfs:range <https://w3id.org/biolink/biolinkml/meta/types/String> ;
    skos:definition "The full name of the latest possible geochronologic epoch or highest chronostratigraphic series attributable to the stratigraphic horizon from which the cataloged item was collected." .

<http://rs.tdwg.org/dwc/terms/Latest_Era_Or_Highest_Erathem> a owl:ObjectProperty,
        meta:SlotDefinition ;
    rdfs:label "Latest Era Or Highest Erathem" ;
    rdfs:range <https://w3id.org/biolink/biolinkml/meta/types/String> ;
    skos:definition "The full name of the latest possible geochronologic era or highest chronostratigraphic erathem attributable to the stratigraphic horizon from which the cataloged item was collected." .

<http://rs.tdwg.org/dwc/terms/Latest_Period_Or_Highest_System> a owl:ObjectProperty,
        meta:SlotDefinition ;
    rdfs:label "Latest Period Or Highest System" ;
    rdfs:range <https://w3id.org/biolink/biolinkml/meta/types/String> ;
    skos:definition "The full name of the latest possible geochronologic period or highest chronostratigraphic system attributable to the stratigraphic horizon from which the cataloged item was collected." .

<http://rs.tdwg.org/dwc/terms/Life_Stage> a owl:ObjectProperty,
        meta:SlotDefinition ;
    rdfs:label "Life Stage" ;
    rdfs:range <https://w3id.org/biolink/biolinkml/meta/types/String> ;
    skos:definition "The age class or life stage of the biological individual(s) at the time the Occurrence was recorded. Recommended best practice is to use a controlled vocabulary." .

<http://rs.tdwg.org/dwc/terms/Lithostratigraphic_Terms> a owl:ObjectProperty,
        meta:SlotDefinition ;
    rdfs:label "Lithostratigraphic Terms" ;
    rdfs:range <https://w3id.org/biolink/biolinkml/meta/types/String> ;
    skos:definition "The combination of all litho-stratigraphic names for the rock from which the cataloged item was collected." .

<http://rs.tdwg.org/dwc/terms/Lowest_Biostratigraphic_Zone> a owl:ObjectProperty,
        meta:SlotDefinition ;
    rdfs:label "Lowest Biostratigraphic Zone" ;
    rdfs:range <https://w3id.org/biolink/biolinkml/meta/types/String> ;
    skos:definition "The full name of the lowest possible geological biostratigraphic zone of the stratigraphic horizon from which the cataloged item was collected." .

<http://rs.tdwg.org/dwc/terms/Material_Sample_ID> a owl:ObjectProperty,
        meta:SlotDefinition ;
    rdfs:label "Material Sample ID" ;
    rdfs:range <https://w3id.org/biolink/biolinkml/meta/types/String> ;
    skos:definition "An identifier for the MaterialSample (as opposed to a particular digital record of the material sample). In the absence of a persistent global unique identifier, construct one from a combination of identifiers in the record that will most closely make the materialSampleID globally unique." .

<http://rs.tdwg.org/dwc/terms/Measurement_Accuracy> a owl:ObjectProperty,
        meta:SlotDefinition ;
    rdfs:label "Measurement Accuracy" ;
    rdfs:range <https://w3id.org/biolink/biolinkml/meta/types/String> ;
    skos:definition "The description of the potential error associated with the measurementValue." .

<http://rs.tdwg.org/dwc/terms/Measurement_Determined_By> a owl:ObjectProperty,
        meta:SlotDefinition ;
    rdfs:label "Measurement Determined By" ;
    rdfs:range <https://w3id.org/biolink/biolinkml/meta/types/String> ;
    skos:definition "A list (concatenated and separated) of names of people, groups, or organizations who determined the value of the MeasurementOrFact." .

<http://rs.tdwg.org/dwc/terms/Measurement_Determined_Date> a owl:ObjectProperty,
        meta:SlotDefinition ;
    rdfs:label "Measurement Determined Date" ;
    rdfs:range <https://w3id.org/biolink/biolinkml/meta/types/String> ;
    skos:definition "The date on which the MeasurementOrFact was made. Recommended best practice is to use an encoding scheme, such as ISO 8601:2004(E)." .

<http://rs.tdwg.org/dwc/terms/Measurement_ID> a owl:ObjectProperty,
        meta:SlotDefinition ;
    rdfs:label "Measurement ID" ;
    rdfs:range <https://w3id.org/biolink/biolinkml/meta/types/String> ;
    skos:definition "An identifier for the MeasurementOrFact (information pertaining to measurements, facts, characteristics, or assertions). May be a global unique identifier or an identifier specific to the data set." .

<http://rs.tdwg.org/dwc/terms/Measurement_Method> a owl:ObjectProperty,
        meta:SlotDefinition ;
    rdfs:label "Measurement Method" ;
    rdfs:range <https://w3id.org/biolink/biolinkml/meta/types/String> ;
    skos:definition "A description of or reference to (publication, URI) the method or protocol used to determine the measurement, fact, characteristic, or assertion." .

<http://rs.tdwg.org/dwc/terms/Measurement_Remarks> a owl:ObjectProperty,
        meta:SlotDefinition ;
    rdfs:label "Measurement Remarks" ;
    rdfs:range <https://w3id.org/biolink/biolinkml/meta/types/String> ;
    skos:definition "Comments or notes accompanying the MeasurementOrFact." .

<http://rs.tdwg.org/dwc/terms/Measurement_Type> a owl:ObjectProperty,
        meta:SlotDefinition ;
    rdfs:label "Measurement Type" ;
    rdfs:range <https://w3id.org/biolink/biolinkml/meta/types/String> ;
    skos:definition "The nature of the measurement, fact, characteristic, or assertion. Recommended best practice is to use a controlled vocabulary." .

<http://rs.tdwg.org/dwc/terms/Measurement_Unit> a owl:ObjectProperty,
        meta:SlotDefinition ;
    rdfs:label "Measurement Unit" ;
    rdfs:range <https://w3id.org/biolink/biolinkml/meta/types/String> ;
    skos:definition "The units associated with the measurementValue. Recommended best practice is to use the International System of Units (SI)." .

<http://rs.tdwg.org/dwc/terms/Measurement_Value> a owl:ObjectProperty,
        meta:SlotDefinition ;
    rdfs:label "Measurement Value" ;
    rdfs:range <https://w3id.org/biolink/biolinkml/meta/types/String> ;
    skos:definition "The value of the measurement, fact, characteristic, or assertion." .

<http://rs.tdwg.org/dwc/terms/Member> a owl:ObjectProperty,
        meta:SlotDefinition ;
    rdfs:label "Member" ;
    rdfs:range <https://w3id.org/biolink/biolinkml/meta/types/String> ;
    skos:definition "The full name of the lithostratigraphic member from which the cataloged item was collected." .

<http://rs.tdwg.org/dwc/terms/Month> a owl:ObjectProperty,
        meta:SlotDefinition ;
    rdfs:label "Month" ;
    rdfs:range <https://w3id.org/biolink/biolinkml/meta/types/String> ;
    skos:definition "The ordinal month in which the Event occurred." .

<http://rs.tdwg.org/dwc/terms/Name_According_To> a owl:ObjectProperty,
        meta:SlotDefinition ;
    rdfs:label "Name According To" ;
    rdfs:range <https://w3id.org/biolink/biolinkml/meta/types/String> ;
    skos:definition "The reference to the source in which the specific taxon concept circumscription is defined or implied - traditionally signified by the Latin \"sensu\" or \"sec.\" (from secundum, meaning \"according to\"). For taxa that result from identifications, a reference to the keys, monographs, experts and other sources should be given." .

<http://rs.tdwg.org/dwc/terms/Name_According_To_ID> a owl:ObjectProperty,
        meta:SlotDefinition ;
    rdfs:label "Name According To ID" ;
    rdfs:range <https://w3id.org/biolink/biolinkml/meta/types/String> ;
    skos:definition "An identifier for the source in which the specific taxon concept circumscription is defined or implied. See nameAccordingTo." .

<http://rs.tdwg.org/dwc/terms/Name_Published_In> a owl:ObjectProperty,
        meta:SlotDefinition ;
    rdfs:label "Name Published In" ;
    rdfs:range <https://w3id.org/biolink/biolinkml/meta/types/String> ;
    skos:definition "A reference for the publication in which the scientificName was originally established under the rules of the associated nomenclaturalCode." .

<http://rs.tdwg.org/dwc/terms/Name_Published_In_ID> a owl:ObjectProperty,
        meta:SlotDefinition ;
    rdfs:label "Name Published In ID" ;
    rdfs:range <https://w3id.org/biolink/biolinkml/meta/types/String> ;
    skos:definition "An identifier for the publication in which the scientificName was originally established under the rules of the associated nomenclaturalCode." .

<http://rs.tdwg.org/dwc/terms/Name_Published_In_Year> a owl:ObjectProperty,
        meta:SlotDefinition ;
    rdfs:label "Name Published In Year" ;
    rdfs:range <https://w3id.org/biolink/biolinkml/meta/types/String> ;
    skos:definition "The four-digit year in which the scientificName was published." .

<http://rs.tdwg.org/dwc/terms/Nomenclatural_Code> a owl:ObjectProperty,
        meta:SlotDefinition ;
    rdfs:label "Nomenclatural Code" ;
    rdfs:range <https://w3id.org/biolink/biolinkml/meta/types/String> ;
    skos:definition "The nomenclatural code (or codes in the case of an ambiregnal name) under which the scientificName is constructed. Recommended best practice is to use a controlled vocabulary." .

<http://rs.tdwg.org/dwc/terms/Nomenclatural_Status> a owl:ObjectProperty,
        meta:SlotDefinition ;
    rdfs:label "Nomenclatural Status" ;
    rdfs:range <https://w3id.org/biolink/biolinkml/meta/types/String> ;
    skos:definition "The status related to the original publication of the name and its conformance to the relevant rules of nomenclature. It is based essentially on an algorithm according to the business rules of the code. It requires no taxonomic opinion." .

<http://rs.tdwg.org/dwc/terms/Occurrence_ID> a owl:ObjectProperty,
        meta:SlotDefinition ;
    rdfs:label "Occurrence ID" ;
    rdfs:range <https://w3id.org/biolink/biolinkml/meta/types/String> ;
    skos:definition "An identifier for the Occurrence (as opposed to a particular digital record of the occurrence). In the absence of a persistent global unique identifier, construct one from a combination of identifiers in the record that will most closely make the occurrenceID globally unique." .

<http://rs.tdwg.org/dwc/terms/Occurrence_Remarks> a owl:ObjectProperty,
        meta:SlotDefinition ;
    rdfs:label "Occurrence Remarks" ;
    rdfs:range <https://w3id.org/biolink/biolinkml/meta/types/String> ;
    skos:definition "Comments or notes about the Occurrence." .

<http://rs.tdwg.org/dwc/terms/Occurrence_Status> a owl:ObjectProperty,
        meta:SlotDefinition ;
    rdfs:label "Occurrence Status" ;
    rdfs:range <https://w3id.org/biolink/biolinkml/meta/types/String> ;
    skos:definition "A statement about the presence or absence of a Taxon at a Location. Recommended best practice is to use a controlled vocabulary." .

<http://rs.tdwg.org/dwc/terms/Order> a owl:ObjectProperty,
        meta:SlotDefinition ;
    rdfs:label "Order" ;
    rdfs:range <https://w3id.org/biolink/biolinkml/meta/types/String> ;
    skos:definition "The name of the order in which the organism is classified." .

<http://rs.tdwg.org/dwc/terms/Organism_ID> a owl:ObjectProperty,
        meta:SlotDefinition ;
    rdfs:label "Organism ID" ;
    rdfs:range <https://w3id.org/biolink/biolinkml/meta/types/String> ;
    skos:definition "An identifier for the Organism instance (as opposed to a particular digital record of the Organism). May be a globally unique identifier or an identifier specific to the data set." .

<http://rs.tdwg.org/dwc/terms/Organism_Name> a owl:ObjectProperty,
        meta:SlotDefinition ;
    rdfs:label "Organism Name" ;
    rdfs:range <https://w3id.org/biolink/biolinkml/meta/types/String> ;
    skos:definition "A textual name or label assigned to an Organism instance." .

<http://rs.tdwg.org/dwc/terms/Organism_Quantity> a owl:ObjectProperty,
        meta:SlotDefinition ;
    rdfs:label "Organism Quantity" ;
    rdfs:range <https://w3id.org/biolink/biolinkml/meta/types/String> ;
    skos:definition "A number or enumeration value for the quantity of organisms." .

<http://rs.tdwg.org/dwc/terms/Organism_Quantity_Type> a owl:ObjectProperty,
        meta:SlotDefinition ;
    rdfs:label "Organism Quantity Type" ;
    rdfs:range <https://w3id.org/biolink/biolinkml/meta/types/String> ;
    skos:definition "The type of quantification system used for the quantity of organisms." .

<http://rs.tdwg.org/dwc/terms/Organism_Remarks> a owl:ObjectProperty,
        meta:SlotDefinition ;
    rdfs:label "Organism Remarks" ;
    rdfs:range <https://w3id.org/biolink/biolinkml/meta/types/String> ;
    skos:definition "Comments or notes about the Organism instance." .

<http://rs.tdwg.org/dwc/terms/Organism_Scope> a owl:ObjectProperty,
        meta:SlotDefinition ;
    rdfs:label "Organism Scope" ;
    rdfs:range <https://w3id.org/biolink/biolinkml/meta/types/String> ;
    skos:definition "A description of the kind of Organism instance. Can be used to indicate whether the Organism instance represents a discrete organism or if it represents a particular type of aggregation. Recommended best practice is to use a controlled vocabulary." .

<http://rs.tdwg.org/dwc/terms/Original_Name_Usage> a owl:ObjectProperty,
        meta:SlotDefinition ;
    rdfs:label "Original Name Usage" ;
    rdfs:range <https://w3id.org/biolink/biolinkml/meta/types/String> ;
    skos:definition "The taxon name, with authorship and date information if known, as it originally appeared when first established under the rules of the associated nomenclaturalCode. The basionym (botany) or basonym (bacteriology) of the scientificName or the senior/earlier homonym for replaced names." .

<http://rs.tdwg.org/dwc/terms/Original_Name_Usage_ID> a owl:ObjectProperty,
        meta:SlotDefinition ;
    rdfs:label "Original Name Usage ID" ;
    rdfs:range <https://w3id.org/biolink/biolinkml/meta/types/String> ;
    skos:definition "An identifier for the name usage (documented meaning of the name according to a source) in which the terminal element of the scientificName was originally established under the rules of the associated nomenclaturalCode." .

<http://rs.tdwg.org/dwc/terms/Other_Catalog_Numbers> a owl:ObjectProperty,
        meta:SlotDefinition ;
    rdfs:label "Other Catalog Numbers" ;
    rdfs:range <https://w3id.org/biolink/biolinkml/meta/types/String> ;
    skos:definition "A list (concatenated and separated) of previous or alternate fully qualified catalog numbers or other human-used identifiers for the same Occurrence, whether in the current or any other data set or collection." .

<http://rs.tdwg.org/dwc/terms/Parent_Event_ID> a owl:ObjectProperty,
        meta:SlotDefinition ;
    rdfs:label "Parent Event ID" ;
    rdfs:range <https://w3id.org/biolink/biolinkml/meta/types/String> ;
    skos:definition "An identifier for the broader Event that groups this and potentially other Events." .

<http://rs.tdwg.org/dwc/terms/Parent_Name_Usage> a owl:ObjectProperty,
        meta:SlotDefinition ;
    rdfs:label "Parent Name Usage" ;
    rdfs:range <https://w3id.org/biolink/biolinkml/meta/types/String> ;
    skos:definition "The full name, with authorship and date information if known, of the direct, most proximate higher-rank parent taxon (in a classification) of the most specific element of the scientificName." .

<http://rs.tdwg.org/dwc/terms/Parent_Name_Usage_ID> a owl:ObjectProperty,
        meta:SlotDefinition ;
    rdfs:label "Parent Name Usage ID" ;
    rdfs:range <https://w3id.org/biolink/biolinkml/meta/types/String> ;
    skos:definition "An identifier for the name usage (documented meaning of the name according to a source) of the direct, most proximate higher-rank parent taxon (in a classification) of the most specific element of the scientificName." .

<http://rs.tdwg.org/dwc/terms/Phylum> a owl:ObjectProperty,
        meta:SlotDefinition ;
    rdfs:label "Phylum" ;
    rdfs:range <https://w3id.org/biolink/biolinkml/meta/types/String> ;
    skos:definition "The name of the phylum (or division) in which the organism is classified." .

<http://rs.tdwg.org/dwc/terms/Preparations> a owl:ObjectProperty,
        meta:SlotDefinition ;
    rdfs:label "Preparations" ;
    rdfs:range <https://w3id.org/biolink/biolinkml/meta/types/String> ;
    skos:definition "A concatenated list of preparations and preservation methods (skin, skull, skeleton, whole animal (ETOH), slide, etc.) for the cataloged item." .

<http://rs.tdwg.org/dwc/terms/Previous_Identifications> a owl:ObjectProperty,
        meta:SlotDefinition ;
    rdfs:label "Previous Identifications" ;
    rdfs:range <https://w3id.org/biolink/biolinkml/meta/types/String> ;
    skos:definition "A list (concatenated and separated) of previous assignments of names to the Organism." .

<http://rs.tdwg.org/dwc/terms/Record_Number> a owl:ObjectProperty,
        meta:SlotDefinition ;
    rdfs:label "Record Number" ;
    rdfs:range <https://w3id.org/biolink/biolinkml/meta/types/String> ;
    skos:definition "An identifier given to the Occurrence at the time it was recorded. Often serves as a link between field notes and an Occurrence record, such as a specimen collector's number." .

<http://rs.tdwg.org/dwc/terms/Recorded_By> a owl:ObjectProperty,
        meta:SlotDefinition ;
    rdfs:label "Recorded By" ;
    rdfs:range <https://w3id.org/biolink/biolinkml/meta/types/String> ;
    skos:definition "A list (concatenated and separated) of names of people, groups, or organizations responsible for recording the original Occurrence. The primary collector or observer, especially one who applies a personal identifier (recordNumber), should be listed first." .

<http://rs.tdwg.org/dwc/terms/Related_Resource_ID> a owl:ObjectProperty,
        meta:SlotDefinition ;
    rdfs:label "Related Resource ID" ;
    rdfs:range <https://w3id.org/biolink/biolinkml/meta/types/String> ;
    skos:definition "An identifier for a related resource (the object, rather than the subject of the relationship)." .

<http://rs.tdwg.org/dwc/terms/Relationship_According_To> a owl:ObjectProperty,
        meta:SlotDefinition ;
    rdfs:label "Relationship According To" ;
    rdfs:range <https://w3id.org/biolink/biolinkml/meta/types/String> ;
    skos:definition "The source (person, organization, publication, reference) establishing the relationship between the two resources." .

<http://rs.tdwg.org/dwc/terms/Relationship_Established_Date> a owl:ObjectProperty,
        meta:SlotDefinition ;
    rdfs:label "Relationship Established Date" ;
    rdfs:range <https://w3id.org/biolink/biolinkml/meta/types/String> ;
    skos:definition "The date-time on which the relationship between the two resources was established. Recommended best practice is to use an encoding scheme, such as ISO 8601:2004(E)." .

<http://rs.tdwg.org/dwc/terms/Relationship_Of_Resource> a owl:ObjectProperty,
        meta:SlotDefinition ;
    rdfs:label "Relationship Of Resource" ;
    rdfs:range <https://w3id.org/biolink/biolinkml/meta/types/String> ;
    skos:definition "The relationship of the resource identified by relatedResourceID to the subject (optionally identified by the resourceID). Recommended best practice is to use a controlled vocabulary." .

<http://rs.tdwg.org/dwc/terms/Relationship_Remarks> a owl:ObjectProperty,
        meta:SlotDefinition ;
    rdfs:label "Relationship Remarks" ;
    rdfs:range <https://w3id.org/biolink/biolinkml/meta/types/String> ;
    skos:definition "Comments or notes about the relationship between the two resources." .

<http://rs.tdwg.org/dwc/terms/Reproductive_Condition> a owl:ObjectProperty,
        meta:SlotDefinition ;
    rdfs:label "Reproductive Condition" ;
    rdfs:range <https://w3id.org/biolink/biolinkml/meta/types/String> ;
    skos:definition "The reproductive condition of the biological individual(s) represented in the Occurrence. Recommended best practice is to use a controlled vocabulary." .

<http://rs.tdwg.org/dwc/terms/Resource_ID> a owl:ObjectProperty,
        meta:SlotDefinition ;
    rdfs:label "Resource ID" ;
    rdfs:range <https://w3id.org/biolink/biolinkml/meta/types/String> ;
    skos:definition "An identifier for the resource that is the subject of the relationship." .

<http://rs.tdwg.org/dwc/terms/Resource_Relationship_ID> a owl:ObjectProperty,
        meta:SlotDefinition ;
    rdfs:label "Resource Relationship ID" ;
    rdfs:range <https://w3id.org/biolink/biolinkml/meta/types/String> ;
    skos:definition "An identifier for an instance of relationship between one resource (the subject) and another (relatedResource, the object)." .

<http://rs.tdwg.org/dwc/terms/Sample_Size_Unit> a owl:ObjectProperty,
        meta:SlotDefinition ;
    rdfs:label "Sample Size Unit" ;
    rdfs:range <https://w3id.org/biolink/biolinkml/meta/types/String> ;
    skos:definition "The unit of measurement of the size (time duration, length, area, or volume) of a sample in a sampling event." .

<http://rs.tdwg.org/dwc/terms/Sample_Size_Value> a owl:ObjectProperty,
        meta:SlotDefinition ;
    rdfs:label "Sample Size Value" ;
    rdfs:range <https://w3id.org/biolink/biolinkml/meta/types/String> ;
    skos:definition "A numeric value for a measurement of the size (time duration, length, area, or volume) of a sample in a sampling event." .

<http://rs.tdwg.org/dwc/terms/Sampling_Effort> a owl:ObjectProperty,
        meta:SlotDefinition ;
    rdfs:label "Sampling Effort" ;
    rdfs:range <https://w3id.org/biolink/biolinkml/meta/types/String> ;
    skos:definition "The amount of effort expended during an Event." .

<http://rs.tdwg.org/dwc/terms/Sampling_Protocol> a owl:ObjectProperty,
        meta:SlotDefinition ;
    rdfs:label "Sampling Protocol" ;
    rdfs:range <https://w3id.org/biolink/biolinkml/meta/types/String> ;
    skos:definition "The name of, reference to, or description of the method or protocol used during an Event." .

<http://rs.tdwg.org/dwc/terms/Scientific_Name> a owl:ObjectProperty,
        meta:SlotDefinition ;
    rdfs:label "Scientific Name" ;
    rdfs:range <https://w3id.org/biolink/biolinkml/meta/types/String> ;
    skos:definition "The full scientific name, with authorship and date information if known. When forming part of an Identification, this should be the name in lowest level taxonomic rank that can be determined. This term should not contain identification qualifications, which should instead be supplied in the IdentificationQualifier term." .

<http://rs.tdwg.org/dwc/terms/Scientific_Name_Authorship> a owl:ObjectProperty,
        meta:SlotDefinition ;
    rdfs:label "Scientific Name Authorship" ;
    rdfs:range <https://w3id.org/biolink/biolinkml/meta/types/String> ;
    skos:definition "The authorship information for the scientificName formatted according to the conventions of the applicable nomenclaturalCode." .

<http://rs.tdwg.org/dwc/terms/Scientific_Name_ID> a owl:ObjectProperty,
        meta:SlotDefinition ;
    rdfs:label "Scientific Name ID" ;
    rdfs:range <https://w3id.org/biolink/biolinkml/meta/types/String> ;
    skos:definition "An identifier for the nomenclatural (not taxonomic) details of a scientific name." .

<http://rs.tdwg.org/dwc/terms/Sex> a owl:ObjectProperty,
        meta:SlotDefinition ;
    rdfs:label "Sex" ;
    rdfs:range <https://w3id.org/biolink/biolinkml/meta/types/String> ;
    skos:definition "The sex of the biological individual represented by the cataloged object or observation. Examples: \"male\", \"female\", \"hermaphrodite\", \"gynandromorph\", \"monoecious\", \"dioecious\", \"not recorded\", \"indeterminate\", \"transitional\"." .

<http://rs.tdwg.org/dwc/terms/Specific_Epithet> a owl:ObjectProperty,
        meta:SlotDefinition ;
    rdfs:label "Specific Epithet" ;
    rdfs:range <https://w3id.org/biolink/biolinkml/meta/types/String> ;
    skos:definition "The name of the first or species epithet of the scientificName." .

<http://rs.tdwg.org/dwc/terms/Start_Day_Of_Year> a owl:ObjectProperty,
        meta:SlotDefinition ;
    rdfs:label "Start Day Of Year" ;
    rdfs:range <https://w3id.org/biolink/biolinkml/meta/types/String> ;
    skos:definition "The earliest ordinal day of the year on which the Event occurred (1 for January 1, 365 for December 31, except in a leap year, in which case it is 366)." .

<http://rs.tdwg.org/dwc/terms/Subgenus> a owl:ObjectProperty,
        meta:SlotDefinition ;
    rdfs:label "Subgenus" ;
    rdfs:range <https://w3id.org/biolink/biolinkml/meta/types/String> ;
    skos:definition "The full scientific name of the subgenus in which the taxon is classified. Values should include the genus to avoid homonym confusion." .

<http://rs.tdwg.org/dwc/terms/Taxon_Concept_ID> a owl:ObjectProperty,
        meta:SlotDefinition ;
    rdfs:label "Taxon Concept ID" ;
    rdfs:range <https://w3id.org/biolink/biolinkml/meta/types/String> ;
    skos:definition "An identifier for the taxonomic concept to which the record refers - not for the nomenclatural details of a taxon." .

<http://rs.tdwg.org/dwc/terms/Taxon_ID> a owl:ObjectProperty,
        meta:SlotDefinition ;
    rdfs:label "Taxon ID" ;
    rdfs:range <https://w3id.org/biolink/biolinkml/meta/types/String> ;
    skos:definition "An identifier for the set of taxon information (data associated with the Taxon class). May be a global unique identifier or an identifier specific to the data set." .

<http://rs.tdwg.org/dwc/terms/Taxon_Rank> a owl:ObjectProperty,
        meta:SlotDefinition ;
    rdfs:label "Taxon Rank" ;
    rdfs:range <https://w3id.org/biolink/biolinkml/meta/types/String> ;
    skos:definition "The taxonomic rank of the most specific name in the scientificName. Recommended best practice is to use a controlled vocabulary." .

<http://rs.tdwg.org/dwc/terms/Taxon_Remarks> a owl:ObjectProperty,
        meta:SlotDefinition ;
    rdfs:label "Taxon Remarks" ;
    rdfs:range <https://w3id.org/biolink/biolinkml/meta/types/String> ;
    skos:definition "Comments or notes about the taxon or name." .

<http://rs.tdwg.org/dwc/terms/Taxonomic_Status> a owl:ObjectProperty,
        meta:SlotDefinition ;
    rdfs:label "Taxonomic Status" ;
    rdfs:range <https://w3id.org/biolink/biolinkml/meta/types/String> ;
    skos:definition "The status of the use of the scientificName as a label for a taxon. Requires taxonomic opinion to define the scope of a taxon. Rules of priority then are used to define the taxonomic status of the nomenclature contained in that scope, combined with the experts opinion. It must be linked to a specific taxonomic reference that defines the concept. Recommended best practice is to use a controlled vocabulary." .

<http://rs.tdwg.org/dwc/terms/Type_Status> a owl:ObjectProperty,
        meta:SlotDefinition ;
    rdfs:label "Type Status" ;
    rdfs:range <https://w3id.org/biolink/biolinkml/meta/types/String> ;
    skos:definition "A list (concatenated and separated) of nomenclatural types (type status, typified scientific name, publication) applied to the subject." .

<http://rs.tdwg.org/dwc/terms/Verbatim_EventDate> a owl:ObjectProperty,
        meta:SlotDefinition ;
    rdfs:label "Verbatim EventDate" ;
    rdfs:range <https://w3id.org/biolink/biolinkml/meta/types/String> ;
    skos:definition "The verbatim original representation of the date and time information for an Event." .

<http://rs.tdwg.org/dwc/terms/Verbatim_Taxon_Rank> a owl:ObjectProperty,
        meta:SlotDefinition ;
    rdfs:label "Verbatim Taxon Rank" ;
    rdfs:range <https://w3id.org/biolink/biolinkml/meta/types/String> ;
    skos:definition "The taxonomic rank of the most specific name in the scientificName as it appears in the original record." .

<http://rs.tdwg.org/dwc/terms/Vernacular_Name> a owl:ObjectProperty,
        meta:SlotDefinition ;
    rdfs:label "Vernacular Name" ;
    rdfs:range <https://w3id.org/biolink/biolinkml/meta/types/String> ;
    skos:definition "A common or vernacular name." .

<http://rs.tdwg.org/dwc/terms/Year> a owl:ObjectProperty,
        meta:SlotDefinition ;
    rdfs:label "Year" ;
    rdfs:range <https://w3id.org/biolink/biolinkml/meta/types/String> ;
    skos:definition "The four-digit year in which the Event occurred, according to the Common Era Calendar." .

<http://rs.tdwg.org/dwc/terms/acceptedNameUsage> a owl:ObjectProperty,
        meta:SlotDefinition ;
    rdfs:label "acceptedNameUsage" ;
    rdfs:range <https://w3id.org/biolink/biolinkml/meta/types/String> ;
    skos:definition "The full name, with authorship and date information if known, of the currently valid (zoological) or accepted (botanical) taxon." .

<http://rs.tdwg.org/dwc/terms/acceptedNameUsageID> a owl:ObjectProperty,
        meta:SlotDefinition ;
    rdfs:label "acceptedNameUsageID" ;
    rdfs:range <https://w3id.org/biolink/biolinkml/meta/types/String> ;
    skos:definition "An identifier for the name usage (documented meaning of the name according to a source) of the currently valid (zoological) or accepted (botanical) taxon." .

<http://rs.tdwg.org/dwc/terms/associatedMedia> a owl:ObjectProperty,
        meta:SlotDefinition ;
    rdfs:label "associatedMedia" ;
    rdfs:range <https://w3id.org/biolink/biolinkml/meta/types/String> ;
    skos:definition "A list (concatenated and separated) of identifiers (publication, global unique identifier, URI) of media associated with the Occurrence." .

<http://rs.tdwg.org/dwc/terms/associatedOccurrences> a owl:ObjectProperty,
        meta:SlotDefinition ;
    rdfs:label "associatedOccurrences" ;
    rdfs:range <https://w3id.org/biolink/biolinkml/meta/types/String> ;
    skos:definition "A list (concatenated and separated) of identifiers of other Occurrence records and their associations to this Occurrence." .

<http://rs.tdwg.org/dwc/terms/associatedOrganisms> a owl:ObjectProperty,
        meta:SlotDefinition ;
    rdfs:label "associatedOrganisms" ;
    rdfs:range <https://w3id.org/biolink/biolinkml/meta/types/String> ;
    skos:definition "A list (concatenated and separated) of identifiers of other Organisms and their associations to this Organism." .

<http://rs.tdwg.org/dwc/terms/associatedReferences> a owl:ObjectProperty,
        meta:SlotDefinition ;
    rdfs:label "associatedReferences" ;
    rdfs:range <https://w3id.org/biolink/biolinkml/meta/types/String> ;
    skos:definition "A list (concatenated and separated) of identifiers (publication, bibliographic reference, global unique identifier, URI) of literature associated with the Occurrence." .

<http://rs.tdwg.org/dwc/terms/associatedSequences> a owl:ObjectProperty,
        meta:SlotDefinition ;
    rdfs:label "associatedSequences" ;
    rdfs:range <https://w3id.org/biolink/biolinkml/meta/types/String> ;
    skos:definition "A list (concatenated and separated) of identifiers (publication, global unique identifier, URI) of genetic sequence information associated with the Occurrence." .

<http://rs.tdwg.org/dwc/terms/associatedTaxa> a owl:ObjectProperty,
        meta:SlotDefinition ;
    rdfs:label "associatedTaxa" ;
    rdfs:range <https://w3id.org/biolink/biolinkml/meta/types/String> ;
    skos:definition "A list (concatenated and separated) of identifiers or names of taxa and their associations with the Occurrence." .

<http://rs.tdwg.org/dwc/terms/bed> a owl:ObjectProperty,
        meta:SlotDefinition ;
    rdfs:label "bed" ;
    rdfs:range <https://w3id.org/biolink/biolinkml/meta/types/String> ;
    skos:definition "The full name of the lithostratigraphic bed from which the cataloged item was collected." .

<http://rs.tdwg.org/dwc/terms/behavior> a owl:ObjectProperty,
        meta:SlotDefinition ;
    rdfs:label "behavior" ;
    rdfs:range <https://w3id.org/biolink/biolinkml/meta/types/String> ;
    skos:definition "The behavior shown by the subject at the time the Occurrence was recorded." .

<http://rs.tdwg.org/dwc/terms/catalogNumber> a owl:ObjectProperty,
        meta:SlotDefinition ;
    rdfs:label "catalogNumber" ;
    rdfs:range <https://w3id.org/biolink/biolinkml/meta/types/String> ;
    skos:definition "An identifier (preferably unique) for the record within the data set or collection." .

<http://rs.tdwg.org/dwc/terms/class> a owl:ObjectProperty,
        meta:SlotDefinition ;
    rdfs:label "class" ;
    rdfs:range <https://w3id.org/biolink/biolinkml/meta/types/String> ;
    skos:definition "The full scientific name of the class in which the taxon is classified." .

<http://rs.tdwg.org/dwc/terms/dateIdentified> a owl:ObjectProperty,
        meta:SlotDefinition ;
    rdfs:label "dateIdentified" ;
    rdfs:range <https://w3id.org/biolink/biolinkml/meta/types/String> ;
    skos:definition "The date on which the subject was identified as representing the Taxon." .

<http://rs.tdwg.org/dwc/terms/day> a owl:ObjectProperty,
        meta:SlotDefinition ;
    rdfs:label "day" ;
    rdfs:range <https://w3id.org/biolink/biolinkml/meta/types/String> ;
    skos:definition "The integer day of the month on which the Event occurred." .

<http://rs.tdwg.org/dwc/terms/disposition> a owl:ObjectProperty,
        meta:SlotDefinition ;
    rdfs:label "disposition" ;
    rdfs:range <https://w3id.org/biolink/biolinkml/meta/types/String> ;
    skos:definition "The current state of a specimen with respect to the collection identified in collectionCode or collectionID." .

<http://rs.tdwg.org/dwc/terms/earliestAgeOrLowestStage> a owl:ObjectProperty,
        meta:SlotDefinition ;
    rdfs:label "earliestAgeOrLowestStage" ;
    rdfs:range <https://w3id.org/biolink/biolinkml/meta/types/String> ;
    skos:definition "The full name of the earliest possible geochronologic age or lowest chronostratigraphic stage attributable to the stratigraphic horizon from which the cataloged item was collected." .

<http://rs.tdwg.org/dwc/terms/earliestEonOrLowestEonothem> a owl:ObjectProperty,
        meta:SlotDefinition ;
    rdfs:label "earliestEonOrLowestEonothem" ;
    rdfs:range <https://w3id.org/biolink/biolinkml/meta/types/String> ;
    skos:definition "The full name of the earliest possible geochronologic eon or lowest chrono-stratigraphic eonothem or the informal name (\"Precambrian\") attributable to the stratigraphic horizon from which the cataloged item was collected." .

<http://rs.tdwg.org/dwc/terms/earliestEpochOrLowestSeries> a owl:ObjectProperty,
        meta:SlotDefinition ;
    rdfs:label "earliestEpochOrLowestSeries" ;
    rdfs:range <https://w3id.org/biolink/biolinkml/meta/types/String> ;
    skos:definition "The full name of the earliest possible geochronologic epoch or lowest chronostratigraphic series attributable to the stratigraphic horizon from which the cataloged item was collected." .

<http://rs.tdwg.org/dwc/terms/earliestEraOrLowestErathem> a owl:ObjectProperty,
        meta:SlotDefinition ;
    rdfs:label "earliestEraOrLowestErathem" ;
    rdfs:range <https://w3id.org/biolink/biolinkml/meta/types/String> ;
    skos:definition "The full name of the earliest possible geochronologic era or lowest chronostratigraphic erathem attributable to the stratigraphic horizon from which the cataloged item was collected." .

<http://rs.tdwg.org/dwc/terms/earliestPeriodOrLowestSystem> a owl:ObjectProperty,
        meta:SlotDefinition ;
    rdfs:label "earliestPeriodOrLowestSystem" ;
    rdfs:range <https://w3id.org/biolink/biolinkml/meta/types/String> ;
    skos:definition "The full name of the earliest possible geochronologic period or lowest chronostratigraphic system attributable to the stratigraphic horizon from which the cataloged item was collected." .

<http://rs.tdwg.org/dwc/terms/endDayOfYear> a owl:ObjectProperty,
        meta:SlotDefinition ;
    rdfs:label "endDayOfYear" ;
    rdfs:range <https://w3id.org/biolink/biolinkml/meta/types/String> ;
    skos:definition "The latest ordinal day of the year on which the Event occurred (1 for January 1, 365 for December 31, except in a leap year, in which case it is 366)." .

<http://rs.tdwg.org/dwc/terms/establishmentMeans> a owl:ObjectProperty,
        meta:SlotDefinition ;
    rdfs:label "establishmentMeans" ;
    rdfs:range <https://w3id.org/biolink/biolinkml/meta/types/String> ;
    skos:definition "The process by which the biological individual(s) represented in the Occurrence became established at the location." .

<http://rs.tdwg.org/dwc/terms/eventDate> a owl:ObjectProperty,
        meta:SlotDefinition ;
    rdfs:label "eventDate" ;
    rdfs:range <https://w3id.org/biolink/biolinkml/meta/types/String> ;
    skos:definition "The date-time or interval during which an Event occurred. For occurrences, this is the date-time when the event was recorded. Not suitable for a time in a geological context." .

<http://rs.tdwg.org/dwc/terms/eventID> a owl:ObjectProperty,
        meta:SlotDefinition ;
    rdfs:label "eventID" ;
    rdfs:range <https://w3id.org/biolink/biolinkml/meta/types/String> ;
    skos:definition "An identifier for the set of information associated with an Event (something that occurs at a place and time). May be a global unique identifier or an identifier specific to the data set." .

<http://rs.tdwg.org/dwc/terms/eventRemarks> a owl:ObjectProperty,
        meta:SlotDefinition ;
    rdfs:label "eventRemarks" ;
    rdfs:range <https://w3id.org/biolink/biolinkml/meta/types/String> ;
    skos:definition "Comments or notes about the Event." .

<http://rs.tdwg.org/dwc/terms/eventTime> a owl:ObjectProperty,
        meta:SlotDefinition ;
    rdfs:label "eventTime" ;
    rdfs:range <https://w3id.org/biolink/biolinkml/meta/types/String> ;
    skos:definition "The time or interval during which an Event occurred." .

<http://rs.tdwg.org/dwc/terms/family> a owl:ObjectProperty,
        meta:SlotDefinition ;
    rdfs:label "family" ;
    rdfs:range <https://w3id.org/biolink/biolinkml/meta/types/String> ;
    skos:definition "The full scientific name of the family in which the taxon is classified." .

<http://rs.tdwg.org/dwc/terms/fieldNotes> a owl:ObjectProperty,
        meta:SlotDefinition ;
    rdfs:label "fieldNotes" ;
    rdfs:range <https://w3id.org/biolink/biolinkml/meta/types/String> ;
    skos:definition "One of a) an indicator of the existence of, b) a reference to (publication, URI), or c) the text of notes taken in the field about the Event." .

<http://rs.tdwg.org/dwc/terms/fieldNumber> a owl:ObjectProperty,
        meta:SlotDefinition ;
    rdfs:label "fieldNumber" ;
    rdfs:range <https://w3id.org/biolink/biolinkml/meta/types/String> ;
    skos:definition "An identifier given to the event in the field. Often serves as a link between field notes and the Event." .

<http://rs.tdwg.org/dwc/terms/formation> a owl:ObjectProperty,
        meta:SlotDefinition ;
    rdfs:label "formation" ;
    rdfs:range <https://w3id.org/biolink/biolinkml/meta/types/String> ;
    skos:definition "The full name of the lithostratigraphic formation from which the cataloged item was collected." .

<http://rs.tdwg.org/dwc/terms/genus> a owl:ObjectProperty,
        meta:SlotDefinition ;
    rdfs:label "genus" ;
    rdfs:range <https://w3id.org/biolink/biolinkml/meta/types/String> ;
    skos:definition "The full scientific name of the genus in which the taxon is classified." .

<http://rs.tdwg.org/dwc/terms/geologicalContextID> a owl:ObjectProperty,
        meta:SlotDefinition ;
    rdfs:label "geologicalContextID" ;
    rdfs:range <https://w3id.org/biolink/biolinkml/meta/types/String> ;
    skos:definition "An identifier for the set of information associated with a GeologicalContext (the location within a geological context, such as stratigraphy). May be a global unique identifier or an identifier specific to the data set." .

<http://rs.tdwg.org/dwc/terms/group> a owl:ObjectProperty,
        meta:SlotDefinition ;
    rdfs:label "group" ;
    rdfs:range <https://w3id.org/biolink/biolinkml/meta/types/String> ;
    skos:definition "The full name of the lithostratigraphic group from which the cataloged item was collected." .

<http://rs.tdwg.org/dwc/terms/habitat> a owl:ObjectProperty,
        meta:SlotDefinition ;
    rdfs:label "habitat" ;
    rdfs:range <https://w3id.org/biolink/biolinkml/meta/types/String> ;
    skos:definition "A category or description of the habitat in which the Event occurred." .

<http://rs.tdwg.org/dwc/terms/higherClassification> a owl:ObjectProperty,
        meta:SlotDefinition ;
    rdfs:label "higherClassification" ;
    rdfs:range <https://w3id.org/biolink/biolinkml/meta/types/String> ;
    skos:definition "A list (concatenated and separated) of taxa names terminating at the rank immediately superior to the taxon referenced in the taxon record." .

<http://rs.tdwg.org/dwc/terms/highestBiostratigraphicZone> a owl:ObjectProperty,
        meta:SlotDefinition ;
    rdfs:label "highestBiostratigraphicZone" ;
    rdfs:range <https://w3id.org/biolink/biolinkml/meta/types/String> ;
    skos:definition "The full name of the highest possible geological biostratigraphic zone of the stratigraphic horizon from which the cataloged item was collected." .

<http://rs.tdwg.org/dwc/terms/identificationID> a owl:ObjectProperty,
        meta:SlotDefinition ;
    rdfs:label "identificationID" ;
    rdfs:range <https://w3id.org/biolink/biolinkml/meta/types/String> ;
    skos:definition "An identifier for the Identification (the body of information associated with the assignment of a scientific name). May be a global unique identifier or an identifier specific to the data set." .

<http://rs.tdwg.org/dwc/terms/identificationQualifier> a owl:ObjectProperty,
        meta:SlotDefinition ;
    rdfs:label "identificationQualifier" ;
    rdfs:range <https://w3id.org/biolink/biolinkml/meta/types/String> ;
    skos:definition "A brief phrase or a standard term (\"cf.\", \"aff.\") to express the determiner's doubts about the Identification." .

<http://rs.tdwg.org/dwc/terms/identificationReferences> a owl:ObjectProperty,
        meta:SlotDefinition ;
    rdfs:label "identificationReferences" ;
    rdfs:range <https://w3id.org/biolink/biolinkml/meta/types/String> ;
    skos:definition "A list (concatenated and separated) of references (publication, global unique identifier, URI) used in the Identification." .

<http://rs.tdwg.org/dwc/terms/identificationRemarks> a owl:ObjectProperty,
        meta:SlotDefinition ;
    rdfs:label "identificationRemarks" ;
    rdfs:range <https://w3id.org/biolink/biolinkml/meta/types/String> ;
    skos:definition "Comments or notes about the Identification." .

<http://rs.tdwg.org/dwc/terms/identificationVerificationStatus> a owl:ObjectProperty,
        meta:SlotDefinition ;
    rdfs:label "identificationVerificationStatus" ;
    rdfs:range <https://w3id.org/biolink/biolinkml/meta/types/String> ;
    skos:definition "A categorical indicator of the extent to which the taxonomic identification has been verified to be correct." .

<http://rs.tdwg.org/dwc/terms/identifiedBy> a owl:ObjectProperty,
        meta:SlotDefinition ;
    rdfs:label "identifiedBy" ;
    rdfs:range <https://w3id.org/biolink/biolinkml/meta/types/String> ;
    skos:definition "A list (concatenated and separated) of names of people, groups, or organizations who assigned the Taxon to the subject." .

<http://rs.tdwg.org/dwc/terms/individualCount> a owl:ObjectProperty,
        meta:SlotDefinition ;
    rdfs:label "individualCount" ;
    rdfs:range <https://w3id.org/biolink/biolinkml/meta/types/String> ;
    skos:definition "The number of individuals represented present at the time of the Occurrence." .

<http://rs.tdwg.org/dwc/terms/infraspecificEpithet> a owl:ObjectProperty,
        meta:SlotDefinition ;
    rdfs:label "infraspecificEpithet" ;
    rdfs:range <https://w3id.org/biolink/biolinkml/meta/types/String> ;
    skos:definition "The name of the lowest or terminal infraspecific epithet of the scientificName, excluding any rank designation." .

<http://rs.tdwg.org/dwc/terms/kingdom> a owl:ObjectProperty,
        meta:SlotDefinition ;
    rdfs:label "kingdom" ;
    rdfs:range <https://w3id.org/biolink/biolinkml/meta/types/String> ;
    skos:definition "The full scientific name of the kingdom in which the taxon is classified." .

<http://rs.tdwg.org/dwc/terms/latestAgeOrHighestStage> a owl:ObjectProperty,
        meta:SlotDefinition ;
    rdfs:label "latestAgeOrHighestStage" ;
    rdfs:range <https://w3id.org/biolink/biolinkml/meta/types/String> ;
    skos:definition "The full name of the latest possible geochronologic age or highest chronostratigraphic stage attributable to the stratigraphic horizon from which the cataloged item was collected." .

<http://rs.tdwg.org/dwc/terms/latestEonOrHighestEonothem> a owl:ObjectProperty,
        meta:SlotDefinition ;
    rdfs:label "latestEonOrHighestEonothem" ;
    rdfs:range <https://w3id.org/biolink/biolinkml/meta/types/String> ;
    skos:definition "The full name of the latest possible geochronologic eon or highest chrono-stratigraphic eonothem or the informal name (\"Precambrian\") attributable to the stratigraphic horizon from which the cataloged item was collected." .

<http://rs.tdwg.org/dwc/terms/latestEpochOrHighestSeries> a owl:ObjectProperty,
        meta:SlotDefinition ;
    rdfs:label "latestEpochOrHighestSeries" ;
    rdfs:range <https://w3id.org/biolink/biolinkml/meta/types/String> ;
    skos:definition "The full name of the latest possible geochronologic epoch or highest chronostratigraphic series attributable to the stratigraphic horizon from which the cataloged item was collected." .

<http://rs.tdwg.org/dwc/terms/latestEraOrHighestErathem> a owl:ObjectProperty,
        meta:SlotDefinition ;
    rdfs:label "latestEraOrHighestErathem" ;
    rdfs:range <https://w3id.org/biolink/biolinkml/meta/types/String> ;
    skos:definition "The full name of the latest possible geochronologic era or highest chronostratigraphic erathem attributable to the stratigraphic horizon from which the cataloged item was collected." .

<http://rs.tdwg.org/dwc/terms/latestPeriodOrHighestSystem> a owl:ObjectProperty,
        meta:SlotDefinition ;
    rdfs:label "latestPeriodOrHighestSystem" ;
    rdfs:range <https://w3id.org/biolink/biolinkml/meta/types/String> ;
    skos:definition "The full name of the latest possible geochronologic period or highest chronostratigraphic system attributable to the stratigraphic horizon from which the cataloged item was collected." .

<http://rs.tdwg.org/dwc/terms/lifeStage> a owl:ObjectProperty,
        meta:SlotDefinition ;
    rdfs:label "lifeStage" ;
    rdfs:range <https://w3id.org/biolink/biolinkml/meta/types/String> ;
    skos:definition "The age class or life stage of the biological individual(s) at the time the Occurrence was recorded." .

<http://rs.tdwg.org/dwc/terms/lithostratigraphicTerms> a owl:ObjectProperty,
        meta:SlotDefinition ;
    rdfs:label "lithostratigraphicTerms" ;
    rdfs:range <https://w3id.org/biolink/biolinkml/meta/types/String> ;
    skos:definition "The combination of all litho-stratigraphic names for the rock from which the cataloged item was collected." .

<http://rs.tdwg.org/dwc/terms/lowestBiostratigraphicZone> a owl:ObjectProperty,
        meta:SlotDefinition ;
    rdfs:label "lowestBiostratigraphicZone" ;
    rdfs:range <https://w3id.org/biolink/biolinkml/meta/types/String> ;
    skos:definition "The full name of the lowest possible geological biostratigraphic zone of the stratigraphic horizon from which the cataloged item was collected." .

<http://rs.tdwg.org/dwc/terms/materialSampleID> a owl:ObjectProperty,
        meta:SlotDefinition ;
    rdfs:label "materialSampleID" ;
    rdfs:range <https://w3id.org/biolink/biolinkml/meta/types/String> ;
    skos:definition "An identifier for the MaterialSample (as opposed to a particular digital record of the material sample). In the absence of a persistent global unique identifier, construct one from a combination of identifiers in the record that will most closely make the materialSampleID globally unique." .

<http://rs.tdwg.org/dwc/terms/measurementAccuracy> a owl:ObjectProperty,
        meta:SlotDefinition ;
    rdfs:label "measurementAccuracy" ;
    rdfs:range <https://w3id.org/biolink/biolinkml/meta/types/String> ;
    skos:definition "The description of the potential error associated with the measurementValue." .

<http://rs.tdwg.org/dwc/terms/measurementDeterminedBy> a owl:ObjectProperty,
        meta:SlotDefinition ;
    rdfs:label "measurementDeterminedBy" ;
    rdfs:range <https://w3id.org/biolink/biolinkml/meta/types/String> ;
    skos:definition "A list (concatenated and separated) of names of people, groups, or organizations who determined the value of the MeasurementOrFact." .

<http://rs.tdwg.org/dwc/terms/measurementDeterminedDate> a owl:ObjectProperty,
        meta:SlotDefinition ;
    rdfs:label "measurementDeterminedDate" ;
    rdfs:range <https://w3id.org/biolink/biolinkml/meta/types/String> ;
    skos:definition "The date on which the MeasurementOrFact was made." .

<http://rs.tdwg.org/dwc/terms/measurementID> a owl:ObjectProperty,
        meta:SlotDefinition ;
    rdfs:label "measurementID" ;
    rdfs:range <https://w3id.org/biolink/biolinkml/meta/types/String> ;
    skos:definition "An identifier for the MeasurementOrFact (information pertaining to measurements, facts, characteristics, or assertions). May be a global unique identifier or an identifier specific to the data set." .

<http://rs.tdwg.org/dwc/terms/measurementMethod> a owl:ObjectProperty,
        meta:SlotDefinition ;
    rdfs:label "measurementMethod" ;
    rdfs:range <https://w3id.org/biolink/biolinkml/meta/types/String> ;
    skos:definition "A description of or reference to (publication, URI) the method or protocol used to determine the measurement, fact, characteristic, or assertion." .

<http://rs.tdwg.org/dwc/terms/measurementRemarks> a owl:ObjectProperty,
        meta:SlotDefinition ;
    rdfs:label "measurementRemarks" ;
    rdfs:range <https://w3id.org/biolink/biolinkml/meta/types/String> ;
    skos:definition "Comments or notes accompanying the MeasurementOrFact." .

<http://rs.tdwg.org/dwc/terms/measurementType> a owl:ObjectProperty,
        meta:SlotDefinition ;
    rdfs:label "measurementType" ;
    rdfs:range <https://w3id.org/biolink/biolinkml/meta/types/String> ;
    skos:definition "The nature of the measurement, fact, characteristic, or assertion." .

<http://rs.tdwg.org/dwc/terms/measurementUnit> a owl:ObjectProperty,
        meta:SlotDefinition ;
    rdfs:label "measurementUnit" ;
    rdfs:range <https://w3id.org/biolink/biolinkml/meta/types/String> ;
    skos:definition "The units associated with the measurementValue." .

<http://rs.tdwg.org/dwc/terms/measurementValue> a owl:ObjectProperty,
        meta:SlotDefinition ;
    rdfs:label "measurementValue" ;
    rdfs:range <https://w3id.org/biolink/biolinkml/meta/types/String> ;
    skos:definition "The value of the measurement, fact, characteristic, or assertion." .

<http://rs.tdwg.org/dwc/terms/member> a owl:ObjectProperty,
        meta:SlotDefinition ;
    rdfs:label "member" ;
    rdfs:range <https://w3id.org/biolink/biolinkml/meta/types/String> ;
    skos:definition "The full name of the lithostratigraphic member from which the cataloged item was collected." .

<http://rs.tdwg.org/dwc/terms/month> a owl:ObjectProperty,
        meta:SlotDefinition ;
    rdfs:label "month" ;
    rdfs:range <https://w3id.org/biolink/biolinkml/meta/types/String> ;
    skos:definition "The ordinal month in which the Event occurred." .

<http://rs.tdwg.org/dwc/terms/nameAccordingTo> a owl:ObjectProperty,
        meta:SlotDefinition ;
    rdfs:label "nameAccordingTo" ;
    rdfs:range <https://w3id.org/biolink/biolinkml/meta/types/String> ;
    skos:definition "The reference to the source in which the specific taxon concept circumscription is defined or implied - traditionally signified by the Latin \"sensu\" or \"sec.\" (from secundum, meaning \"according to\"). For taxa that result from identifications, a reference to the keys, monographs, experts and other sources should be given." .

<http://rs.tdwg.org/dwc/terms/nameAccordingToID> a owl:ObjectProperty,
        meta:SlotDefinition ;
    rdfs:label "nameAccordingToID" ;
    rdfs:range <https://w3id.org/biolink/biolinkml/meta/types/String> ;
    skos:definition "An identifier for the source in which the specific taxon concept circumscription is defined or implied. See nameAccordingTo." .

<http://rs.tdwg.org/dwc/terms/namePublishedIn> a owl:ObjectProperty,
        meta:SlotDefinition ;
    rdfs:label "namePublishedIn" ;
    rdfs:range <https://w3id.org/biolink/biolinkml/meta/types/String> ;
    skos:definition "A reference for the publication in which the scientificName was originally established under the rules of the associated nomenclaturalCode." .

<http://rs.tdwg.org/dwc/terms/namePublishedInID> a owl:ObjectProperty,
        meta:SlotDefinition ;
    rdfs:label "namePublishedInID" ;
    rdfs:range <https://w3id.org/biolink/biolinkml/meta/types/String> ;
    skos:definition "An identifier for the publication in which the scientificName was originally established under the rules of the associated nomenclaturalCode." .

<http://rs.tdwg.org/dwc/terms/namePublishedInYear> a owl:ObjectProperty,
        meta:SlotDefinition ;
    rdfs:label "namePublishedInYear" ;
    rdfs:range <https://w3id.org/biolink/biolinkml/meta/types/String> ;
    skos:definition "The four-digit year in which the scientificName was published." .

<http://rs.tdwg.org/dwc/terms/nomenclaturalCode> a owl:ObjectProperty,
        meta:SlotDefinition ;
    rdfs:label "nomenclaturalCode" ;
    rdfs:range <https://w3id.org/biolink/biolinkml/meta/types/String> ;
    skos:definition "The nomenclatural code (or codes in the case of an ambiregnal name) under which the scientificName is constructed." .

<http://rs.tdwg.org/dwc/terms/nomenclaturalStatus> a owl:ObjectProperty,
        meta:SlotDefinition ;
    rdfs:label "nomenclaturalStatus" ;
    rdfs:range <https://w3id.org/biolink/biolinkml/meta/types/String> ;
    skos:definition "The status related to the original publication of the name and its conformance to the relevant rules of nomenclature. It is based essentially on an algorithm according to the business rules of the code. It requires no taxonomic opinion." .

<http://rs.tdwg.org/dwc/terms/occurrenceID> a owl:ObjectProperty,
        meta:SlotDefinition ;
    rdfs:label "occurrenceID" ;
    rdfs:range <https://w3id.org/biolink/biolinkml/meta/types/String> ;
    skos:definition "An identifier for the Occurrence (as opposed to a particular digital record of the occurrence). In the absence of a persistent global unique identifier, construct one from a combination of identifiers in the record that will most closely make the occurrenceID globally unique." .

<http://rs.tdwg.org/dwc/terms/occurrenceRemarks> a owl:ObjectProperty,
        meta:SlotDefinition ;
    rdfs:label "occurrenceRemarks" ;
    rdfs:range <https://w3id.org/biolink/biolinkml/meta/types/String> ;
    skos:definition "Comments or notes about the Occurrence." .

<http://rs.tdwg.org/dwc/terms/occurrenceStatus> a owl:ObjectProperty,
        meta:SlotDefinition ;
    rdfs:label "occurrenceStatus" ;
    rdfs:range <https://w3id.org/biolink/biolinkml/meta/types/String> ;
    skos:definition "A statement about the presence or absence of a Taxon at a Location." .

<http://rs.tdwg.org/dwc/terms/order> a owl:ObjectProperty,
        meta:SlotDefinition ;
    rdfs:label "order" ;
    rdfs:range <https://w3id.org/biolink/biolinkml/meta/types/String> ;
    skos:definition "The full scientific name of the order in which the taxon is classified." .

<http://rs.tdwg.org/dwc/terms/organismID> a owl:ObjectProperty,
        meta:SlotDefinition ;
    rdfs:label "organismID" ;
    rdfs:range <https://w3id.org/biolink/biolinkml/meta/types/String> ;
    skos:definition "An identifier for the Organism instance (as opposed to a particular digital record of the Organism). May be a globally unique identifier or an identifier specific to the data set." .

<http://rs.tdwg.org/dwc/terms/organismName> a owl:ObjectProperty,
        meta:SlotDefinition ;
    rdfs:label "organismName" ;
    rdfs:range <https://w3id.org/biolink/biolinkml/meta/types/String> ;
    skos:definition "A textual name or label assigned to an Organism instance." .

<http://rs.tdwg.org/dwc/terms/organismQuantity> a owl:ObjectProperty,
        meta:SlotDefinition ;
    rdfs:label "organismQuantity" ;
    rdfs:range <https://w3id.org/biolink/biolinkml/meta/types/String> ;
    skos:definition "A number or enumeration value for the quantity of organisms." .

<http://rs.tdwg.org/dwc/terms/organismQuantityType> a owl:ObjectProperty,
        meta:SlotDefinition ;
    rdfs:label "organismQuantityType" ;
    rdfs:range <https://w3id.org/biolink/biolinkml/meta/types/String> ;
    skos:definition "The type of quantification system used for the quantity of organisms." .

<http://rs.tdwg.org/dwc/terms/organismRemarks> a owl:ObjectProperty,
        meta:SlotDefinition ;
    rdfs:label "organismRemarks" ;
    rdfs:range <https://w3id.org/biolink/biolinkml/meta/types/String> ;
    skos:definition "Comments or notes about the Organism instance." .

<http://rs.tdwg.org/dwc/terms/organismScope> a owl:ObjectProperty,
        meta:SlotDefinition ;
    rdfs:label "organismScope" ;
    rdfs:range <https://w3id.org/biolink/biolinkml/meta/types/String> ;
    skos:definition "A description of the kind of Organism instance. Can be used to indicate whether the Organism instance represents a discrete organism or if it represents a particular type of aggregation." .

<http://rs.tdwg.org/dwc/terms/originalNameUsage> a owl:ObjectProperty,
        meta:SlotDefinition ;
    rdfs:label "originalNameUsage" ;
    rdfs:range <https://w3id.org/biolink/biolinkml/meta/types/String> ;
    skos:definition "The taxon name, with authorship and date information if known, as it originally appeared when first established under the rules of the associated nomenclaturalCode. The basionym (botany) or basonym (bacteriology) of the scientificName or the senior/earlier homonym for replaced names." .

<http://rs.tdwg.org/dwc/terms/originalNameUsageID> a owl:ObjectProperty,
        meta:SlotDefinition ;
    rdfs:label "originalNameUsageID" ;
    rdfs:range <https://w3id.org/biolink/biolinkml/meta/types/String> ;
    skos:definition "An identifier for the name usage (documented meaning of the name according to a source) in which the terminal element of the scientificName was originally established under the rules of the associated nomenclaturalCode." .

<http://rs.tdwg.org/dwc/terms/otherCatalogNumbers> a owl:ObjectProperty,
        meta:SlotDefinition ;
    rdfs:label "otherCatalogNumbers" ;
    rdfs:range <https://w3id.org/biolink/biolinkml/meta/types/String> ;
    skos:definition "A list (concatenated and separated) of previous or alternate fully qualified catalog numbers or other human-used identifiers for the same Occurrence, whether in the current or any other data set or collection." .

<http://rs.tdwg.org/dwc/terms/parentEventID> a owl:ObjectProperty,
        meta:SlotDefinition ;
    rdfs:label "parentEventID" ;
    rdfs:range <https://w3id.org/biolink/biolinkml/meta/types/String> ;
    skos:definition "An identifier for the broader Event that groups this and potentially other Events." .

<http://rs.tdwg.org/dwc/terms/parentNameUsage> a owl:ObjectProperty,
        meta:SlotDefinition ;
    rdfs:label "parentNameUsage" ;
    rdfs:range <https://w3id.org/biolink/biolinkml/meta/types/String> ;
    skos:definition "The full name, with authorship and date information if known, of the direct, most proximate higher-rank parent taxon (in a classification) of the most specific element of the scientificName." .

<http://rs.tdwg.org/dwc/terms/parentNameUsageID> a owl:ObjectProperty,
        meta:SlotDefinition ;
    rdfs:label "parentNameUsageID" ;
    rdfs:range <https://w3id.org/biolink/biolinkml/meta/types/String> ;
    skos:definition "An identifier for the name usage (documented meaning of the name according to a source) of the direct, most proximate higher-rank parent taxon (in a classification) of the most specific element of the scientificName." .

<http://rs.tdwg.org/dwc/terms/phylum> a owl:ObjectProperty,
        meta:SlotDefinition ;
    rdfs:label "phylum" ;
    rdfs:range <https://w3id.org/biolink/biolinkml/meta/types/String> ;
    skos:definition "The full scientific name of the phylum or division in which the taxon is classified." .

<http://rs.tdwg.org/dwc/terms/preparations> a owl:ObjectProperty,
        meta:SlotDefinition ;
    rdfs:label "preparations" ;
    rdfs:range <https://w3id.org/biolink/biolinkml/meta/types/String> ;
    skos:definition "A list (concatenated and separated) of preparations and preservation methods for a specimen." .

<http://rs.tdwg.org/dwc/terms/previousIdentifications> a owl:ObjectProperty,
        meta:SlotDefinition ;
    rdfs:label "previousIdentifications" ;
    rdfs:range <https://w3id.org/biolink/biolinkml/meta/types/String> ;
    skos:definition "A list (concatenated and separated) of previous assignments of names to the Organism." .

<http://rs.tdwg.org/dwc/terms/recordNumber> a owl:ObjectProperty,
        meta:SlotDefinition ;
    rdfs:label "recordNumber" ;
    rdfs:range <https://w3id.org/biolink/biolinkml/meta/types/String> ;
    skos:definition "An identifier given to the Occurrence at the time it was recorded. Often serves as a link between field notes and an Occurrence record, such as a specimen collector's number." .

<http://rs.tdwg.org/dwc/terms/recordedBy> a owl:ObjectProperty,
        meta:SlotDefinition ;
    rdfs:label "recordedBy" ;
    rdfs:range <https://w3id.org/biolink/biolinkml/meta/types/String> ;
    skos:definition "A list (concatenated and separated) of names of people, groups, or organizations responsible for recording the original Occurrence. The primary collector or observer, especially one who applies a personal identifier (recordNumber), should be listed first." .

<http://rs.tdwg.org/dwc/terms/relatedResourceID> a owl:ObjectProperty,
        meta:SlotDefinition ;
    rdfs:label "relatedResourceID" ;
    rdfs:range <https://w3id.org/biolink/biolinkml/meta/types/String> ;
    skos:definition "An identifier for a related resource (the object, rather than the subject of the relationship)." .

<http://rs.tdwg.org/dwc/terms/relationshipAccordingTo> a owl:ObjectProperty,
        meta:SlotDefinition ;
    rdfs:label "relationshipAccordingTo" ;
    rdfs:range <https://w3id.org/biolink/biolinkml/meta/types/String> ;
    skos:definition "The source (person, organization, publication, reference) establishing the relationship between the two resources." .

<http://rs.tdwg.org/dwc/terms/relationshipEstablishedDate> a owl:ObjectProperty,
        meta:SlotDefinition ;
    rdfs:label "relationshipEstablishedDate" ;
    rdfs:range <https://w3id.org/biolink/biolinkml/meta/types/String> ;
    skos:definition "The date-time on which the relationship between the two resources was established." .

<http://rs.tdwg.org/dwc/terms/relationshipOfResource> a owl:ObjectProperty,
        meta:SlotDefinition ;
    rdfs:label "relationshipOfResource" ;
    rdfs:range <https://w3id.org/biolink/biolinkml/meta/types/String> ;
    skos:definition "The relationship of the resource identified by relatedResourceID to the subject (optionally identified by the resourceID)." .

<http://rs.tdwg.org/dwc/terms/relationshipRemarks> a owl:ObjectProperty,
        meta:SlotDefinition ;
    rdfs:label "relationshipRemarks" ;
    rdfs:range <https://w3id.org/biolink/biolinkml/meta/types/String> ;
    skos:definition "Comments or notes about the relationship between the two resources." .

<http://rs.tdwg.org/dwc/terms/reproductiveCondition> a owl:ObjectProperty,
        meta:SlotDefinition ;
    rdfs:label "reproductiveCondition" ;
    rdfs:range <https://w3id.org/biolink/biolinkml/meta/types/String> ;
    skos:definition "The reproductive condition of the biological individual(s) represented in the Occurrence." .

<http://rs.tdwg.org/dwc/terms/resourceID> a owl:ObjectProperty,
        meta:SlotDefinition ;
    rdfs:label "resourceID" ;
    rdfs:range <https://w3id.org/biolink/biolinkml/meta/types/String> ;
    skos:definition "An identifier for the resource that is the subject of the relationship." .

<http://rs.tdwg.org/dwc/terms/resourceRelationshipID> a owl:ObjectProperty,
        meta:SlotDefinition ;
    rdfs:label "resourceRelationshipID" ;
    rdfs:range <https://w3id.org/biolink/biolinkml/meta/types/String> ;
    skos:definition "An identifier for an instance of relationship between one resource (the subject) and another (relatedResource, the object)." .

<http://rs.tdwg.org/dwc/terms/sampleSizeUnit> a owl:ObjectProperty,
        meta:SlotDefinition ;
    rdfs:label "sampleSizeUnit" ;
    rdfs:range <https://w3id.org/biolink/biolinkml/meta/types/String> ;
    skos:definition "The unit of measurement of the size (time duration, length, area, or volume) of a sample in a sampling event." .

<http://rs.tdwg.org/dwc/terms/sampleSizeValue> a owl:ObjectProperty,
        meta:SlotDefinition ;
    rdfs:label "sampleSizeValue" ;
    rdfs:range <https://w3id.org/biolink/biolinkml/meta/types/String> ;
    skos:definition "A numeric value for a measurement of the size (time duration, length, area, or volume) of a sample in a sampling event." .

<http://rs.tdwg.org/dwc/terms/samplingEffort> a owl:ObjectProperty,
        meta:SlotDefinition ;
    rdfs:label "samplingEffort" ;
    rdfs:range <https://w3id.org/biolink/biolinkml/meta/types/String> ;
    skos:definition "The amount of effort expended during an Event." .

<http://rs.tdwg.org/dwc/terms/samplingProtocol> a owl:ObjectProperty,
        meta:SlotDefinition ;
    rdfs:label "samplingProtocol" ;
    rdfs:range <https://w3id.org/biolink/biolinkml/meta/types/String> ;
    skos:definition "The name of, reference to, or description of the method or protocol used during an Event." .

<http://rs.tdwg.org/dwc/terms/scientificName> a owl:ObjectProperty,
        meta:SlotDefinition ;
    rdfs:label "scientificName" ;
    rdfs:range <https://w3id.org/biolink/biolinkml/meta/types/String> ;
    skos:definition "The full scientific name, with authorship and date information if known. When forming part of an Identification, this should be the name in lowest level taxonomic rank that can be determined. This term should not contain identification qualifications, which should instead be supplied in the IdentificationQualifier term." .

<http://rs.tdwg.org/dwc/terms/scientificNameAuthorship> a owl:ObjectProperty,
        meta:SlotDefinition ;
    rdfs:label "scientificNameAuthorship" ;
    rdfs:range <https://w3id.org/biolink/biolinkml/meta/types/String> ;
    skos:definition "The authorship information for the scientificName formatted according to the conventions of the applicable nomenclaturalCode." .

<http://rs.tdwg.org/dwc/terms/scientificNameID> a owl:ObjectProperty,
        meta:SlotDefinition ;
    rdfs:label "scientificNameID" ;
    rdfs:range <https://w3id.org/biolink/biolinkml/meta/types/String> ;
    skos:definition "An identifier for the nomenclatural (not taxonomic) details of a scientific name." .

<http://rs.tdwg.org/dwc/terms/sex> a owl:ObjectProperty,
        meta:SlotDefinition ;
    rdfs:label "sex" ;
    rdfs:range <https://w3id.org/biolink/biolinkml/meta/types/String> ;
    skos:definition "The sex of the biological individual(s) represented in the Occurrence." .

<http://rs.tdwg.org/dwc/terms/specificEpithet> a owl:ObjectProperty,
        meta:SlotDefinition ;
    rdfs:label "specificEpithet" ;
    rdfs:range <https://w3id.org/biolink/biolinkml/meta/types/String> ;
    skos:definition "The name of the first or species epithet of the scientificName." .

<http://rs.tdwg.org/dwc/terms/startDayOfYear> a owl:ObjectProperty,
        meta:SlotDefinition ;
    rdfs:label "startDayOfYear" ;
    rdfs:range <https://w3id.org/biolink/biolinkml/meta/types/String> ;
    skos:definition "The earliest ordinal day of the year on which the Event occurred (1 for January 1, 365 for December 31, except in a leap year, in which case it is 366)." .

<http://rs.tdwg.org/dwc/terms/subgenus> a owl:ObjectProperty,
        meta:SlotDefinition ;
    rdfs:label "subgenus" ;
    rdfs:range <https://w3id.org/biolink/biolinkml/meta/types/String> ;
    skos:definition "The full scientific name of the subgenus in which the taxon is classified. Values should include the genus to avoid homonym confusion." .

<http://rs.tdwg.org/dwc/terms/taxonConceptID> a owl:ObjectProperty,
        meta:SlotDefinition ;
    rdfs:label "taxonConceptID" ;
    rdfs:range <https://w3id.org/biolink/biolinkml/meta/types/String> ;
    skos:definition "An identifier for the taxonomic concept to which the record refers - not for the nomenclatural details of a taxon." .

<http://rs.tdwg.org/dwc/terms/taxonID> a owl:ObjectProperty,
        meta:SlotDefinition ;
    rdfs:label "taxonID" ;
    rdfs:range <https://w3id.org/biolink/biolinkml/meta/types/String> ;
    skos:definition "An identifier for the set of taxon information (data associated with the Taxon class). May be a global unique identifier or an identifier specific to the data set." .

<http://rs.tdwg.org/dwc/terms/taxonRank> a owl:ObjectProperty,
        meta:SlotDefinition ;
    rdfs:label "taxonRank" ;
    rdfs:range <https://w3id.org/biolink/biolinkml/meta/types/String> ;
    skos:definition "The taxonomic rank of the most specific name in the scientificName." .

<http://rs.tdwg.org/dwc/terms/taxonRemarks> a owl:ObjectProperty,
        meta:SlotDefinition ;
    rdfs:label "taxonRemarks" ;
    rdfs:range <https://w3id.org/biolink/biolinkml/meta/types/String> ;
    skos:definition "Comments or notes about the taxon or name." .

<http://rs.tdwg.org/dwc/terms/taxonomicStatus> a owl:ObjectProperty,
        meta:SlotDefinition ;
    rdfs:label "taxonomicStatus" ;
    rdfs:range <https://w3id.org/biolink/biolinkml/meta/types/String> ;
    skos:definition "The status of the use of the scientificName as a label for a taxon. Requires taxonomic opinion to define the scope of a taxon. Rules of priority then are used to define the taxonomic status of the nomenclature contained in that scope, combined with the experts opinion. It must be linked to a specific taxonomic reference that defines the concept." .

<http://rs.tdwg.org/dwc/terms/typeStatus> a owl:ObjectProperty,
        meta:SlotDefinition ;
    rdfs:label "typeStatus" ;
    rdfs:range <https://w3id.org/biolink/biolinkml/meta/types/String> ;
    skos:definition "A list (concatenated and separated) of nomenclatural types (type status, typified scientific name, publication) applied to the subject." .

<http://rs.tdwg.org/dwc/terms/verbatimEventDate> a owl:ObjectProperty,
        meta:SlotDefinition ;
    rdfs:label "verbatimEventDate" ;
    rdfs:range <https://w3id.org/biolink/biolinkml/meta/types/String> ;
    skos:definition "The verbatim original representation of the date and time information for an Event." .

<http://rs.tdwg.org/dwc/terms/verbatimTaxonRank> a owl:ObjectProperty,
        meta:SlotDefinition ;
    rdfs:label "verbatimTaxonRank" ;
    rdfs:range <https://w3id.org/biolink/biolinkml/meta/types/String> ;
    skos:definition "The taxonomic rank of the most specific name in the scientificName as it appears in the original record." .

<http://rs.tdwg.org/dwc/terms/vernacularName> a owl:ObjectProperty,
        meta:SlotDefinition ;
    rdfs:label "vernacularName" ;
    rdfs:range <https://w3id.org/biolink/biolinkml/meta/types/String> ;
    skos:definition "A common or vernacular name." .

<http://rs.tdwg.org/dwc/terms/year> a owl:ObjectProperty,
        meta:SlotDefinition ;
    rdfs:label "year" ;
    rdfs:range <https://w3id.org/biolink/biolinkml/meta/types/String> ;
    skos:definition "The four-digit year in which the Event occurred, according to the Common Era Calendar." .

meta:TypeDefinition a owl:Class ;
    rdfs:label "type_definition" ;
    skos:definition "A data type definition." .

meta:topValue a owl:DatatypeProperty ;
    rdfs:label "value" .

meta:ClassDefinition a owl:Class ;
    rdfs:label "class_definition" ;
    skos:definition "the definition of a class or interface" .

meta:SlotDefinition a owl:Class ;
    rdfs:label "slot_definition" ;
    skos:definition "the definition of a property or a slot" .

<https://w3id.org/biolink/biolinkml/meta/types/String> a owl:Class,
        meta:TypeDefinition ;
    rdfs:label "string" ;
    rdfs:subClassOf [ a owl:Restriction ;
            owl:onDataRange xsd:string ;
            owl:onProperty meta:topValue ;
            owl:qualifiedCardinality 1 ] ;
    skos:definition "A character string" .



